edited and fix all project according to new fiixes

hol/policy_to_table/tables_specScript.sml
@@ -28,299 +28,131 @@ open bdd_genTheory;
 open pred_specTheory;     
 open policy_specTheory;     
      
-
+open tables_spec_oldTheory;
 
 val _ = new_theory "tables_spec";
 
     
 
-(* atomic variable based predicates predicates*)
-val _ = Hol_datatype `
-     atom_var = True
-                | False
-                | NotTrue
-                | NotFalse
-                | Var of string
-                | Not of string
-               `;
-
-val _ = Hol_datatype `action_expr = action of 'a | state of num`;
-
-
-Type var_line = “:(atom_var list # num # 'a action_expr)”;
-Type var_table = “: ('a var_line) list”
-Type var_table_list = “: ('a var_table) list”
-   
-
-
-
-(***************************************************)
-(* some work for the variable based atoms          *)
-(***************************************************)
-
-
-
-Definition sem_var_atom_def:
-  (sem_var_atom ((Var x): atom_var) mv = (ALOOKUP mv x)) /\
-  (sem_var_atom True _ = SOME T) /\
-  (sem_var_atom False _ = SOME F) /\
-  (sem_var_atom NotTrue _ = SOME F) /\
-  (sem_var_atom NotFalse _ = SOME T) /\
-  (sem_var_atom (Not x) mv = 
-   case (ALOOKUP mv x) of
-   | SOME b => SOME (~b)
-   | _ => NONE
-  )
+Definition is_not_true_var_atom_def:
+  (is_not_true_var_atom True = F) ∧
+  (is_not_true_var_atom _ = T)
 End
 
 
-Definition mk_substitute_atom_def:
-  (mk_substitute_atom (True:atom_var) x b = True) ∧
-  (mk_substitute_atom False x b = False) ∧
-  (mk_substitute_atom NotTrue x b = NotTrue) ∧
-  (mk_substitute_atom NotFalse x b = NotFalse) ∧
-  (mk_substitute_atom (Var x') x b = 
-   if (x=x') then (if b then True else False) else (Var x')) ∧
-  (mk_substitute_atom (Not x') x b = 
-   if (x=x') then (if b then NotTrue else NotFalse) else (Not x'))
-End
-
-   
-Definition simp_atom_def:
-  (simp_atom ((Var x):atom_var) = Var x) /\
-  (simp_atom True = True) /\
-  (simp_atom False = False) /\
-  (simp_atom NotTrue = False) /\
-  (simp_atom NotFalse = True) /\
-  (simp_atom (Not x) = Not x)
-End
-
-
-Definition final_atom_def:
-  final_atom (p:atom_var) = 
-  case p of
-  | True => SOME T
-  | False => SOME F
-  | NotTrue => SOME F
-  | NotFalse => SOME T
-  | _ => NONE
-End
-
-
-Definition fv_atom_def:
-  (fv_atom ((Var x):atom_var) = [x]) ∧
-  (fv_atom True = []) ∧
-  (fv_atom False = []) ∧
-  (fv_atom NotTrue = []) ∧
-  (fv_atom NotFalse = []) ∧
-  (fv_atom (Not x) = [x])
-End
-
-                        
-                
-(***************************************************)
-(* specialized definitions for a predicate record. *)
-(*   here 'a would be policy and 'b would be       *) 
-(*          action wrt record data type            *)
-(***************************************************)
-
-           
-
-(* Check if all predicates in list evaluate to true *)
-Definition is_atoml_true_def:
-  is_atoml_true atoml mv = 
-  EVERY (\minipred. sem_var_atom minipred mv = SOME T) atoml
-End
-
-        
-(* Check if row matches current state and guard conditions *)
-Definition is_match_row_def:
-  is_match_row st_in st_num atoml mv = 
-    ((st_in = st_num) ∧ is_atoml_true atoml mv ∧ atoml ≠ [])
-End
-
-
-Definition check_all_rows_match_def:
-  check_all_rows_match st_in tbl mv =
-  MAP (\(atoml,st_num,res). (is_match_row st_in st_num atoml mv, res)) tbl
-End
-
-
-
-(* Find first matching line in a single table *)
-Definition match_tbl_def:
-  match_tbl (tbl: 'a var_table) mv st_in =
-  let lines_res = (check_all_rows_match st_in tbl mv) in
-    case min_idx_till lines_res T of
-    | SOME (idx, line) => SOME (SND line)
-    | NONE => NONE
-End
-
-
-        
-        
-        
-(* Process table list with state propagation *) 
-Definition match_tbll_def:
-  match_tbll ([]: 'a var_table_list) mv st_in = NONE ∧
-  match_tbll [tbl] mv st_in =
-  ( case match_tbl tbl mv st_in of
-    | SOME (action a) => SOME (action a)
-    | _ => NONE       
-  )∧
-  match_tbll (tbl::tbls) mv st_in =
-  ( case match_tbl tbl mv st_in of
-    | SOME (state n) => match_tbll tbls mv n
-    | _ => NONE
-  )
-End
-
- 
-(* Top-level table semantics, return the starting state as well*)       
-Definition sem_tables_def:
-  sem_tables ((tbll: 'a var_table_list),st_in) mv =
-   match_tbll tbll mv st_in
-End
-
-
-(*
-EVAL “match_tbl [([False], 0 , action "s")] [] 0”;
-EVAL “match_tbl [([True], 0 , action "s")] [] 0”;
-EVAL “match_tbl [([Var "a"], 0 , action "s1");([True], 0 , action "s2")] [("a",T)] 0”;
-EVAL “match_tbl [([Var "a"; True], 0 , action "s1"); ([True], 0 , action "s2")] [("a",T)] 0”;
-
-                    
-EVAL “match_tbl [([False;True],0,state 2); ([False],0,state 3);([True],0,state 3)] [] 0”;
-EVAL “match_tbl [([True],3,state 4); ([False],3,state 5); ([True],2,state 2)] [] 3”;
-EVAL “match_tbl [([True],2,action ("fwd",[(1:num)])); ([True],4,action ("fwd",[2])); ([True],5,action ("drop",[]))] [] 4”;
-
-
-EVAL “sem_tables ([[([False],0,state 2); ([False],0,state 3);([True],0,state 3)];
-                  [([True],3,state 4); ([False],3,state 5); ([True],2,state 2)];
-                  [([True],2,action ("fwd",[1])); ([True],4,action ("fwd",[2])); ([True],5,action ("drop",[]))]],0) []”                  
-*)
-
-      
-(* table substitute *)
-                          
-Definition mk_substitute_row_def:
-  mk_substitute_row atoml x b =
-    MAP (\atom. mk_substitute_atom atom x b) atoml
-End
-   
-Definition mk_substitute_tbl_def:
-  mk_substitute_tbl (tbl: 'a var_table) x b =
-  ((MAP (\(atoml,st_num,res). (mk_substitute_row atoml x b, st_num, res)) tbl) :'a var_table)
-End
-
-   
-Definition mk_substitute_tbll_def:
-  mk_substitute_tbll (tbll: 'a var_table_list) x b =
-  MAP (\(tbl). mk_substitute_tbl (tbl: 'a var_table) x b) tbll 
-End
-
-
-Definition mk_substitute_tables_def:
-  mk_substitute_tables ((tbll: 'a var_table_list), st_in) x b =
-   (mk_substitute_tbll tbll x b, st_in:num)
-End
-        
-(* table simplifications *)
 
 Definition simp_row_def:
   simp_row atoml =
-  let simplified_row = MAP (\atom. simp_atom atom) atoml in
-    case MEM False simplified_row of
-    | T => MAP (\a. False) atoml
-    | F => simplified_row
+  if atoml = [] then [] else
+  let simp_row = MAP (\atom. simp_atom atom) atoml in
+    let simp_row' = FILTER (\x. is_not_true_var_atom x) simp_row in
+      case simp_row' of
+      | [] => [True]
+      | _ => 
+          (case MEM False simp_row' of
+           | T => [False]
+           | F => simp_row')
 End
 
 
-Definition simp_tbl_def:
-  simp_tbl (tbl: 'a var_table) =
-  MAP (\(atoml,st_num,res). simp_row atoml,st_num,res) tbl
+
+
+
+(*
+here we work with none, and some.
+these represent the state of the previous table.
+
+   If the previous table is final, it menas it has only one line and one state as a result.
+   this state as a reult represent the answer of the previous table, that we will use to match on the current table.
+
+   If is it SOME (st_num), then we have the ability to reduce the current table so much, otherwise,
+   if NONE, then we do not know the previous table what it could return yet,
+   thus we reduce but not as much when evaluating it EVAL. 
+
+
+   
+*)
+
+
+        
+Definition simp_table_def:
+  (simp_table [] s = []) ∧
+                  
+  (simp_table ((atoms,st,res)::table)  NONE =
+   let atoms' = simp_row atoms in
+     case atoms' of
+     | [False] => simp_table table NONE
+     | _ =>  ((atoms', st, res)::simp_table table NONE)
+  ) ∧
+    
+  (simp_table ((atoms,st,res)::table) (SOME s') =
+   if (s' ≠ st) then
+     simp_table table (SOME s')
+   else
+     (
+     let atoms' = simp_row atoms in
+       case atoms' of
+       | [False] => simp_table table (SOME s')
+       | [True] => [(atoms', st, res)]
+       | _ =>  ((atoms', st, res) :: (simp_table table (SOME s')))
+     )
+  )
 End
 
 
-Definition simp_tbll_def:
-  simp_tbll (tbll: 'a var_table_list) =
-  MAP (\tbl. simp_tbl tbl) tbll
-End
 
+(* simplify table by table in the tables list. if the table is final i.e.
+   one row only and containng true, then we know what is the state to match on
+   the next table in the list, else we just casually reduce *)
 
 Definition simp_tables_def:
-  simp_tables ((tbll: 'a var_table_list), st_in) =
-   (simp_tbll tbll, st_in:num)
+  (simp_tables [] s = []) ∧
+  (simp_tables (t::tbll) s = 
+   (let t' = simp_table t s in
+      ( case t' of
+        | [([True], st , state s'')] => (t'::(simp_tables tbll (SOME s'')))
+        | _ => (t'::(simp_tables tbll NONE))
+      )
+   )
+  )
 End
 
 
-(*
-EVAL “simp_tbl [([False], 0 , action "s")]”;
-EVAL “simp_tbl [([True; False], 0 , action "s")]”;
-EVAL “simp_tbl [([Var "a"], 0 , action "s1");([True;False], 0 , action "s2")]”;
-EVAL “simp_tbl [([Var "a"; False], 0 , action "s1"); ([True], 0 , action "s2")]”;
-
-EVAL “simp_tbll   ([[([False; Var "a"],0,state 2); ([False],0,state 3);([True],0,state 3)];
-                  [([True],3,state 4); ([False],3,state 5); ([True],2,state 2)];
-                  [([Var "a"; False], 0 , action "s1"); ([True], 0 , action "s2")]]) ”                  
-*)
 
 
+Definition simp_tables_wrapper_def:
+  simp_tables_wrapper ((tbll: 'a var_table_list), st_in) =
+   (simp_tables tbll (SOME st_in), st_in)
+End
+
+
+
+
+
+
+(*****************************)
+
+
+Definition final_row_def:
+  (final_row ([],_,_) s = NONE) ∧
+  (final_row ([True], s', s'') s = (if s = s' then SOME s'' else NONE)) ∧
+  (final_row _ s = NONE)
+End
         
-(* table final *)
-
-Definition all_true_def:
-  all_true atoml =
-  EVERY (\atom. atom = True) atoml
-End
-
-
-Definition all_false_def:
-  all_false atoml =
-  EVERY (\atom. atom = False) atoml
-End
-        
-       
-Definition is_hit_def:
-  is_hit st_in st_num atoml = 
-    ((st_in = st_num) ∧ all_true atoml ∧ atoml ≠ [])
-End
-
-
-Definition is_hit_tbl_check_def:
-  is_hit_tbl_check (tbl: 'a var_table) st_in =
-  MAP (\(atoml, st_num, res). is_hit st_in st_num atoml, st_num, res) tbl
-End
 
 
 
-Definition pre_lines_are_fail_def:
-  pre_lines_are_fail (tbl: 'a var_table) idx st_in =
-  EVERY (\(atoml, st_num, res).  if st_num = st_in then all_false atoml else T) (SEG idx 0 tbl)
-End
-
-        
 Definition final_tbl_def:
-  final_tbl (tbl: 'a var_table) st_in =
-  let lines_res = is_hit_tbl_check tbl st_in in
-    case min_idx_till lines_res T of
-    | SOME (idx, b, st_num, res) =>
-        ( case pre_lines_are_fail tbl idx st_in of
-          | T => SOME res
-          | F => NONE
-        )
-    | _ => NONE
+  (final_tbl [] s = NONE) ∧
+  (final_tbl (row::rows) s =         
+     case final_row row s of
+       SOME a => SOME a
+     | NONE => if (FST row = [False]) then final_tbl rows s else NONE
+  )
 End
 
-(*
-EVAL “final_tbl [([False], 0 , action "s")] 0” (*must fail *)
-EVAL “final_tbl [([True], 0 , action "s")] 0”
-EVAL “final_tbl [([False], 0 , action "s1");([True], 0 , action "s2")] 0”
-EVAL “final_tbl [([Var "a"], 0 , action "s1");([True], 1 , action "s2")] 1”
-EVAL “final_tbl [([Var "a"], 0 , action "s1");([True], 0 , action "s2")] 0” (* must fail *)  
-*)
-        
-        
+
+
 Definition final_tbll_def:
   final_tbll ([]: 'a var_table_list) st_in = NONE ∧
   final_tbll [tbl] st_in =
@@ -336,68 +168,19 @@ Definition final_tbll_def:
 End
 
 
-
 Definition final_tables_def:
   final_tables (tbll, st_in) =
   final_tbll tbll st_in
 End
 
-        
-(*
-     
-EVAL “final_tbll [[([False],0,state 2); ([False],0,state 3); ([True],0,state 3)];
-                  [([True],3,state 4); ([False],3,state 5); ([True],2,state 2)];
-                  [([True],2,action ("fwd",[1])); ([True],4,action ("fwd",[2]));
-               ([True],5,action ("drop",[]))]] 0 ”
-
-EVAL “final_tbll [[([False],0,state 2); ([False],0,state 3); ([False],0,state 3)];
-                  [([True],3,state 4); ([False],3,state 5); ([True],2,state 2)];
-                  [([True],2,action ("fwd",[1])); ([True],4,action ("fwd",[2]));
-               ([True],5,action ("drop",[]))]] 0 ”
-*)
-
-(*  free variables tables *)
-
-        
-Definition fv_row_def:
-  fv_row atoml =
-  let fv_in_row = MAP (\atom. fv_atom atom) atoml in
-    nub(FLAT fv_in_row)
-End
 
 
-Definition fv_tbl_def:
-  fv_tbl (tbl: 'a var_table) =
-  (let fv_in_tbl = MAP(\(atom,st_num,res). fv_row atom) tbl in
-      nub (FLAT fv_in_tbl))
-End
-        
-        
-
-    
-Definition fv_tbll_def:
-  fv_tbll (tbll: 'a var_table_list) =
-  let fv_in_tbll = MAP (\tbl. fv_tbl tbl) tbll in
-    nub(FLAT fv_in_tbll)
-End
-
-
-        
-Definition fv_tables_def:
-  fv_tables (tbll, st_in) =
-  fv_tbll tbll
-End
-
-
-
-        
-                                                                 
 Definition table_structure_def:
   table_structure =
   <|
     sem := sem_tables;
     sub := mk_substitute_tables;
-    simp := simp_tables;
+    simp := simp_tables_wrapper;
     final := final_tables;
     fv := fv_tables;
   |>
@@ -405,527 +188,2048 @@ End
 
 
 
-
-
-
-
-
-        
-
-               
-
-               
-Theorem fv_mem_tbll_thm:
-  ∀ tbll tbl mv.
-    (∀x. MEM x (fv_tbll (tbl::tbll)) ⇒ ∃b. ALOOKUP mv x = SOME b) ⇒
-    (∀x. MEM x (fv_tbll  tbll) ⇒ ∃b. ALOOKUP mv x = SOME b)
+Triviality simp_row_not_empty:
+  ∀ atoms.
+    simp_row atoms = [] ⇔ atoms = []
 Proof
-  gvs[fv_tbll_def]
-QED
-
-        
-Theorem fv_mem_tbll_hd_thm:
-  ∀ tbll tbl mv.
-    (∀x. MEM x (fv_tbll (tbl::tbll)) ⇒ ∃b. ALOOKUP mv x = SOME b) ⇒
-    (∀x. MEM x (fv_tbl  tbl) ⇒ ∃b. ALOOKUP mv x = SOME b)
-Proof
-  gvs[fv_tbll_def, fv_tbl_def]
-QED
-        
-
-Theorem fv_mem_tbl_thm:
-  ∀ tbl h mv.
-    (∀x. MEM x (fv_tbl (h::tbl)) ⇒ ∃b. ALOOKUP mv x = SOME b) ⇒
-    (∀x. MEM x (fv_tbl  tbl) ⇒ ∃b. ALOOKUP mv x = SOME b)
-Proof
-  gvs[fv_tbl_def]
-QED
-
-
-Theorem fv_mem_tbl_h_thm:
-  ∀ tbl h mv.
-    (∀x. MEM x (fv_tbl (h::tbl)) ⇒ ∃b. ALOOKUP mv x = SOME b) ⇒
-    (∀x. MEM x (fv_tbl  [h]) ⇒ ∃b. ALOOKUP mv x = SOME b)
-Proof
-  gvs[fv_tbl_def]
-QED        
-
-
-
-Theorem fv_mem_row_thm:
-  ∀ atoml h mv.
-    (∀x. MEM x (fv_row (h::atoml)) ⇒ ∃b. ALOOKUP mv x = SOME b) ⇒
-    (∀x. MEM x (fv_row atoml) ⇒ ∃b. ALOOKUP mv x = SOME b)
-Proof
-  gvs[fv_row_def]
-QED 
-
-
-
-Theorem fv_mem_row_h_thm:
-  ∀ atoml h mv.
-    (∀x. MEM x (fv_row (h::atoml)) ⇒ ∃b. ALOOKUP mv x = SOME b) ⇒
-    (∀x. MEM x (fv_row [h]) ⇒ ∃b. ALOOKUP mv x = SOME b)
-Proof
-  gvs[fv_row_def]
-QED
-
-(*
-Theorem fv_mem_atom_not_thm:        
-  ∀ atom mv.
-    (∀x. MEM x (fv_row [Not atom]) ⇒ ∃b. ALOOKUP mv x = SOME b) ⇒
-    (∀x. MEM x (fv_row [atom]) ⇒ ∃b. ALOOKUP mv x = SOME b)
-Proof     
-  gvs[fv_row_def, fv_atom_def]
-QED
-*)
-
-          
-Theorem mk_substitute_tbl_normalize1:
-  ∀h rows x b.
-       mk_substitute_tbl (h::rows) x b =
-       mk_substitute_tbl [h] x b ⧺ mk_substitute_tbl rows x b
-Proof
-  gvs[mk_substitute_tbl_def]
-QED
-
-
-Theorem mk_substitute_tbl_normalize2:
-  ∀atoml st_num res rows x b.
-       mk_substitute_tbl ((atoml,st_num,res)::rows) x b =
-       (mk_substitute_row atoml x b,st_num,res)::mk_substitute_tbl rows x b
-Proof
-  gvs[mk_substitute_tbl_def]
-QED
-
-
-Theorem simp_tbl_normalize1:
-  ∀atoml st_num res rows x b.
-       simp_tbl ((atoml,st_num,res)::rows) =
-       (simp_row atoml,st_num,res)::simp_tbl rows
-Proof
-  gvs[simp_tbl_def]
-QED
-
-
-        
-Theorem sub_then_simp_answer_indeed_in_fv:
-  ∀ atom h' b s.                      
-    (simp_atom (mk_substitute_atom atom h' b) = Var s) ⇒
-    MEM s (fv_atom atom)
-Proof
-  Cases >>
-  rpt strip_tac >>
-  gvs[fv_atom_def, mk_substitute_atom_def, simp_atom_def] >>
-  rpt (BasicProvers.FULL_CASE_TAC >> gvs[]) >>
-  gvs[fv_atom_def, mk_substitute_atom_def, simp_atom_def] 
-QED
-
-
-Triviality mem_fv_sub_simp_tbl_triv1:
-  ∀ atom h' b x.        
-    MEM x (fv_atom (simp_atom (mk_substitute_atom atom h' b))) ⇒
-    MEM x (fv_atom atom)
-Proof
-  Cases >>
-  rpt strip_tac >>
-  gvs[fv_atom_def, mk_substitute_atom_def, simp_atom_def] >>
-  rpt (BasicProvers.FULL_CASE_TAC >> gvs[]) >>
-  gvs[fv_atom_def, mk_substitute_atom_def, simp_atom_def] 
-QED
-             
-      
-
-Theorem mem_imp_sem_tbl:
-  ∀ atom mv.
-    (∀x. MEM x (fv_atom atom) ⇒ ∃b. ALOOKUP mv x = SOME b) ⇒
-    sem_var_atom atom mv ≠ NONE ∧ ∃ b' . sem_var_atom atom mv = SOME b'
-Proof
-  Cases >>
-  rw[fv_atom_def] >> gvs[AllCaseEqs()] >>
-  gvs[sem_var_atom_def, simp_atom_def] >>
+  rw[simp_row_def] >>
   rpt (BasicProvers.FULL_CASE_TAC >> gvs[]) 
 QED
 
 
-Triviality non_empty_line_simp_not_empty:
-  ∀ atoml h' b.
-    atoml ≠ [] ⇔  simp_row (mk_substitute_row atoml h' b) ≠ []
-Proof
-  Induct >> gvs[mk_substitute_row_def, simp_row_def] >>
-  rpt strip_tac >>
-  rpt (BasicProvers.FULL_CASE_TAC >> gvs[])
-QED
 
 
 
-Theorem lookup_implies_sem_var_atoms_same:
-  ∀ atom h' b bool mv.
-    ALOOKUP mv h' = SOME b  ⇒
-    (sem_var_atom atom mv = SOME bool ⇔ sem_var_atom (simp_atom (mk_substitute_atom atom h' b)) mv = SOME bool)
-Proof
-  Cases >>
-  rpt strip_tac >>
-  rpt (gvs[mk_substitute_atom_def, simp_atom_def, sem_var_atom_def] >>
-       BasicProvers.FULL_CASE_TAC >>
-       res_tac >>               
-       gvs[])
-QED
 
-
-
-Theorem sem_var_atom_failure_from_simp_atom_false:        
-  ∀ atoml h' b mv.
-    atoml ≠ [] ∧
-    ALOOKUP mv h' = SOME b ∧
-    MEM False (MAP (λatom. simp_atom atom) (MAP (λatom. mk_substitute_atom atom h' b) atoml)) ⇒
-    ~ EVERY (λminipred. sem_var_atom minipred mv = SOME T) atoml
+Theorem simp_row_sub_false_head:
+  ∀ atoms_list x b.
+    (simp_row (mk_substitute_row (True::atoms_list) x b) = [False] ⇒
+     simp_row (mk_substitute_row (atoms_list) x b) = [False]) ∧
+    (simp_row (mk_substitute_row (NotFalse::atoms_list) x b) = [False] ⇒
+     simp_row (mk_substitute_row (atoms_list) x b) = [False])
+    
 Proof
   Induct >>
-  rpt strip_tac >> gvs[] >>
-  imp_res_tac lookup_implies_sem_var_atoms_same >> gvs[sem_var_atom_def] >>
-  res_tac >>
-  Cases_on ‘atoml = []’ >> gvs[] >>
-  imp_res_tac NOT_EVERY
-QED
-
-        
-
-Theorem subst_simp_sound_for_atom:
-  ∀atom h' b mv.
-    ALOOKUP mv h' = SOME b ⇒
-    (simp_atom (mk_substitute_atom atom h' b) = True ⇒
-     sem_var_atom atom mv = SOME T) ∧
-    (simp_atom (mk_substitute_atom atom h' b) = False ⇒
-     sem_var_atom atom mv = SOME F)
-Proof                                   
-  Cases >>
-  gvs[simp_atom_def, mk_substitute_atom_def, sem_var_atom_def] >>
-  rpt strip_tac >>
-  rpt (BasicProvers.FULL_CASE_TAC >> gvs[simp_atom_def, mk_substitute_atom_def, sem_var_atom_def])
+  rw[mk_substitute_row_def, simp_row_def] >>
+  gvs[mk_substitute_atom_def, simp_atom_def, is_not_true_var_atom_def]
 QED
 
 
-       
 
-Theorem lookup_implies_sem_var_atoml_same2:
-  ∀ atoml h' b mv.
-    ALOOKUP mv h' = SOME b ∧
-    atoml ≠ [] ∧
-    EVERY ((λminipred. sem_var_atom minipred mv = SOME T)) (simp_row (mk_substitute_row atoml h' b)) ⇒
-    EVERY (λminipred. sem_var_atom minipred mv = SOME T) atoml
+Theorem simp_row_sub_false_var_head:
+  ∀ atoms_list mv x s b.
+    (ALOOKUP mv s = SOME T ∧
+    ALOOKUP mv x = SOME b ∧
+    simp_row (mk_substitute_row (Var s::atoms_list) x b) = [False] ⇒
+     simp_row (mk_substitute_row atoms_list x b) = [False]) ∧
+
+    (ALOOKUP mv s = SOME F ∧
+     ALOOKUP mv x = SOME b ∧
+     simp_row (mk_substitute_row (Not s::atoms_list) x b) = [False] ⇒
+     simp_row (mk_substitute_row atoms_list x b) = [False]) 
 Proof
   Induct >>
-  rpt strip_tac >> 
-  gvs[mk_substitute_row_def, simp_row_def] >>
-
+  rw[mk_substitute_row_def, simp_row_def] >>
+  gvs[mk_substitute_atom_def, simp_atom_def, is_not_true_var_atom_def] >>
   rpt (BasicProvers.FULL_CASE_TAC >> gvs[]) >>
-  gvs[sem_var_atom_def] >>
-                             
-  imp_res_tac lookup_implies_sem_var_atoms_same >> gvs[] >> res_tac >>
-  gvs[] >>
-  Cases_on ‘atoml = []’ >> gvs[]
+  gvs[mk_substitute_atom_def, simp_atom_def, is_not_true_var_atom_def]
 QED
 
 
 
 
 
-          
-Theorem simp_sub_mem_normalization:
-  ∀ atoml h h' b atom.        
-    atom ≠ simp_atom (mk_substitute_atom h h' b) ∧
-    MEM atom (simp_row (mk_substitute_row (h::atoml) h' b)) ⇒
-    MEM atom (simp_row (mk_substitute_row atoml h' b))
+Theorem simp_sub_row_false_then_atoms_sem_false:
+  ∀ atoms_list x b mv.
+    ALOOKUP mv x = SOME b ∧
+    simp_row (mk_substitute_row atoms_list x b) = [False] ⇒
+    ~ is_atoml_true atoms_list mv
 Proof
-  rpt strip_tac >>
-  gvs[mk_substitute_row_def, simp_row_def] >>
-  rpt (BasicProvers.FULL_CASE_TAC >> gvs[]) >>
-  gvs[MEM_MAP] >> metis_tac[]
-QED
-
-
-         
-        
-
-Theorem is_match_row_substitute_preserve1:
-  ∀ atoml mv h' b s_in st_num.        
-    ALOOKUP mv h' = SOME b ∧
-    is_match_row s_in st_num atoml mv ⇒
-    is_match_row s_in st_num (simp_row (mk_substitute_row atoml h' b)) mv
-Proof
-  Induct >>
-  gvs[is_match_row_def] >>
-  rpt strip_tac >>
-  gvs[is_atoml_true_def] >>
   
-  Cases_on ‘atoml = []’ >> gvs[] >|[
-    simp[mk_substitute_row_def, simp_row_def] >>
-    rpt (BasicProvers.FULL_CASE_TAC >> gvs[sem_var_atom_def]) >>
-    imp_res_tac subst_simp_sound_for_atom >> gvs[] >>
-    imp_res_tac lookup_implies_sem_var_atoms_same >> gvs[]
-    ,
-    res_tac >>
-    rgs[] >>
-    gvs[Once EVERY_NOT_EXISTS] >>
-    gvs[EVERY_MEM] >>
-    gvs[EVERY_MAP] >>
-    rpt strip_tac >>
+  Induct >-
+   rw[mk_substitute_row_def, simp_row_def, is_atoml_true_def] >>
+  
+  rw[] >>
+  Cases_on ‘h’ >>
+  
+  (imp_res_tac simp_row_sub_false_head >>
+   res_tac >>
+   gvs[is_atoml_true_def] >>
+   gvs[sem_var_atom_def]) >>
+  
+  strip_tac >>
+  rpt (BasicProvers.FULL_CASE_TAC >> gvs[]) >>
+  imp_res_tac simp_row_sub_false_var_head  >>
+  gvs[]
+QED
     
-    Cases_on ‘minipred = simp_atom(mk_substitute_atom h h' b)’ >> gvs[] >>
-    res_tac >|[
-        imp_res_tac lookup_implies_sem_var_atoms_same >> gvs[]
-        ,
-        imp_res_tac simp_sub_mem_normalization >>
-        res_tac
-      ]   
+
+        
+
+Theorem simp_sub_empty_then_min_index_none:
+  ∀ t x b s_in mv.
+    ALOOKUP mv x = SOME b ∧
+    simp_table (mk_substitute_tbl t x b) (SOME s_in) = [] ⇒
+    min_idx_till (check_all_rows_match s_in t mv) T = NONE
+Proof
+
+  Induct >> rw[] >|[
+    rw[mk_substitute_tbl_def, simp_table_def] >>
+    gvs[check_all_rows_match_def, min_idx_till_def, INDEX_FIND_def]
     ,
     
-    gvs[mk_substitute_row_def, simp_row_def] >>
-    rpt (BasicProvers.FULL_CASE_TAC >> gvs[])
-    ,
-                                
-    res_tac >>
-    rgs[] >>
-    gvs[mk_substitute_row_def, simp_row_def] >>
-    rpt (BasicProvers.FULL_CASE_TAC >> gvs[])
+    PairCases_on ‘h’ >>
+    rename1 ‘((atoms_list,st,res)::t)’ >>
+    gvs[Once mk_substitute_tbl_normalize2] >>
+    gvs[check_all_rows_match_def, is_match_row_def] >>
+    rgs[simp_table_def] >>
+    
+    
+    rpt (BasicProvers.FULL_CASE_TAC >> gvs[]) >>
+        
+    (res_tac >>
+     rgs[min_idx_till_def] >>
+     gvs[INDEX_FIND_NONE_EXISTS]) >>
+    
+    imp_res_tac simp_sub_row_false_then_atoms_sem_false >>
+    fs[]          
   ]
 QED
 
 
 
-Theorem is_match_row_substitute_preserve2:
-  ∀ atoml mv h' b s_in st_num.        
-    ALOOKUP mv h' = SOME b ∧
-    is_match_row s_in st_num (simp_row (mk_substitute_row atoml h' b)) mv ⇒
-    is_match_row s_in st_num atoml mv
+        
+
+Triviality mk_substitute_row_empty:
+  ∀ atoms_list x b.
+    mk_substitute_row atoms_list x b = [] ⇒
+    atoms_list = []
+Proof
+  Induct >> gvs[mk_substitute_row_def]
+QED
+
+
+        
+Triviality simp_table_mk_substitute_tbl_empty1:
+  ∀ t h x b s_in.
+    simp_table (mk_substitute_tbl (h::t) x b) (SOME s_in) = [] ⇒
+    simp_table (mk_substitute_tbl t x b) (SOME s_in) = []
+Proof
+  rw[mk_substitute_tbl_def, simp_table_def] >>
+  PairCases_on ‘h’ >>
+  gvs[simp_table_def] >>
+  rpt (BasicProvers.FULL_CASE_TAC >> gvs[]) 
+QED
+
+        
+        
+Theorem simp_table_sub_every_prop1:
+  ∀ t x b  s_in mv.
+    ALOOKUP mv x = SOME b ∧
+    simp_table (mk_substitute_tbl t x b) (SOME s_in) = [] ⇒
+    EVERY ($¬ ∘ (λ(p,a). p)) (MAP
+                              (λ(atoml,st_num,res'). (s_in = st_num ∧ is_atoml_true atoml mv ∧ atoml ≠ [],res')) t)
+Proof
+  
+  Induct >>
+  rw[] >|[
+    PairCases_on ‘h’ >> gvs[] >>
+    rpt strip_tac >>
+    Cases_on ‘h0’ >> gvs[mk_substitute_tbl_def, simp_table_def] >>
+    rpt (BasicProvers.FULL_CASE_TAC >> gvs[]) >>
+    imp_res_tac simp_sub_row_false_then_atoms_sem_false
+    ,
+    imp_res_tac simp_table_mk_substitute_tbl_empty1 >>
+    res_tac >>
+    gvs[]
+  ]
+QED 
+        
+               
+               
+        
+Theorem simp_sub_empty_then_min_index_tbl_none:
+∀ t x b s_in mv s_num res.
+  ALOOKUP mv x = SOME b ∧
+  simp_table (mk_substitute_tbl t x b) (SOME s_in) = [([],s_num,res)] ⇒
+  min_idx_till (check_all_rows_match s_in t mv) T = NONE
+Proof
+
+  Induct >> rw[] >|[
+    gvs[check_all_rows_match_def, min_idx_till_def, INDEX_FIND_def]
+    ,
+    
+    PairCases_on ‘h’ >>
+    rename1 ‘((atoms_list,st,result)::t)’ >>
+    gvs[Once mk_substitute_tbl_normalize2] >>
+    gvs[check_all_rows_match_def, is_match_row_def] >>
+    rgs[simp_table_def] >>
+    
+    
+    rpt (BasicProvers.FULL_CASE_TAC >> gvs[]) >>
+        
+    (res_tac >>
+     rgs[min_idx_till_def] >>
+     gvs[INDEX_FIND_NONE_EXISTS]) >>
+    
+    imp_res_tac simp_sub_row_false_then_atoms_sem_false >>
+    fs[] >>
+
+
+    imp_res_tac simp_row_not_empty >> gvs[] >>
+    imp_res_tac mk_substitute_row_empty >> gvs[] >>        
+    imp_res_tac simp_table_sub_every_prop1
+  ]
+QED
+
+
+
+        
+
+                             
+Theorem match_tbll_head_empty:
+  ∀ tbll mv s_in.
+    match_tbll ([]::tbll) mv s_in = NONE
+Proof
+  rw[] >> Cases_on ‘tbll’ >> 
+  gvs[match_tbll_def, match_tbl_def, check_all_rows_match_def, min_idx_till_def, INDEX_FIND_def]
+QED
+
+
+Theorem match_tbll_row_empty:
+  ∀ tbll st res mv s_in.
+    match_tbll ([([],st,res)]::tbll) mv s_in = NONE
+Proof
+ rw[] >> Cases_on ‘tbll’ >> 
+ gvs[match_tbll_def, match_tbl_def, check_all_rows_match_def, min_idx_till_def, INDEX_FIND_def, is_match_row_def]
+QED
+
+
+
+Theorem match_tbll_final_before_ending_none:
+  ∀ tbll st mv s_in a.
+    tbll ≠ [] ⇒
+    match_tbll ([([True],st,action a)]::tbll) mv s_in = NONE
+Proof
+  rw[] >> Cases_on ‘tbll’ >> 
+  gvs[match_tbll_def, match_tbl_def, check_all_rows_match_def, min_idx_till_def,
+      INDEX_FIND_def, is_match_row_def, is_atoml_true_def, sem_var_atom_def] >>
+  rpt (BasicProvers.FULL_CASE_TAC >> gvs[])
+QED
+
+
+
+
+
+        
+Triviality simp_tables_sub_not_empty_table:
+ ∀ t x b l.
+  simp_tables (mk_substitute_tbl t x b::l) NONE ≠ []
+Proof
+
+rw[simp_tables_def, mk_substitute_tbl_def] >>
+  rpt (BasicProvers.FULL_CASE_TAC >> gvs[])
+QED
+
+
+
+Triviality simp_table_impossible_case1:
+  ∀ atoml h s_in t t' st_num res st_num' res'.
+    simp_table [(atoml, st_num, res)] (SOME s_in) ≠ [(True::t::t',st_num',res')]
+Proof
+  Induct_on ‘atoml’ >> 
+  gvs[simp_table_def] >> rpt strip_tac >>
+  rpt (BasicProvers.FULL_CASE_TAC >> gvs[simp_row_def]) >>
+  rw[] >>
+  gvs[is_not_true_var_atom_def]
+QED   
+
+      
+Theorem filtering_not_true_then_not_mem:
+  ∀ atoml filtered_list.
+    FILTER (λx. is_not_true_var_atom x) (MAP (λatom. simp_atom atom) atoml) = filtered_list ⇒
+    ¬ MEM True filtered_list ∧ ¬ MEM NotTrue filtered_list ∧ ¬ MEM NotFalse filtered_list
 Proof
   Induct >>
-  gvs[is_match_row_def] >>
-  rpt strip_tac >>
-  gvs[is_atoml_true_def] >>
+  rw[is_not_true_var_atom_def] >>
+  Cases_on ‘h’ >>
+  gvs[simp_atom_def, is_not_true_var_atom_def]
+QED
+
+
+
+                   
+
+Theorem filtering_not_true_then_notTrue_notFalse_mem:
+  ∀ atoml filtered_list x b.
+    FILTER (λx. is_not_true_var_atom x) (MAP (λatom. simp_atom atom) (mk_substitute_row atoml x b)) =
+    filtered_list ⇒
+    (¬ MEM NotTrue filtered_list ∧ ¬ MEM NotFalse filtered_list) 
+Proof
+  Induct_on ‘atoml’ >>
+  rw[mk_substitute_row_def, simp_atom_def, is_not_true_var_atom_def] >>
   (
-  imp_res_tac lookup_implies_sem_var_atoml_same2 >> 
-  gvs[mk_substitute_row_def, simp_row_def] 
+    Cases_on ‘h’ >> gvs[mk_substitute_atom_def, simp_atom_def, is_not_true_var_atom_def] >>
+    gvs[mk_substitute_row_def] >>
+    rpt (BasicProvers.FULL_CASE_TAC >> gvs[simp_atom_def])
   )
 QED
 
+        
 
+        
 
-Theorem is_match_row_substitute_preserve:
-  ∀ atoml mv h' b (s_in:num) st_num.        
-    ALOOKUP mv h' = SOME b ⇒
-    (is_match_row s_in st_num (simp_row (mk_substitute_row atoml h' b)) mv =
-    is_match_row s_in st_num atoml mv)
-Proof
-  rpt strip_tac >>
-  EQ_TAC >>
-  metis_tac[is_match_row_substitute_preserve1, is_match_row_substitute_preserve2]
+Theorem simp_table_impossible_case2:
+  ∀ l t t' s_in st_num res.        
+    (simp_table l (SOME s_in) ≠ [(True::t::t',st_num,res)]) ∧
+    (simp_table l (SOME s_in) ≠ [(False::t',st_num,res)])
+Proof                 
+  Induct_on ‘l’ >>
+  rw[] >>
+  gvs[simp_table_def] >>
+  Cases_on ‘l’ >>
+  PairCases_on ‘h’ >>
+  gvs[simp_table_impossible_case1] >>
+  gvs[simp_table_def] >>
+  rpt (BasicProvers.FULL_CASE_TAC >> gvs[simp_row_def]) >>
+  rw[] >>
+  gvs[is_not_true_var_atom_def] >>
+  imp_res_tac filtering_not_true_then_not_mem >>
+  gvs[]
 QED
 
 
 
-Theorem exists_is_match_row_after_subst_simp:        
-  ∀ tbl s_in h' b mv.
-    ALOOKUP mv h' = SOME b ∧
-    EXISTS (λ(p,a). p) (MAP (λ(atoml,st_num,res). (is_match_row s_in st_num atoml mv,res)) tbl) ⇒
-    EXISTS (λ(p,a). p) (MAP (λ(atoml,st_num,res). (is_match_row s_in st_num atoml mv,res))
-                            (simp_tbl (mk_substitute_tbl tbl h' b)))
+Theorem simp_table_impossible_case3:
+∀ l t t' s_in st_num res mv x b.
+  (simp_table (mk_substitute_tbl t x b) (SOME s_in) ≠ [(NotTrue::t',st_num,res)]) ∧
+  (simp_table (mk_substitute_tbl t x b) (SOME s_in) ≠ [(NotFalse::t',st_num,res)])                 
 Proof
-  Induct >-
-   gvs[mk_substitute_tbl_def, simp_tbl_def] >>
-  rpt strip_tac >>
-  simp[mk_substitute_tbl_def, simp_tbl_def] >>
-  gvs[] >|[
+  Induct_on ‘t’ >>
+  rw[] >>
+  gvs[simp_table_def, mk_substitute_tbl_def] >>
+  PairCases_on ‘h’ >>
+  gvs[simp_table_def] >>
+  rpt (BasicProvers.FULL_CASE_TAC >> gvs[simp_row_def]) >>
+  rw[] >>
+  imp_res_tac filtering_not_true_then_not_mem >>
+  gvs[] >>
+  res_tac >>
+  gvs[] >>
+  imp_res_tac filtering_not_true_then_notTrue_notFalse_mem >> gvs[]
+QED
+
+
+(*        
+Theorem simp_tbl_none_impies_some_cases:
+∀ tbl n h1 h2.
+  (simp_table (tbl) NONE = [] ⇒ simp_table (tbl) (SOME n) = []) ∧
+  (simp_table (tbl) NONE = [([],h1,h2)] ⇒ simp_table (tbl) (SOME n) = [([],h1,h2)])
+Proof
+
+Induct >>
+rw[simp_table_def] >>
+
+Cases_on ‘tbl’ >> PairCases_on ‘h’ >> gvs[simp_table_def]  >>       
+rpt (BasicProvers.FULL_CASE_TAC >> gvs[simp_row_def])
+QED  
+*)
+
+
+    
+Theorem simp_table_return_true_then_rows_none:
+  ∀ tbl rows h1 h2.
+    simp_table tbl NONE = [(True::rows,h1,h2)] ⇒
+    rows = []
+Proof
   
-    PairCases_on ‘h’ >>
-    rename1 ‘(atoml, st_num, res)’ >>
-    gvs[MAP_MAP_o] >>
-    gvs[EXISTS_MAP] >>
-    imp_res_tac is_match_row_substitute_preserve1 >> gvs[]
-    ,
-    res_tac >>
-    gvs[mk_substitute_tbl_def, simp_tbl_def]
-  ]    
-QED
-
-
-Theorem exists_is_match_row_before_subst_simp:        
-  ∀ tbl s_in h' b mv.
-    ALOOKUP mv h' = SOME b ∧
-    EXISTS (λ(p,a). p) (MAP (λ(atoml,st_num,res). (is_match_row s_in st_num atoml mv,res))
-                            (simp_tbl (mk_substitute_tbl tbl h' b))) ⇒
-    EXISTS (λ(p,a). p) (MAP (λ(atoml,st_num,res). (is_match_row s_in st_num atoml mv,res)) tbl)
-Proof
-  Induct >-
-   gvs[mk_substitute_tbl_def, simp_tbl_def] >>
-  rpt strip_tac >>
-  gvs[mk_substitute_tbl_def, simp_tbl_def] >>
-  gvs[] >|[
+  Induct >>
+  rw[simp_table_def] >>
   
-    PairCases_on ‘h’ >>
-    rename1 ‘(atoml, st_num, res)’ >>
-    gvs[MAP_MAP_o] >>
-    gvs[EXISTS_MAP] >>
-    imp_res_tac is_match_row_substitute_preserve2 >> gvs[]
-    ,
-    res_tac >>
-    gvs[mk_substitute_tbl_def, simp_tbl_def]
-  ]    
+  Cases_on ‘tbl’ >> PairCases_on ‘h’ >> gvs[simp_table_def]  >>       
+  rpt (BasicProvers.FULL_CASE_TAC >> gvs[simp_row_def]) >>
+  imp_res_tac filtering_not_true_then_not_mem >>
+  gvs[]
+QED          
+
+
+
+
+Triviality length_of_simp_single_table:
+ ∀rows anyop.
+   LENGTH (simp_tables [rows] anyop) ≤ 1
+Proof
+Induct >> rw[simp_tables_def] >>
+rpt (BasicProvers.FULL_CASE_TAC >> gvs[simp_row_def]) 
+QED
+                                                
+
+Triviality simp_tables_single_not_empty:
+∀ rows anyop.
+simp_tables [rows] anyop ≠ []
+Proof
+  rw[simp_tables_def] >>
+  rpt (BasicProvers.FULL_CASE_TAC >> gvs[simp_row_def]) 
+QED
+                                                
+
+
+Triviality simp_table_none_append:
+  ∀ rows h.
+    simp_table (h::rows) NONE = (simp_table [h] NONE)++(simp_table rows NONE)
+Proof
+  rw[] >> PairCases_on ‘h’ >>
+  rw[simp_table_def] >>
+  rpt (BasicProvers.FULL_CASE_TAC >> gvs[simp_row_def]) 
 QED
 
 
 
 
-Theorem is_match_row_lists_subst_simp_eq:        
-∀tbl h' b mv s_in.
-       ALOOKUP mv h' = SOME b ⇒
-       MAP (λ(atoml,st_num,res). (is_match_row s_in st_num atoml mv,res))
-         (simp_tbl (mk_substitute_tbl tbl h' b)) =
-       MAP (λ(atoml,st_num,res). (is_match_row s_in st_num atoml mv,res)) tbl 
+Theorem min_idx_till_none_eq_res:
+  ∀ l1 l2 res.
+    min_idx_till l1 T = min_idx_till l2 T ⇒
+    (min_idx_till ((F,res)::l1) T = NONE) = (min_idx_till l2 T = NONE)
+Proof
+
+  rw[min_idx_till_def] >>
+  gvs[INDEX_FIND_def] >>
+  Cases_on ‘INDEX_FIND 0 (λ(p,a). p) l1’ >> 
+  gvs[P_NONE_hold] >>
+                   
+  Cases_on ‘INDEX_FIND 0 (λ(p,a). p) l2’ >> gvs[] >>
+  Cases_on ‘INDEX_FIND 1 (λ(p,a). p) l1’ >> gvs[] >>
+  imp_res_tac P_NONE_hold2 >>
+  gvs[]
+QED
+
+
+
+Theorem min_idx_till_some_eq_res:     
+  ∀ l1 l2 res.
+    min_idx_till l1 T = min_idx_till l2 T ⇒
+    ∃ n m res' . (min_idx_till ((F,res)::l1) T = SOME (n,res')) =
+                 (min_idx_till            l2 T = SOME (m,res'))
+Proof
+
+  rw[min_idx_till_def] >>
+  gvs[INDEX_FIND_def] >>
+  Cases_on ‘INDEX_FIND 0 (λ(p,a). p) l1’ >> gvs[] >>
+  
+  gvs[P_NONE_hold] >>
+  
+  Cases_on ‘INDEX_FIND 0 (λ(p,a). p) l2’ >> gvs[] >>
+  Cases_on ‘INDEX_FIND 1 (λ(p,a). p) l1’ >> gvs[] >>
+  imp_res_tac P_NONE_hold2 >>
+  gvs[] >>
+  
+  Cases_on ‘x’ >> Cases_on ‘x'’ >>
+  imp_res_tac P_implies_next >>
+  gvs[] >>
+  qexistsl_tac [‘SUC q’, ‘q’, ‘r’] >>
+  gvs[] 
+QED
+
+
+
+
+
+Theorem INDEX_FIND_some_eq_next: 
+  ∀ l1 res n.
+  INDEX_FIND 0 (λ(p,a). p) l1 = SOME (n,res) ⇔ INDEX_FIND 1 (λ(p,a). p) l1 = SOME (n + 1,res)
+Proof
+  rw[] >>
+  Cases_on ‘INDEX_FIND 0 (λ(p,a). p) l1’ >>
+  gvs[P_NONE_hold] >>
+  
+  Cases_on ‘x’ >> gvs[] >>
+  imp_res_tac P_implies_next >>
+  gvs[ADD1]
+QED
+
+
+        
+Theorem min_idx_till_some_eq_next: 
+  ∀ l1 res res' n.
+  (min_idx_till l1 T = SOME (n,res)) ⇔  (min_idx_till ((F,res')::l1) T = SOME (n+1,res))
+Proof
+  rw[min_idx_till_def, INDEX_FIND_def] >>
+  gvs[INDEX_FIND_some_eq_next]
+QED
+
+
+
+Theorem INDEX_FIND_some_eq_next2: 
+  ∀ l1 res n.
+  (INDEX_FIND 0 (λ(p,a). p) l1 = SOME (n -1,res) ∧ n>0) ⇔ INDEX_FIND 1 (λ(p,a). p) l1 = SOME (n,res)
+Proof
+  rw[] >>
+  Cases_on ‘INDEX_FIND 0 (λ(p,a). p) l1’ >>
+  gvs[P_NONE_hold] >>
+  
+  Cases_on ‘x’ >> gvs[] >>
+  imp_res_tac P_implies_next >>
+  gvs[ADD1] >>
+  
+  Cases_on ‘n’ >> gvs[ADD1]   
+QED
+
+    
+        
+Theorem min_idx_till_some_eq_next2: 
+  ∀ l1 res res' n.
+  (min_idx_till l1 T = SOME (n-1,res) ∧ n>0) ⇔ (min_idx_till ((F,res')::l1) T = SOME (n,res))
+Proof
+  rw[min_idx_till_def, INDEX_FIND_def] >>
+  gvs[INDEX_FIND_some_eq_next] >>
+  Cases_on ‘INDEX_FIND 1 (λ(p,a). p) l1’ >> gvs[] >>
+  Cases_on ‘x’ >> gvs[] >>
+  imp_res_tac INDEX_FIND_some_eq_next2 >>
+   Cases_on ‘n’ >> gvs[ADD1] 
+QED
+
+
+
+        
+
+Triviality simp_row_false_emptyl:
+  ∀ atoml t.        
+    simp_row atoml = False::t ⇒
+    simp_row atoml = [False]
+Proof
+  rw[simp_row_def] >>
+  rpt (BasicProvers.FULL_CASE_TAC >> gvs[]) 
+QED
+
+
+      
+Theorem min_idx_check_rows_simp_tbl_none:
+  ∀ rows st_in simp_rows simp_rows' mv.
+    simp_table rows NONE = simp_rows ∧
+    simp_table rows (SOME st_in) = simp_rows' ⇒
+    (min_idx_till (check_all_rows_match st_in simp_rows mv) T = NONE) =
+    (min_idx_till (check_all_rows_match st_in simp_rows' mv) T = NONE)
+Proof
+
+  Induct_on ‘rows’ >>
+  rpt strip_tac >-
+   rgs[simp_table_def] >>
+  
+  PairCases_on ‘h’ >>
+  rename1 ‘simp_table ((atoms,st,res)::rows) (SOME st_in)’ >>
+  rgs[simp_table_def] >>
+  Cases_on ‘simp_row atoms’ >> gvs[] >|[
+    Cases_on ‘st_in ≠ st’ >>
+    gvs[] >|[
+      gvs[check_all_rows_match_def] >>
+      simp[Once is_match_row_def] >>
+      metis_tac[min_idx_till_none_eq_res]
+      ,
+      gvs[check_all_rows_match_def] >>
+      gvs[is_match_row_def, min_idx_till_def] >>
+      gvs[INDEX_FIND_def, index_none_not_every]
+    ]
+    ,
+
+    Cases_on ‘st_in ≠ st’ >>
+    gvs[] >|[
+        Cases_on ‘h’ >> gvs[] >>
+        (
+        imp_res_tac simp_row_false_emptyl >>
+        gvs[] >>
+        gvs[check_all_rows_match_def] >>
+        simp[Once is_match_row_def] >>
+        metis_tac[min_idx_till_none_eq_res]
+        )
+        
+        ,
+        (* when st is the same as st_in*)
+        Cases_on ‘t’ >> gvs[] >|[
+            rpt (BasicProvers.FULL_CASE_TAC >> gvs[]) >>
+            (gvs[check_all_rows_match_def, is_match_row_def, is_atoml_true_def, sem_var_atom_def] >>
+             gvs[min_idx_till_def, INDEX_FIND_def, index_none_not_every])
+            ,
+            Cases_on ‘h’ >> gvs[] >>
+            (gvs[check_all_rows_match_def, is_match_row_def, is_atoml_true_def, sem_var_atom_def] >>
+             gvs[min_idx_till_def, INDEX_FIND_def, index_none_not_every]) 
+          ]                         
+      ]
+  ]
+QED
+
+
+
+
+
+
+(* TODO: refactor this proof *)         
+Theorem min_idx_check_rows_simp_tbl_some:
+  ∀ rows st_in simp_rows simp_rows' mv.
+    simp_table rows NONE = simp_rows ∧
+    simp_table rows (SOME st_in) = simp_rows' ⇒
+    ∃ m n res. (min_idx_till (check_all_rows_match st_in simp_rows mv) T = SOME (n, res)) =
+               (min_idx_till (check_all_rows_match st_in simp_rows' mv) T = SOME (m, res))
+Proof
+
+  Induct_on ‘rows’ >>
+  rpt strip_tac >-
+   rgs[simp_table_def, check_all_rows_match_def, min_idx_till_def, INDEX_FIND_def] >>
+  
+  PairCases_on ‘h’ >>
+  rename1 ‘simp_table ((atoms,st,res)::rows) (SOME st_in)’ >>
+  rgs[simp_table_def] >>
+  Cases_on ‘simp_row atoms’ >> gvs[] >|[
+           
+    Cases_on ‘st_in ≠ st’ >>
+    gvs[] >|[
+      gvs[check_all_rows_match_def] >>
+      simp[Once is_match_row_def] >>
+                
+      first_x_assum (strip_assume_tac o (Q.SPECL [‘st_in’, ‘mv’])) >>
+      qexistsl_tac [‘m’, ‘n+1’, ‘res'’] >>      
+      gvs[GSYM min_idx_till_some_eq_next]
+
+      ,
+      gvs[check_all_rows_match_def] >>
+      gvs[is_match_row_def] >>
+                            
+      first_x_assum (strip_assume_tac o (Q.SPECL [‘st’, ‘mv’])) >>
+      qexistsl_tac [‘m+1’, ‘n+1’, ‘res'’] >>      
+      gvs[GSYM min_idx_till_some_eq_next] 
+      
+    ]
+    ,
+
+    Cases_on ‘st_in ≠ st’ >>
+    gvs[] >|[
+        Cases_on ‘h’ >> gvs[] >>
+        (
+        imp_res_tac simp_row_false_emptyl >>
+        gvs[] >>
+        
+        
+        gvs[check_all_rows_match_def] >>
+        simp[Once is_match_row_def] >>
+        
+        first_x_assum (strip_assume_tac o (Q.SPECL [‘st_in’, ‘mv’])) >>
+        qexistsl_tac [‘m’, ‘n+1’, ‘res'’] >> 
+        gvs[GSYM min_idx_till_some_eq_next]
+        )
+        
+        ,
+        (* when st is the same as st_in*)
+        Cases_on ‘t’ >> gvs[] >|[
+            rpt (BasicProvers.FULL_CASE_TAC >> gvs[]) >>
+            (gvs[check_all_rows_match_def, is_match_row_def, is_atoml_true_def, sem_var_atom_def] >>
+             gvs[min_idx_till_def, INDEX_FIND_def, index_none_not_every]) >|[
+
+              qexistsl_tac [‘0’, ‘0’, ‘(T,res)’] >> 
+              gvs[]
+              ,
+
+              first_x_assum (strip_assume_tac o (Q.SPECL [‘st’, ‘mv’])) >>
+              qexistsl_tac [‘m+1’, ‘n+1’, ‘res’] >>      
+              gvs[GSYM INDEX_FIND_some_eq_next] 
+              ,
+              qexistsl_tac [‘0’, ‘0’, ‘(T,res)’] >> 
+              gvs[]
+              ,
+              BasicProvers.FULL_CASE_TAC >> gvs[] >|[
+                  qexistsl_tac [‘0’, ‘0’, ‘(T,res)’] >> 
+                  gvs[]
+                  ,
+                  
+                  first_x_assum (strip_assume_tac o (Q.SPECL [‘st’, ‘mv’])) >>
+                  qexistsl_tac [‘m+1’, ‘n+1’, ‘res’] >>      
+                  gvs[GSYM INDEX_FIND_some_eq_next] 
+
+                ]
+              ,
+              rpt (BasicProvers.FULL_CASE_TAC >> gvs[]) >|[
+                  first_x_assum (strip_assume_tac o (Q.SPECL [‘st’, ‘mv’])) >>
+                  qexistsl_tac [‘m+1’, ‘n+1’, ‘res’] >>      
+                  gvs[GSYM INDEX_FIND_some_eq_next] 
+                  ,
+                  qexistsl_tac [‘0’, ‘0’, ‘(T,res)’] >> 
+                  gvs[]
+                  ,
+                  first_x_assum (strip_assume_tac o (Q.SPECL [‘st’, ‘mv’])) >>
+                  qexistsl_tac [‘m+1’, ‘n+1’, ‘res’] >>      
+                  gvs[GSYM INDEX_FIND_some_eq_next] 
+                ]
+            ]
+            ,
+            Cases_on ‘h’ >> gvs[] >>
+            (gvs[check_all_rows_match_def, is_match_row_def, is_atoml_true_def, sem_var_atom_def] >>
+             gvs[min_idx_till_def, INDEX_FIND_def, index_none_not_every]) >|[
+
+                rpt (BasicProvers.FULL_CASE_TAC >> gvs[]) >|[
+                  qexistsl_tac [‘0’, ‘0’, ‘(T,res)’] >> 
+                  gvs[]
+                  ,
+                  first_x_assum (strip_assume_tac o (Q.SPECL [‘st’, ‘mv’])) >>
+                  qexistsl_tac [‘m+1’, ‘n+1’, ‘res’] >>      
+                  gvs[GSYM INDEX_FIND_some_eq_next] 
+                ]
+                ,
+                
+                first_x_assum (strip_assume_tac o (Q.SPECL [‘st’, ‘mv’])) >>
+                qexistsl_tac [‘m+1’, ‘n+1’, ‘res’] >>      
+                gvs[GSYM INDEX_FIND_some_eq_next] 
+                ,
+                
+                first_x_assum (strip_assume_tac o (Q.SPECL [‘st’, ‘mv’])) >>
+                qexistsl_tac [‘m+1’, ‘n+1’, ‘res’] >>      
+                gvs[GSYM INDEX_FIND_some_eq_next] 
+                ,
+                
+                rpt (BasicProvers.FULL_CASE_TAC >> gvs[]) >|[
+                  qexistsl_tac [‘0’, ‘0’, ‘(T,res)’] >> 
+                  gvs[]
+                  ,
+                  first_x_assum (strip_assume_tac o (Q.SPECL [‘st’, ‘mv’])) >>
+                  qexistsl_tac [‘m+1’, ‘n+1’, ‘res’] >>      
+                  gvs[GSYM INDEX_FIND_some_eq_next] 
+                  ]
+                ,
+                 rpt (BasicProvers.FULL_CASE_TAC >> gvs[]) >|[
+                  qexistsl_tac [‘0’, ‘0’, ‘(T,res)’] >> 
+                  gvs[]
+                  ,
+                  first_x_assum (strip_assume_tac o (Q.SPECL [‘st’, ‘mv’])) >>
+                  qexistsl_tac [‘m+1’, ‘n+1’, ‘res’] >>      
+                  gvs[GSYM INDEX_FIND_some_eq_next] 
+                  ]
+                ,
+                rpt (BasicProvers.FULL_CASE_TAC >> gvs[]) >|[
+                    
+                    first_x_assum (strip_assume_tac o (Q.SPECL [‘st’, ‘mv’])) >>
+                    qexistsl_tac [‘m+1’, ‘n+1’, ‘res’] >>      
+                    gvs[GSYM INDEX_FIND_some_eq_next]
+                    ,
+                    qexistsl_tac [‘0’, ‘0’, ‘(T,res)’] >> 
+                    gvs[]
+                    ,
+                    first_x_assum (strip_assume_tac o (Q.SPECL [‘st’, ‘mv’])) >>
+                    qexistsl_tac [‘m+1’, ‘n+1’, ‘res’] >>      
+                    gvs[GSYM INDEX_FIND_some_eq_next]
+                  ]
+
+              ]
+          ]                         
+      ]
+  ]
+QED
+
+
+
+
+
+
+
+
+
+
+
+
+
+        
+
+Theorem  min_idx_till_none_not_none:      
+  ∀ l .        
+    (min_idx_till l T = NONE) ⇔
+      ¬ (min_idx_till l T ≠ NONE)
+Proof
+  gvs[min_idx_till_def]
+QED
+
+Triviality a_not_a:
+∀ l . min_idx_till l T = NONE ∧ min_idx_till l T ≠ NONE ⇒ F
+Proof
+  gvs[min_idx_till_def]
+QED
+
+
+
+Triviality simp_table_none_empty_some_empty:
+  ∀ rows n.
+    simp_table rows NONE = [] ⇒
+    simp_table rows (SOME n) = []
 Proof
   Induct >>
-  rpt strip_tac >>
-  gvs[mk_substitute_tbl_def,simp_tbl_def] >>
+  rw[simp_table_def] >>
   PairCases_on ‘h’ >>
-  rename1 ‘(atoml, st_num, res)’ >>
-  gvs[MAP_MAP_o] >>
-  gvs[EXISTS_MAP] >>
-  res_tac >>
-                  
-  imp_res_tac is_match_row_substitute_preserve >>
-  gvs[]
+  gvs[simp_table_def] >>
+  rpt (BasicProvers.FULL_CASE_TAC >> gvs[simp_row_def]) 
 QED
 
 
-
-
-Theorem subst_simp_sem_tables_INDEX_FIND_congruence:
-  ∀ tbl mv s_in h' b i.
-    ALOOKUP mv h' = SOME b  ⇒
-    INDEX_FIND i (λ(p,a). p)
-               (MAP (λ(atoml,st_num,res). (is_match_row s_in st_num atoml mv,res)) (simp_tbl (mk_substitute_tbl tbl h' b))) =
-    INDEX_FIND i (λ(p,a). p)
-               (MAP (λ(atoml,st_num,res). (is_match_row s_in st_num atoml mv,res)) tbl)
-
-Proof
-  rpt strip_tac >>
-  imp_res_tac is_match_row_lists_subst_simp_eq >>
-  gvs[]
-QED
-
-
-
-Theorem subst_check_rows_sem_tables_INDEX_FIND_congruence:
-  ∀ tbl mv s_in h' b.
-    ALOOKUP mv h' = SOME b  ⇒
-    (check_all_rows_match s_in(simp_tbl (mk_substitute_tbl tbl h' b)) mv) =
-    (check_all_rows_match s_in tbl mv)
-Proof
-  gvs[check_all_rows_match_def] >>
-  rpt strip_tac >>
-  imp_res_tac is_match_row_lists_subst_simp_eq >>
-  gvs[]
-QED
-                      
-
-Theorem min_idx_till_subst_simp_invariant1:
-  ∀ tbl mv s_in h' b atoml st_num res .
-      ALOOKUP mv h' = SOME b  ⇒
-      min_idx_till (check_all_rows_match s_in (simp_tbl (mk_substitute_tbl ((atoml,st_num,res)::tbl) h' b)) mv) T =
-      min_idx_till (check_all_rows_match s_in ((atoml,st_num,res)::tbl) mv) T
-Proof
-  rpt strip_tac >> 
-  gvs[min_idx_till_def] >>
-  imp_res_tac subst_check_rows_sem_tables_INDEX_FIND_congruence >>
-  gvs[]  
-QED
-
-
-Theorem min_idx_till_subst_simp_invariant2:
-  ∀ tbl mv s_in h' b  .
-      ALOOKUP mv h' = SOME b  ⇒
-      min_idx_till (check_all_rows_match s_in (simp_tbl (mk_substitute_tbl (tbl) h' b)) mv) T =
-      min_idx_till (check_all_rows_match s_in (tbl) mv) T
-Proof   
-  rpt strip_tac >> 
-  gvs[min_idx_till_def] >>
-  imp_res_tac subst_check_rows_sem_tables_INDEX_FIND_congruence >>
-  gvs[]  
-QED
-
-
-Theorem sem_tables_subst_simp_invariant:
-  ∀ tbl mv s_in h' b row .
-    ALOOKUP mv h' = SOME b   ⇒
-    sem_tables ([simp_tbl (mk_substitute_tbl (row::tbl) h' b)],s_in) mv =
-    sem_tables ([row::tbl],s_in) mv
-Proof
-  rpt strip_tac >>
-  PairCases_on ‘row’ >> rename1 ‘(atoml,st_num,res)’ >>
-  gvs[] >>
         
-  simp[sem_tables_def, match_tbll_def] >>
-  gvs[match_tbl_def] >>
+Triviality simp_table_none_true_cases:
+  ∀ rows n st res.
+    (simp_table rows NONE = [([True],st,res)] ⇒
+    (simp_table rows (SOME n) = [([True],st,res)] ∨
+     simp_table rows (SOME n) = []
+    )) ∧
+
+    ( ∀ s . simp_table rows NONE = [([Var s],st,res)] ⇒
+     (simp_table rows (SOME n) = [([Var s],st,res)] ∨
+      simp_table rows (SOME n) = []                              
+     )) ∧
+
+    ( ∀ s l. simp_table rows NONE = [(Var s::l,st,res)] ⇒
+     (simp_table rows (SOME n) = [(Var s::l,st,res)] ∨
+      simp_table rows (SOME n) = []                              
+     )) ∧
+
+    ( ∀ s . simp_table rows NONE = [([Not s],st,res)] ⇒
+     (simp_table rows (SOME n) = [([Not s],st,res)] ∨
+      simp_table rows (SOME n) = []                              
+     )) ∧
+
+    ( ∀ s l. simp_table rows NONE = [(Not s::l,st,res)] ⇒
+     (simp_table rows (SOME n) = [(Not s::l,st,res)] ∨
+      simp_table rows (SOME n) = []                              
+     )) ∧
+
+    ( ∀ a l. simp_table rows NONE = [(a::l,st,res)] ⇒
+     (simp_table rows (SOME n) = [(a::l,st,res)] ∨
+      simp_table rows (SOME n) = []                              
+     )) ∧
+
+    ( ∀ a l. simp_table rows NONE = [([],st,res)] ⇒
+     (simp_table rows (SOME n) = [([],st,res)] ∨
+      simp_table rows (SOME n) = []                              
+     )) 
+Proof
+  Induct >>
+  rw[simp_table_def] >>
+  PairCases_on ‘h’ >>
+  gvs[simp_table_def] >>
+  rpt (BasicProvers.FULL_CASE_TAC >> gvs[simp_row_def]) >>
+  
+  imp_res_tac simp_table_none_empty_some_empty >>
+  imp_res_tac filtering_not_true_then_not_mem >>
+  gvs[]
+QED
+
+
+
+        
+Triviality simp_table_true_cases1:
+∀ rows n atoml st1 st2 res1 res2.
+simp_table rows NONE = [(True::atoml,st1,res1)] ∧
+simp_table rows (SOME n) = [([True],st2,res2)] ⇒
+(st1=st2 ∧ st2=n ∧ res1=res2)
+Proof
+
+  Induct >>
+  rw[simp_table_def] >>
+  PairCases_on ‘h’ >>
+  gvs[simp_table_def] >>
   rpt (BasicProvers.FULL_CASE_TAC >> gvs[]) >>
   
-  imp_res_tac min_idx_till_subst_simp_invariant1 >> gvs[] 
+  imp_res_tac simp_table_none_empty_some_empty >>
+  imp_res_tac filtering_not_true_then_not_mem >>
+  gvs[] >>
+  res_tac
 QED
-  
 
-     
-Theorem prop1_var_single_tbl_verbose:
-  ∀ tbl mv h' b s_in.
-    ALOOKUP mv h' = SOME b ⇒
-    sem_tables (simp_tbll (mk_substitute_tbll [tbl] h' b),s_in) mv =
-    sem_tables ([tbl],s_in) mv
+
+Triviality simp_row_cannot_result1:
+  ∀ atoml a l.
+    simp_row atoml ≠ [NotFalse] ∧
+    simp_row atoml ≠ [NotTrue] ∧
+    simp_row atoml ≠ False::a::l ∧
+    simp_row atoml ≠ True::a::l ∧
+    simp_row atoml ≠ NotFalse::a::l ∧
+    simp_row atoml ≠ NotTrue::a::l
+
 Proof
-  Cases >-
-   (gvs[fv_tbll_def, mk_substitute_tbll_def, simp_tbll_def] >> 
-   gvs[fv_tbl_def, mk_substitute_tbl_def, simp_tbl_def]) >> 
+  Induct >>
+  rw[simp_row_def] >>
+  rpt (BasicProvers.FULL_CASE_TAC >> gvs[]) >>
+  Cases_on ‘h’ >> gvs[simp_atom_def, is_not_true_var_atom_def] >>
+  rpt strip_tac >> gvs[] >>
+  imp_res_tac filtering_not_true_then_not_mem >> gvs[]
+QED
 
+
+
+    
+        
+Theorem simp_table_cannot_result1:
+  ∀ rows st res.
+    (simp_table rows NONE ≠ [([NotFalse],st,res)]) ∧
+    (simp_table rows NONE ≠ [([NotTrue],st,res)]) ∧
+    (simp_table rows NONE ≠ [([False],st,res)]) ∧
+                    
+    (∀ a l.(simp_table rows NONE ≠ [(False::a::l,st,res)])) ∧
+    (∀ a l.(simp_table rows NONE ≠ [(True::a::l,st,res)])) ∧
+    (∀ a l.(simp_table rows NONE ≠ [(NotTrue::a::l,st,res)])) ∧
+    (∀ a l.(simp_table rows NONE ≠ [(NotFalse::a::l,st,res)]))
+Proof
+  
+  Induct >>
+  rw[simp_table_def] >>
+  PairCases_on ‘h’ >>
+  gvs[simp_table_def] >>
+  rpt (BasicProvers.FULL_CASE_TAC >> gvs[]) >>
   rpt strip_tac >>
-  gvs[mk_substitute_tbll_def, simp_tbll_def] >> 
-  imp_res_tac sem_tables_subst_simp_invariant >>
-  gvs[]  
-QED
-            
+  gvs[simp_row_cannot_result1] 
+QED   
+               
 
 
-            
-Theorem prop1_var_tables_verbose:
-  ∀ tbls h b mv s_in.
-    ALOOKUP mv h = SOME b 
-    ⇒
-    sem_tables (simp_tbll (mk_substitute_tbll tbls h b),s_in) mv =
-    sem_tables (tbls,s_in) mv
+
+
+
+Theorem min_idx_check_rows_simp_tbl_some2:
+  ∀ rows st_in mv simp_rows simp_rows' m n r r'.
+    simp_table rows NONE = simp_rows ∧
+    simp_table rows (SOME st_in) = simp_rows' ⇒
+    (min_idx_till (check_all_rows_match st_in simp_rows mv) T = SOME (n, r)) ∧
+    (min_idx_till (check_all_rows_match st_in simp_rows' mv) T = SOME (m, r')) ⇒
+    r=r'
 Proof
 
-  Induct_on ‘tbls’ >> rpt strip_tac >-
-   gvs[fv_tbll_def, mk_substitute_tbll_def, simp_tbll_def] >> 
-  rename1 ‘(tbl::tbll)’ >>
+  Induct_on ‘rows’ >>
+  rpt strip_tac >-
+   rgs[simp_table_def, check_all_rows_match_def, min_idx_till_def, INDEX_FIND_def] >>
+  
+  
+  PairCases_on ‘h’ >>
+  rename1 ‘simp_table ((atoms,st,res)::rows) (SOME st_in)’ >>
+  rgs[simp_table_def] >>
+  Cases_on ‘simp_row atoms’ >> gvs[] >-
+   (
+   imp_res_tac simp_row_not_empty >>
+   gvs[] >>
+   Cases_on ‘st_in ≠ st’ >>
+   gvs[check_all_rows_match_def] >>
+   gvs[GSYM INDEX_FIND_some_eq_next2] >>
+   res_tac >>
+   gvs[is_match_row_def] >>
 
-  imp_res_tac prop1_var_single_tbl_verbose >>
-  first_x_assum (strip_assume_tac o (Q.SPECL [‘tbl’, ‘s_in’])) >>
+   gvs[GSYM min_idx_till_some_eq_next2] >>
+   res_tac 
+   ) >>
+        
+  Cases_on ‘st_in ≠ st’ >>
+  gvs[] >|[
+        Cases_on ‘h’ >> gvs[] >>
+        gvs[check_all_rows_match_def] >>
+        gvs[is_match_row_def] >>
+
+        gvs[GSYM min_idx_till_some_eq_next2] >>
+        res_tac >>
+
+        Cases_on ‘t’ >> gvs[simp_row_cannot_result1]
+        ,
+
+        Cases_on ‘h’ >> Cases_on ‘t’ >>  gvs[simp_row_cannot_result1] >>
+
+        (gvs[check_all_rows_match_def, is_match_row_def, is_atoml_true_def, sem_var_atom_def] >>
+         gvs[min_idx_till_def, INDEX_FIND_def, index_none_not_every]) >>
+         
+        rpt (BasicProvers.FULL_CASE_TAC >> gvs[]) >>
+        gvs[GSYM min_idx_till_some_eq_next2] >>
+        res_tac >>
+
+
                 
-  Cases_on ‘tbll’ >> gvs[] >> 
-  rename1 ‘(tbl::nexttbl::tbll)’ >>
-
-  gvs[sem_tables_def, match_tbll_def] >>
-  Cases_on ‘match_tbl tbl mv s_in’ >> gvs[] >>
-  rpt (BasicProvers.FULL_CASE_TAC >> gvs[]) >>
-
-  gvs[mk_substitute_tbll_def, simp_tbll_def] >>
-  gvs[match_tbll_def] >>     
-  Cases_on ‘match_tbl (simp_tbl (mk_substitute_tbl tbl h' b)) mv s_in’ >> gvs[] >>
-  rpt (BasicProvers.FULL_CASE_TAC >> gvs[]) >>
-
-  gvs[match_tbl_def] >>
-  rpt (BasicProvers.FULL_CASE_TAC >> gvs[]) >>
-  imp_res_tac min_idx_till_subst_simp_invariant2 >> gvs[]
+        gvs[INDEX_FIND_some_eq_next] >>
+        Cases_on ‘n’ >> Cases_on ‘m’ >> gvs[index_find_not_prev, ADD1] >>
+        res_tac 
+]
+                               
 QED
+
+
+               
+          
+        
+        
+Theorem simp_tables_single_match_eq:
+  ∀ rows n tbl tbl' mv.
+    simp_tables [rows] NONE = [tbl] ∧
+    simp_tables [rows] (SOME n) = [tbl'] ⇒
+    match_tbl tbl mv n = match_tbl tbl' mv n
+Proof
+
+  rw[simp_tables_def, match_tbl_def] >>
+  Cases_on ‘simp_table rows NONE’ >> 
+  Cases_on ‘simp_table rows (SOME n)’ >> 
+  gvs[] >>
+  
+  imp_res_tac min_idx_check_rows_simp_tbl_none >>
+  imp_res_tac min_idx_check_rows_simp_tbl_some >>
+  gvs[] >>
+  
+  (first_x_assum (strip_assume_tac o (Q.SPECL [‘mv’])) >>
+   first_x_assum (strip_assume_tac o (Q.SPECL [‘mv’]))) >| [
+    
+    imp_res_tac simp_table_none_empty_some_empty >> gvs[]
+    ,
+    
+    Cases_on ‘t’ >> PairCases_on ‘h’ >> gvs[] >>
+    Cases_on ‘h0’ >> gvs[] >>
+    
+    (rpt (BasicProvers.FULL_CASE_TAC >> gvs[]) >>     
+     gvs[check_all_rows_match_def, min_idx_till_def, is_match_row_def] >>
+     gvs[INDEX_FIND_def])
+    
+    ,
+    
+    Cases_on ‘t’ >> PairCases_on ‘h’ >> gvs[] >>
+    Cases_on ‘h0’ >> gvs[] >|[
+        
+        Cases_on ‘t'’ >> PairCases_on ‘h'’ >> gvs[] >>
+        (rpt (BasicProvers.FULL_CASE_TAC >> gvs[]) >>     
+         gvs[check_all_rows_match_def, min_idx_till_def, is_match_row_def] >>
+         gvs[INDEX_FIND_def])
+        ,
+        
+        Cases_on ‘h’ >> Cases_on ‘t’ >> gvs[] >>
+        gvs[simp_table_cannot_result1]  >>
+        (
+        TRY(Cases_on ‘h2’) >> gvs[] >>
+        imp_res_tac simp_table_none_true_cases >> gvs[] >>
+        first_x_assum (strip_assume_tac o (Q.SPECL [‘n’])) >>
+        gvs[])
+        
+        ,                
+        Cases_on ‘t'’ >> PairCases_on ‘h'’ >> gvs[] >|[
+            Cases_on ‘h'0’ >> gvs[] >|[
+              
+              (rpt (BasicProvers.FULL_CASE_TAC >> gvs[]) >>     
+               gvs[check_all_rows_match_def, min_idx_till_def, is_match_row_def] >>
+               gvs[INDEX_FIND_def])
+              ,
+              
+              rpt (BasicProvers.FULL_CASE_TAC >> gvs[]) >>
+              gvs[is_atoml_true_def, sem_var_atom_def] >>                     
+              
+              imp_res_tac min_idx_check_rows_simp_tbl_some2 >>
+              res_tac >> gvs[] >>
+              res_tac >> gvs[] 
+                            
+            ]
+            ,
+            rpt (BasicProvers.FULL_CASE_TAC >> gvs[]) >>
+            gvs[is_atoml_true_def, sem_var_atom_def] >>                     
+            
+            imp_res_tac min_idx_check_rows_simp_tbl_some2 >>
+            res_tac >> gvs[] 
+          ]
+        ,
+        Cases_on ‘t'’ >> PairCases_on ‘h'’ >> gvs[] >|[
+            Cases_on ‘h'0’ >> gvs[] >|[
+              
+              (rpt (BasicProvers.FULL_CASE_TAC >> gvs[]) >>     
+               gvs[check_all_rows_match_def, min_idx_till_def, is_match_row_def] >>
+               gvs[INDEX_FIND_def])
+              ,
+              
+              rpt (BasicProvers.FULL_CASE_TAC >> gvs[]) >>
+              gvs[is_atoml_true_def, sem_var_atom_def] >>                     
+              
+              imp_res_tac min_idx_check_rows_simp_tbl_some2 >>
+              res_tac >> gvs[] >>
+              res_tac >> gvs[] 
+                            
+            ]
+            ,
+            rpt (BasicProvers.FULL_CASE_TAC >> gvs[]) >>
+            gvs[is_atoml_true_def, sem_var_atom_def] >>                     
+            
+            imp_res_tac min_idx_check_rows_simp_tbl_some2 >>
+            res_tac >> gvs[] 
+          ]
+      ]
+  ]
+QED
+              
+
+
+                                                
+Theorem match_tbll_single_some_none_eq:
+  ∀rows mv n.
+    match_tbll (simp_tables [rows] NONE) mv n =
+    match_tbll (simp_tables [rows] (SOME n)) mv n
+Proof
+  
+  rw[] >>
+  assume_tac length_of_simp_single_table >>
+  first_assum (strip_assume_tac o (Q.SPECL [‘rows’, ‘NONE’])) >>
+  first_x_assum (strip_assume_tac o (Q.SPECL [‘rows’, ‘SOME n’])) >>
+ 
+  Cases_on ‘simp_tables [rows] NONE’ >> gvs[] >>
+  Cases_on ‘simp_tables [rows] (SOME n)’ >> gvs[] >>
+  
+  gvs[simp_tables_single_not_empty] >>
+  Cases_on ‘t’ >> gvs[] >>
+  Cases_on ‘t'’ >> gvs[] >>
+  
+  gvs[match_tbll_def] >>
+  imp_res_tac simp_tables_single_match_eq >>
+  metis_tac[]
+QED
+
+
+
+
+
+
+
+
+
+
+Triviality simp_tables_res_empty_length:
+  ∀ tbll sop.
+    simp_tables tbll sop = [] ⇒
+    tbll = []
+Proof
+  Cases_on ‘sop’ >>
+  Induct >> rw[simp_tables_def] >>
+  rpt (BasicProvers.FULL_CASE_TAC >> gvs[]) 
+QED
+
+        
+Triviality simp_tables_res_single_length:
+  ∀ tbll tbl n sop.
+    simp_tables tbll sop = [tbl] ⇒
+    LENGTH tbll = 1
+Proof
+  Induct >> rw[simp_tables_def] >>
+  rpt (BasicProvers.FULL_CASE_TAC >> gvs[]) >>
+  imp_res_tac simp_tables_res_empty_length
+QED
+
+
+
+(*
+new definition for simp_tables 
+so that the proofs are easier to deal with
+*)
+
+
+Definition next_state_def:
+  next_state t' = case t' of
+                  | [([True], s, state s'')] => SOME s''
+                  | _ => NONE
+End
+
+
+Definition simp_tables2_def:
+  (simp_tables2 [] s = []) ∧
+  (simp_tables2 (t::tbll) s = 
+   let t' = simp_table t s in
+   t' :: simp_tables2 tbll (next_state t')
+  )
+End
+
+
+Theorem simp_tables_eq:
+  ∀ l s.
+    simp_tables l s = simp_tables2 l s
+Proof 
+  Induct >>
+  rw[simp_tables2_def, simp_tables_def] >>
+  rpt (BasicProvers.FULL_CASE_TAC >> gvs[]) >>     
+  
+  Cases_on ‘s’ >> gvs[next_state_def]
+QED
+
+
+Theorem next_state_rel_to_final_match_res:
+  ∀ tbl n n' n'' mv.
+    match_tbl tbl mv n = SOME (state n') ∧
+    next_state tbl = SOME n'' ⇒
+    n' = n''
+Proof
+  rw[next_state_def] >>
+  rpt (BasicProvers.FULL_CASE_TAC >> rgs[]) >>
+  gvs[match_tbl_def, check_all_rows_match_def, is_match_row_def,
+      is_atoml_true_def, min_idx_till_def, sem_var_atom_def, INDEX_FIND_def] >>
+  rpt (BasicProvers.FULL_CASE_TAC >> rgs[]) 
+QED
+
+
+
+Theorem simp_table_eq_none_some:
+  ∀ tbl t_s t_n mv n.
+    simp_table tbl (SOME n) = t_s ∧
+    simp_table tbl NONE = t_n ⇒
+    match_tbl t_n mv n = match_tbl t_s mv n
+Proof
+
+  rw[match_tbl_def] >>
+  rpt (BasicProvers.FULL_CASE_TAC >> rgs[])  >>
+  
+  ‘∃ l . simp_table tbl NONE = l’ by gvs[] >>
+  ‘∃ l' . simp_table tbl (SOME n) = l'’ by gvs[] >|[
+    
+    imp_res_tac min_idx_check_rows_simp_tbl_none >>
+    gvs[]
+    ,
+    imp_res_tac min_idx_check_rows_simp_tbl_none >>
+    gvs[] >>
+    first_x_assum (strip_assume_tac o (Q.SPECL [‘mv’])) >>
+    gvs[]
+    ,
+    imp_res_tac min_idx_check_rows_simp_tbl_some2 >>
+    gvs[] >>
+    
+    first_x_assum (strip_assume_tac o (Q.SPECL [‘r'’, ‘mv’, ‘q'’])) >>
+    gvs[]
+  ]
+QED
+
+
+        
+        
+Theorem match_tbll_simp_tables_eq_thm:
+  ∀tbll mv n.
+    match_tbll (simp_tables tbll NONE) mv n =
+    match_tbll (simp_tables tbll (SOME n)) mv n
+Proof
+  
+Induct_on ‘tbll’ >> rw[] >|[
+    gvs[simp_tables_def]
+    ,
+    Cases_on ‘tbll’ >> gvs[] >|[
+        gvs[match_tbll_single_some_none_eq]
+        ,
+        Cases_on ‘simp_tables (h::h'::t) (SOME n)’ >>
+        Cases_on ‘simp_tables (h::h'::t) NONE’ >>  
+        imp_res_tac simp_tables_res_empty_length >> gvs[] >>
+                    
+        Cases_on ‘t'’ >>
+        Cases_on ‘t''’ >>  
+        imp_res_tac simp_tables_res_single_length >> gvs[] >> 
+
+        rename1 ‘match_tbll (t1_n::t2_n::t3_n) mv n = match_tbll (t1_s::t2_s::t3_s) mv n’ >>
+                    
+
+        gvs[simp_tables_eq] >>
+        
+        (Q.PAT_X_ASSUM ‘simp_tables2 (h::h'::t) (SOME n) = t1_s::t2_s::t3_s’
+          (fn thm => ASSUME_TAC (SIMP_RULE (srw_ss()) [Once simp_tables2_def] thm))) >>
+        
+        
+        
+        (Q.PAT_X_ASSUM ‘simp_tables2 (h::h'::t) NONE = t1_n::t2_n::t3_n’
+          (fn thm => ASSUME_TAC (SIMP_RULE (srw_ss()) [Once simp_tables2_def] thm))) >>
+        
+        rgs[] >>
+        
+        simp[match_tbll_def] >>
+        ‘match_tbl t1_n mv n = match_tbl t1_s mv n’ by (imp_res_tac simp_table_eq_none_some >>
+                                                        first_x_assum (strip_assume_tac o (Q.SPECL [‘mv’]))
+                                                       ) >>
+        
+        
+        Cases_on ‘match_tbl t1_s mv n’ >> rgs[] >>
+        Cases_on ‘x’ >> rgs[] >>
+                
+        Cases_on ‘next_state t1_s’ >>
+        Cases_on ‘next_state t1_n’ >>
+        rgs[] >>
+        
+        imp_res_tac next_state_rel_to_final_match_res >> gvs[]
+      ]
+  ]
+QED
+   
+
+
+(* to do : same as simp_table_cannot_result1 merge them *)
+Theorem simp_table_cannot_result2:
+  ∀ rows st res n.
+    (simp_table rows (SOME n) ≠ [([NotFalse],st,res)]) ∧
+    (simp_table rows (SOME n) ≠ [([NotTrue],st,res)]) ∧
+    (simp_table rows (SOME n) ≠ [([False],st,res)]) ∧
+                    
+    (∀ a l.(simp_table rows (SOME n) ≠ [(False::a::l,st,res)])) ∧
+    (∀ a l.(simp_table rows (SOME n) ≠ [(True::a::l,st,res)])) ∧
+    (∀ a l.(simp_table rows (SOME n) ≠ [(NotTrue::a::l,st,res)])) ∧
+    (∀ a l.(simp_table rows (SOME n) ≠ [(NotFalse::a::l,st,res)])) 
+Proof
+  
+  Induct >>
+  rw[simp_table_def] >>
+  PairCases_on ‘h’ >>
+  gvs[simp_table_def] >>
+  rpt (BasicProvers.FULL_CASE_TAC >> gvs[]) >>
+  rpt strip_tac >>
+  gvs[simp_row_cannot_result1] 
+QED
+
+
+
+
+
+        
+Theorem sem_var_atom_sub_same:
+  ∀ atom mv x b b'.
+    ALOOKUP mv x = SOME b  ⇒
+    (sem_var_atom atom mv = SOME b' ⇔
+    sem_var_atom (mk_substitute_atom atom x b) mv = SOME b')
+Proof
+  Cases >>
+  rw[sem_var_atom_def, mk_substitute_atom_def] >>
+  Cases_on ‘b'’ >> gvs[]
+QED
+
+
+Theorem sem_var_atoml_sub_same_imp1:
+  ∀ atoml mv x b.        
+    ALOOKUP mv x = SOME b ∧
+    EVERY (λminipred. sem_var_atom minipred mv = SOME T) atoml ⇒
+    EVERY (λminipred. sem_var_atom minipred mv = SOME T)
+          (MAP (λatom. mk_substitute_atom atom x b) atoml)
+Proof
+  Induct >>
+  rw[] >>
+  imp_res_tac sem_var_atom_sub_same
+QED
+
+
+Theorem sem_var_atoml_sub_same_imp2:
+  ∀ atoml mv x b.        
+    ALOOKUP mv x = SOME b ∧
+    EVERY (λminipred. sem_var_atom minipred mv = SOME T)
+          (MAP (λatom. mk_substitute_atom atom x b) atoml) ⇒
+    EVERY (λminipred. sem_var_atom minipred mv = SOME T) atoml
+Proof
+  Induct >>
+  rw[] >>
+  imp_res_tac sem_var_atom_sub_same >>
+  res_tac
+QED
+
+
+        
+        
+Theorem is_match_row_mk_sub_eq:
+  ∀ atoml st s_in mv x b.
+    ALOOKUP mv x = SOME b ⇒
+    (is_match_row s_in st atoml mv ⇔ is_match_row s_in st (mk_substitute_row atoml x b) mv)
+Proof
+  Induct >>
+  rw[is_match_row_def] >>
+  gvs[mk_substitute_row_def, is_atoml_true_def] >>
+  
+  EQ_TAC >> rw[] >>
+  
+  imp_res_tac sem_var_atom_sub_same >> gvs[] >>
+  imp_res_tac sem_var_atoml_sub_same_imp1 >> gvs[] >>
+  imp_res_tac sem_var_atoml_sub_same_imp2 >> gvs[]
+QED
+
+
+    
+Theorem check_all_rows_match_sub_eq:
+  ∀ tbl x b mv s_in.
+    ALOOKUP mv x = SOME b ⇒
+    (check_all_rows_match s_in tbl mv = check_all_rows_match s_in (mk_substitute_tbl tbl x b) mv)
+Proof
+  Induct >>
+  rw[check_all_rows_match_def] >-
+   gvs[mk_substitute_tbl_def] >>
+  
+  PairCases_on ‘h’ >>
+  gvs[check_all_rows_match_def] >>
+  
+  res_tac >>
+  first_x_assum (strip_assume_tac o (Q.SPECL [‘s_in’])) >>
+  gvs[] >>
+  
+  gvs[mk_substitute_tbl_def] >>
+  assume_tac (INST_TYPE [“:'a ”|-> “:num”  ] is_match_row_mk_sub_eq)  >>
+  metis_tac[]
+QED                           
+
+
+
+Triviality simp_row_single_true_rel:
+  ∀ atoms h.
+    simp_row (h::atoms) = [True] ⇒
+    (simp_row atoms = [True] ∨ atoms = [])
+Proof
+  rw[simp_row_def] >>
+  gvs[] 
+QED
+      
+
+
+Triviality simp_row_single_false_rel:
+  ∀ t h mv.
+    sem_var_atom h mv = SOME T ∧
+    simp_row (h::t) = [False] ⇒
+    simp_row (t) = [False]
+Proof
+  rw[simp_row_def] >>
+  gvs[is_not_true_var_atom_def]  >>
+  
+  Cases_on ‘h’ >> gvs[simp_row_def, sem_var_atom_def, simp_atom_def, is_not_true_var_atom_def] >>  
+  rpt (BasicProvers.FULL_CASE_TAC >> gvs[])
+QED        
+
+
+           
+Theorem simp_row_true_imp_atoml_true:
+  ∀ atoms mv.
+    atoms ≠ [] ∧
+    simp_row atoms = [True] ⇒
+    (is_atoml_true atoms mv)
+Proof
+  Induct >>
+  rw[is_atoml_true_def] >|[
+    
+    (* for head *)
+    rgs[Once simp_row_def] >>
+    rpt (BasicProvers.FULL_CASE_TAC >> gvs[]) >>
+
+    gvs[is_not_true_var_atom_def] >>
+    Cases_on ‘h’ >> gvs[simp_atom_def, is_not_true_var_atom_def, is_atoml_true_def, sem_var_atom_def]
+    ,
+        
+    (* for list *)
+    imp_res_tac simp_row_single_true_rel >>
+    res_tac >> gvs[] >>
+    
+    Cases_on ‘atoms’ >>
+    imp_res_tac simp_row_not_empty >> gvs[] >>
+    first_x_assum (strip_assume_tac o (Q.SPECL [‘mv’])) >>
+    gvs[is_atoml_true_def]
+  ]
+QED
+
+
+
+
+
+                                          
+        
+Theorem simp_row_false_imp_atoml_false:
+  ∀ atoms mv.
+    simp_row atoms = [False] ⇒
+    ~ (is_atoml_true atoms mv)
+Proof
+  Induct >>
+  rw[is_atoml_true_def] >-
+   rgs[simp_row_def] >>
+  
+  
+  Cases_on ‘atoms’ >>
+  imp_res_tac simp_row_not_empty >> gvs[] >>
+  first_x_assum (strip_assume_tac o (Q.SPECL [‘mv’])) >>
+  gvs[is_atoml_true_def] >|[
+    Cases_on ‘h’ >> gvs[simp_row_def, sem_var_atom_def, simp_atom_def, is_not_true_var_atom_def]    
+    ,
+    imp_res_tac simp_row_single_false_rel >>
+    res_tac
+  ]
+QED
+
+
+Triviality filter_simp_empty_then_all_true:
+  ∀ atoms mv.
+    atoms ≠ [] ∧
+    FILTER (λx. is_not_true_var_atom x) (MAP (λatom. simp_atom atom) atoms) = [] ⇒
+    EVERY (λminipred. sem_var_atom minipred mv = SOME T) atoms
+Proof
+  Induct >>
+  rw[] >>
+  Cases_on ‘h’ >> gvs[sem_var_atom_def, simp_atom_def, is_not_true_var_atom_def] >>    
+  Cases_on ‘atoms’ >> gvs[]
+QED
+                                          
+        
+        
+Theorem simp_row_var_imp_atoml_true:
+  ∀ atoms mv s.
+    simp_row atoms = [Var s] ⇒
+    (is_atoml_true atoms mv ⇔ is_atoml_true [Var s] mv)
+Proof
+  Induct >>
+  rw[is_atoml_true_def] >-
+   gvs[simp_row_def] >>
+  
+  Cases_on ‘h’ >> gvs[simp_row_def, sem_var_atom_def, simp_atom_def, is_not_true_var_atom_def] >>
+  rpt (BasicProvers.FULL_CASE_TAC >> gvs[]) >>
+  gvs[is_atoml_true_def, sem_var_atom_def] >>
+  imp_res_tac filter_simp_empty_then_all_true >>
+  gvs[]
+QED
+
+
+
+
+Theorem simp_row_not_imp_atoml_true:
+  ∀ atoms mv s.
+    simp_row atoms = [Not s] ⇒
+    (is_atoml_true atoms mv ⇔ is_atoml_true [Not s] mv)
+Proof
+  Induct >>
+  rw[is_atoml_true_def] >-
+   gvs[simp_row_def] >>
+  
+  Cases_on ‘h’ >> gvs[simp_row_def, sem_var_atom_def, simp_atom_def, is_not_true_var_atom_def] >>
+  rpt (BasicProvers.FULL_CASE_TAC >> gvs[]) >>
+  gvs[is_atoml_true_def, sem_var_atom_def] >>
+
+  imp_res_tac filter_simp_empty_then_all_true >>
+  gvs[] >>
+                         
+  first_x_assum (strip_assume_tac o (Q.SPECL [‘mv’])) >>
+  rpt (BasicProvers.FULL_CASE_TAC >> gvs[])
+QED
+
+
+
+
+Theorem simp_row_list_imp_atoml_true:
+  ∀ atoms l mv.
+    simp_row atoms = l ⇒
+    is_atoml_true atoms mv = is_atoml_true l mv
+Proof
+  Induct >>
+  rw[is_atoml_true_def] >-
+   gvs[simp_row_def] >>
+  
+  Cases_on ‘h’ >> gvs[simp_row_def, sem_var_atom_def, simp_atom_def, is_not_true_var_atom_def] >>
+  rpt (BasicProvers.FULL_CASE_TAC >> gvs[]) >>
+  gvs[is_atoml_true_def, sem_var_atom_def]
+QED
+
+
+                                          
+Theorem min_idx_till_simp_eq_none:
+  ∀ l s_in mv.
+    min_idx_till (check_all_rows_match s_in l mv) T = NONE ⇔
+      min_idx_till (check_all_rows_match s_in (simp_table l (SOME s_in)) mv) T = NONE
+Proof
+  
+  Induct >>
+  rw[]  >-
+   gvs[simp_table_def] >>
+  
+  PairCases_on ‘h’ >>         
+  rename1 ‘((atoms,st,res)::rows)’ >>
+  
+  gvs[simp_table_def] >>
+  Cases_on ‘s_in ≠ st’ >> gvs[] >|[
+    gvs[check_all_rows_match_def, is_match_row_def] >>
+    metis_tac[min_idx_till_none_eq_res]
+    ,
+    Cases_on ‘simp_row atoms’ >-
+     (
+     imp_res_tac simp_row_not_empty >> gvs[] >>
+     gvs[check_all_rows_match_def, is_match_row_def] >>
+     metis_tac[min_idx_till_none_eq_res]
+     ) >>
+    
+    
+    Cases_on ‘t’ >> gvs[] >| [
+        Cases_on ‘h’ >> gvs[simp_row_cannot_result1] >| [
+          
+          (* true case *)
+          gvs[check_all_rows_match_def] >>
+          gvs[is_match_row_def] >>
+          Cases_on ‘atoms = []’ >-
+           gvs[simp_row_def] >>
+          imp_res_tac simp_row_true_imp_atoml_true >>
+          first_x_assum (strip_assume_tac o (Q.SPECL [‘mv’])) >>
+          gvs[min_idx_till_def, is_atoml_true_def, INDEX_FIND_def, sem_var_atom_def]
+          ,
+          (* false *)
+          imp_res_tac simp_row_false_imp_atoml_false >>
+          first_x_assum (strip_assume_tac o (Q.SPECL [‘mv’])) >>
+          gvs[check_all_rows_match_def] >>
+          gvs[is_match_row_def] >>
+          metis_tac[min_idx_till_none_eq_res]
+          ,
+          (* var case *)
+          gvs[check_all_rows_match_def, is_match_row_def] >>
+          Cases_on ‘atoms = []’ >-
+           gvs[simp_row_def] >>
+          gvs[] >>
+          imp_res_tac simp_row_var_imp_atoml_true >>
+          gvs[] >>
+          Cases_on ‘is_atoml_true [Var s] mv’ >> gvs[] >|[
+              gvs[min_idx_till_def, is_atoml_true_def, INDEX_FIND_def, sem_var_atom_def]
+              ,
+              metis_tac[min_idx_till_none_eq_res]
+            ]
+          ,
+          (* case not *)
+          gvs[check_all_rows_match_def, is_match_row_def] >>
+          Cases_on ‘atoms = []’ >-
+           gvs[simp_row_def] >>
+          gvs[] >>
+          imp_res_tac simp_row_not_imp_atoml_true >>
+          gvs[] >> 
+          Cases_on ‘is_atoml_true [Not s] mv’ >> gvs[] >|[
+              gvs[min_idx_till_def, is_atoml_true_def, INDEX_FIND_def, sem_var_atom_def]
+              ,
+              metis_tac[min_idx_till_none_eq_res]
+            ]               
+        ]
+        ,
+        gvs[check_all_rows_match_def, is_match_row_def] >>
+        imp_res_tac simp_row_list_imp_atoml_true >>
+        gvs[] >>
+
+        Cases_on ‘atoms = []’ >-
+         gvs[simp_row_def] >>
+        gvs[] >>
+              
+        Cases_on ‘is_atoml_true (h::h'::t') mv’ >> gvs[] >|[
+            gvs[min_idx_till_def, is_atoml_true_def, INDEX_FIND_def, sem_var_atom_def]
+            ,
+            metis_tac[min_idx_till_none_eq_res]
+          ]                                                    
+      ]      
+  ]                    
+QED
+
+        
+
+
+    
+Theorem min_idx_till_simp_sub_eq_none:
+  ∀ t t' mv x b s_in.
+    ALOOKUP mv x = SOME b ∧
+    simp_table (mk_substitute_tbl t x b) (SOME s_in) = t' ⇒
+    (min_idx_till (check_all_rows_match s_in t mv) T = NONE ⇔
+       min_idx_till (check_all_rows_match s_in t' mv) T = NONE )
+Proof
+  rw[] >>
+  ‘check_all_rows_match s_in t mv = check_all_rows_match s_in (mk_substitute_tbl t x b) mv’
+    by gvs[check_all_rows_match_sub_eq] >>
+  gvs[] >>
+  metis_tac[min_idx_till_simp_eq_none]
+QED
+
+
+(* to do : same proof as none, merge them *)
+Theorem min_idx_till_simp_eq_some:
+  ∀l s_in mv r r' idx idx'.
+    min_idx_till (check_all_rows_match s_in l mv) T = SOME (idx,r) ∧
+    min_idx_till (check_all_rows_match s_in (simp_table l (SOME s_in)) mv) T = SOME (idx',r')       ⇒
+    r = r'
+Proof
+  Induct >>
+  rw[]  >-
+   gvs[simp_table_def] >>
+  
+  PairCases_on ‘h’ >>         
+  rename1 ‘((atoms,st,res)::rows)’ >>
+  
+  gvs[simp_table_def] >>
+  Cases_on ‘s_in ≠ st’ >> gvs[] >|[
+    gvs[check_all_rows_match_def, is_match_row_def] >>
+    gvs[GSYM min_idx_till_some_eq_next2] >>
+    res_tac
+    ,
+    Cases_on ‘simp_row atoms’ >-
+     (
+     imp_res_tac simp_row_not_empty >> gvs[] >>
+     gvs[check_all_rows_match_def, is_match_row_def] >>
+     gvs[GSYM min_idx_till_some_eq_next2] >>
+     res_tac
+     ) >>
+   
+    Cases_on ‘t’ >> gvs[] >| [
+        Cases_on ‘h’ >> gvs[simp_row_cannot_result1] >| [
+          
+          (* true case *)
+          gvs[check_all_rows_match_def] >>
+          gvs[is_match_row_def] >>
+          Cases_on ‘atoms = []’ >-
+           gvs[simp_row_def] >>
+          imp_res_tac simp_row_true_imp_atoml_true >>
+          first_x_assum (strip_assume_tac o (Q.SPECL [‘mv’])) >>
+          gvs[min_idx_till_def, is_atoml_true_def, INDEX_FIND_def, sem_var_atom_def]
+          ,
+          (* false *)
+          imp_res_tac simp_row_false_imp_atoml_false >>
+          first_x_assum (strip_assume_tac o (Q.SPECL [‘mv’])) >>
+          gvs[check_all_rows_match_def] >>
+          gvs[is_match_row_def] >>
+          gvs[GSYM min_idx_till_some_eq_next2] >>
+          res_tac
+          ,
+          (* var case *)
+          gvs[check_all_rows_match_def, is_match_row_def] >>
+          Cases_on ‘atoms = []’ >-
+           gvs[simp_row_def] >>
+          gvs[] >>
+          imp_res_tac simp_row_var_imp_atoml_true >>
+          gvs[] >>
+          Cases_on ‘is_atoml_true [Var s] mv’ >> gvs[] >|[
+              gvs[min_idx_till_def, is_atoml_true_def, INDEX_FIND_def, sem_var_atom_def]
+              ,
+              gvs[GSYM min_idx_till_some_eq_next2] >>
+              res_tac
+            ]
+          ,
+          (* case not *)
+          gvs[check_all_rows_match_def, is_match_row_def] >>
+          Cases_on ‘atoms = []’ >-
+           gvs[simp_row_def] >>
+          gvs[] >>
+          imp_res_tac simp_row_not_imp_atoml_true >>
+          gvs[] >> 
+          Cases_on ‘is_atoml_true [Not s] mv’ >> gvs[] >|[
+              gvs[min_idx_till_def, is_atoml_true_def, INDEX_FIND_def, sem_var_atom_def]
+              ,
+               gvs[GSYM min_idx_till_some_eq_next2] >>
+              res_tac
+            ]               
+        ]
+        ,
+        gvs[check_all_rows_match_def, is_match_row_def] >>
+        imp_res_tac simp_row_list_imp_atoml_true >>
+        gvs[] >>
+
+        Cases_on ‘atoms = []’ >-
+         gvs[simp_row_def] >>
+        gvs[] >>
+              
+        Cases_on ‘is_atoml_true (h::h'::t') mv’ >> gvs[] >|[
+            gvs[min_idx_till_def, is_atoml_true_def, INDEX_FIND_def, sem_var_atom_def]
+            ,
+             gvs[GSYM min_idx_till_some_eq_next2] >>
+              res_tac
+          ]                                                    
+      ]   
+  ]
+QED
+
+
+        
+Theorem min_idx_till_simp_sub_eq_some:
+  ∀ t t' mv x b s_in idx idx' res res'.
+    ALOOKUP mv x = SOME b ∧
+    simp_table (mk_substitute_tbl t x b) (SOME s_in) = t' ∧
+    min_idx_till (check_all_rows_match s_in t mv) T = SOME (idx, res) ∧
+    min_idx_till (check_all_rows_match s_in t' mv) T = SOME (idx', res') ⇒
+    res = res'
+Proof
+  rw[] >>
+  ‘check_all_rows_match s_in t mv = check_all_rows_match s_in (mk_substitute_tbl t x b) mv’
+    by gvs[check_all_rows_match_sub_eq] >>
+  gvs[] >>
+  metis_tac[min_idx_till_simp_eq_some]
+QED
+
+      
+      
+
+    
+Theorem prop1_mini_subcases:
+  ∀ t l s_in  x b mv.
+    ALOOKUP mv x = SOME b ∧
+    simp_table (mk_substitute_tbl t x b) (SOME s_in) = l ⇒
+    match_tbl t mv s_in = match_tbl l mv s_in
+Proof
+  rw[match_tbl_def] >>
+  
+  rpt (BasicProvers.FULL_CASE_TAC >> gvs[]) >>
+  ‘∃l. (simp_table (mk_substitute_tbl t x b) (SOME s_in)) = l’ by gvs[] >>
+  rgs[] >|[
+    
+    imp_res_tac min_idx_till_simp_sub_eq_none >> gvs[]
+    ,
+    imp_res_tac min_idx_till_simp_sub_eq_none >> gvs[] 
+    ,
+    PairCases_on ‘r’ >> PairCases_on ‘r'’ >> gvs[] >>
+    imp_res_tac min_idx_till_simp_sub_eq_some >> gvs[]
+  ]
+QED
+
+      
+
+
+
+
+        
+Triviality simp_table_final_case:
+  ∀ rows n st res.
+    simp_table rows (SOME n) = [([True],st,res)] ⇒
+    (n=st)
+Proof
+
+  Induct >>
+  rw[simp_table_def] >>
+  PairCases_on ‘h’ >>
+  gvs[simp_table_def] >>
+  rpt (BasicProvers.FULL_CASE_TAC >> gvs[])
+QED
+
+
+Triviality match_tbl_simple_final_case:
+  ∀ h1 st s_in n n' mv.
+    match_tbl [([True],st,state n)] mv s_in = SOME (state n') ⇒
+    (s_in = st ∧ n = n')
+Proof
+  rw[match_tbl_def, check_all_rows_match_def, is_match_row_def,
+       is_atoml_true_def, sem_var_atom_def, min_idx_till_def, INDEX_FIND_def] >>
+   rpt (BasicProvers.FULL_CASE_TAC >> gvs[])
+QED
+        
+
+
+
+Theorem prop1_tables_verbose:
+  ∀ tbll mv h b s_in.
+    ALOOKUP mv h = SOME b
+    ⇒
+    sem_tables (simp_tables (MAP (λt. mk_substitute_tbl t h b) tbll) (SOME s_in),s_in) mv =
+    sem_tables (tbll,s_in) mv
+Proof
+ Induct >> rw[] >-
+   (
+   gvs[simp_tables_def, match_tbll_def]
+   ) >>
+  
+
+  
+   (* we need to be able to cut the tables list into something manageble for the proof*)
+   rename1 ‘mk_substitute_tbl t x b’ >>
+
+   simp[simp_tables_def] >>
+   Cases_on ‘simp_table (mk_substitute_tbl t x b) (SOME s_in)’ >> gvs[] >|[
+
+    (*case when the whole first table is empty *)
+    gvs[sem_tables_def, match_tbll_head_empty] >>
+    Cases_on ‘tbll’ >> gvs[] >>
+    
+    simp[match_tbll_def, match_tbl_def] >>
+    imp_res_tac simp_sub_empty_then_min_index_none >>
+    gvs[min_idx_till_def, check_all_rows_match_def, INDEX_FIND_def]
+
+    ,
+
+    Cases_on ‘t'’ >> gvs[] >|[
+             
+        PairCases_on ‘h’ >> gvs[] >>
+        Cases_on ‘h0’ >> gvs[] >|[
+
+          (* case when the first table's row is empty *)
+          gvs[sem_tables_def, match_tbll_row_empty] >>
+          Cases_on ‘tbll’ >> gvs[] >>
+          
+          simp[match_tbll_def, match_tbl_def] >>
+          imp_res_tac simp_sub_empty_then_min_index_tbl_none >>
+          gvs[min_idx_till_def, check_all_rows_match_def, INDEX_FIND_def]
+          ,
+          (*case if the first table is not empty *)
+          Cases_on ‘h’ >> gvs[] >|[
+              (* case1: True case*)
+
+                 
+              (*case simplification returns True::t' *)
+              (*if t' is empty or not, as in a final table with a final row *)
+              Cases_on ‘t'’ >> gvs[simp_table_cannot_result2] >>
+                (* case final table or not*)
+              Cases_on ‘h2’ >> gvs[] >|[
+                       
+                  (*case returns action *)
+                gvs[sem_tables_def] >>
+                Cases_on ‘tbll’ >> gvs[] >|[
+                  (* case the list contains one single table *)
+                  gvs[simp_tables_def, match_tbll_def, fv_tbll_def] >>
+                  imp_res_tac prop1_mini_subcases >>
+                  gvs[]
+                  ,
+                  (*prove to be none here ... none *)
+                  gvs[sem_tables_def, simp_tables_sub_not_empty_table,
+                      match_tbll_final_before_ending_none] >>
+                  gvs[match_tbll_def] >>
+                  
+                  imp_res_tac prop1_mini_subcases >> gvs[] >>
+                  imp_res_tac simp_table_final_case >> gvs[] >>
+                  gvs[match_tbl_def, check_all_rows_match_def, is_match_row_def,
+                     is_atoml_true_def, sem_var_atom_def, min_idx_till_def, INDEX_FIND_def]
+                  ]
+                ,
+                        
+                  (* case returns state not action *)
+                  gvs[sem_tables_def] >>
+                  Cases_on ‘tbll’ >> gvs[] >|[
+                      (* trivial case *)
+                      gvs[simp_tables_def, match_tbll_def, fv_tbll_def] >>
+                      imp_res_tac prop1_mini_subcases >>
+                      gvs[]
+                      ,
+                      gvs[match_tbll_def] >>
+                      (* prove for head, then use IH *)
+                      Cases_on ‘simp_tables
+                                (mk_substitute_tbl h x b::MAP (λt. mk_substitute_tbl t x b) t')
+                                (SOME n)’ >> gvs[] >>
+                      gvs[simp_tables_sub_not_empty_table] >>
+                      gvs[match_tbll_def] >>
+                      
+                      gvs[simp_tables_sub_not_empty_table] >>
+                      imp_res_tac prop1_mini_subcases >>
+                      gvs[] >>
+                      
+                      Cases_on ‘match_tbl [([True],h1,state n)] mv s_in’ >> gvs[] >>
+                      Cases_on ‘x'’ >> gvs[] >|[
+                          
+                          gvs[match_tbl_def, check_all_rows_match_def, is_match_row_def,
+                              is_atoml_true_def, sem_var_atom_def, min_idx_till_def, INDEX_FIND_def] >>
+                          rpt (BasicProvers.FULL_CASE_TAC >> gvs[])
+                          ,
+                          
+                          imp_res_tac match_tbl_simple_final_case >> gvs[] >>
+                          res_tac >>
+                          first_x_assum (strip_assume_tac o (Q.SPECL [‘n’])) >>
+                          
+                          Cases_on ‘simp_tables
+                                    (mk_substitute_tbl h x b::MAP (λt. mk_substitute_tbl t x b) t')
+                                    (SOME n)’ >> gvs[] >>
+                          gvs[ match_tbll_def]
+                             
+                          ,
+                          
+                          
+                          imp_res_tac match_tbl_simple_final_case >> gvs[] >>
+                          res_tac >>
+                          first_x_assum (strip_assume_tac o (Q.SPECL [‘n’])) >>
+                          metis_tac[]
+                        ]
+                  ]
+              ]
+                                       
+              (* end of true case *)
+              ,
+              (* case 2: False case *)
+              gvs[simp_table_impossible_case2]
+              ,
+              (* case 3: NotTrue case *)
+              gvs[simp_table_impossible_case3]
+              ,
+              (* case 4: NotFalse case *)
+              gvs[simp_table_impossible_case3]
+              ,
+              (* case 5: Var *)
+              Cases_on ‘tbll’ >> gvs[] >>
+              gvs[sem_tables_def, match_tbll_def] >|[
+                  gvs[simp_tables_def, match_tbll_def, fv_tbll_def] >>
+                  imp_res_tac prop1_mini_subcases >>
+                  gvs[]
+                  ,
+                        
+                  Cases_on ‘simp_tables
+                            (mk_substitute_tbl h x b::MAP (λt. mk_substitute_tbl t x b) t'') NONE’ >> gvs[] >>
+                                  
+                  gvs[match_tbll_def] >>
+                  gvs[simp_tables_sub_not_empty_table] >>
+                  imp_res_tac prop1_mini_subcases >>
+                  gvs[] >>
+                  Cases_on ‘match_tbl [(Var s::t',h1,h2)] mv s_in’ >> gvs[] >>
+                  Cases_on ‘x'’ >> gvs[] >>
+                  res_tac >>
+                  first_x_assum (strip_assume_tac o (Q.SPECL [‘n’])) >>
+
+                  ‘match_tbll
+                   (simp_tables (mk_substitute_tbl h x b::MAP (λt. mk_substitute_tbl t x b) t'')
+                    (SOME n)) mv n
+                   =
+                   match_tbll
+                   (simp_tables (mk_substitute_tbl h x b::MAP (λt. mk_substitute_tbl t x b) t'')
+                    NONE) mv n ’
+                    by gvs[match_tbll_simp_tables_eq_thm] >>
+                  gvs[]
+                ]
+
+              ,
+              (* case 6: Not *)
+              Cases_on ‘tbll’ >> gvs[] >>
+              gvs[sem_tables_def, match_tbll_def] >|[
+                  gvs[simp_tables_def, match_tbll_def, fv_tbll_def] >>
+                  imp_res_tac prop1_mini_subcases >>
+                  gvs[]
+                  ,
+                  Cases_on ‘simp_tables
+                            (mk_substitute_tbl h x b::MAP (λt. mk_substitute_tbl t x b) t'') NONE’ >> gvs[] >>
+                  gvs[simp_tables_sub_not_empty_table] >>
+                  gvs[match_tbll_def] >>
+
+                  gvs[simp_tables_sub_not_empty_table] >>
+                  imp_res_tac prop1_mini_subcases >>
+                  gvs[] >>
+
+                  Cases_on ‘match_tbl [(Not s::t',h1,h2)] mv s_in’ >> gvs[] >>
+                  Cases_on ‘x'’ >> gvs[] >>
+                  res_tac >>
+                  first_x_assum (strip_assume_tac o (Q.SPECL [‘n’])) >>
+                  
+                  ‘match_tbll
+                   (simp_tables (mk_substitute_tbl h x b::MAP (λt. mk_substitute_tbl t x b) t'')
+                                    (SOME n)) mv n
+                   =
+                   match_tbll
+                   (simp_tables (mk_substitute_tbl h x b::MAP (λt. mk_substitute_tbl t x b) t'')
+                                    NONE) mv n ’
+                    by gvs[match_tbll_simp_tables_eq_thm] >>
+                  gvs[]
+                ]
+            ]
+        ]
+        ,
+        (*IH case*)
+        Cases_on ‘tbll’ >> gvs[] >>
+        gvs[sem_tables_def, match_tbll_def] >|[
+            simp[simp_tables_def,  match_tbll_def] >>
+            imp_res_tac prop1_mini_subcases >>
+            gvs[]
+            ,
+            Cases_on ‘simp_tables
+               (mk_substitute_tbl h'' x b::
+                                  MAP (λt. mk_substitute_tbl t x b) t') NONE’ >>
+            gvs[simp_tables_sub_not_empty_table] >>
+
+            rename1 ‘match_tbll ((r1::r2::r3)::tbl2::tbl3) mv s_in’ >>
+                                                 
+            simp[match_tbll_def] >>
+            ‘match_tbl (r1::r2::r3) mv s_in = match_tbl t mv s_in’ by (
+              imp_res_tac prop1_mini_subcases >>
+              gvs[]) >>
+            gvs[] >>
+
+            rpt (BasicProvers.FULL_CASE_TAC >> gvs[]) >>
+            res_tac >>
+            first_x_assum (strip_assume_tac o (Q.SPECL [‘n’])) >>
 
                           
+            ‘match_tbll
+          (simp_tables
+             (mk_substitute_tbl h'' x b::MAP (λt. mk_substitute_tbl t x b) t')
+             (SOME n)) mv n
+             =
+             match_tbll
+          (simp_tables
+             (mk_substitute_tbl h'' x b::MAP (λt. mk_substitute_tbl t x b) t')
+             NONE) mv n ’
+              by gvs[match_tbll_simp_tables_eq_thm] >>
+            
+            gvs[]
+
+          ]
+      ]
+  ]
+QED
+
+
+
+
                
 Theorem prop1_var_tables:
   prop1 table_structure
@@ -936,458 +2240,140 @@ Proof
   Cases_on ‘p’ >>
   rename1 ‘(tbls, s_in)’ >>
 
-  gvs[fv_tables_def, mk_substitute_tables_def, simp_tables_def] >>
-  imp_res_tac prop1_var_tables_verbose >> gvs[]    
+  gvs[mk_substitute_tables_def, simp_tables_def, simp_tables_wrapper_def] >>
+  gvs[mk_substitute_tbll_def] >>
+  gvs[prop1_tables_verbose]
 QED
 
 
-Theorem is_hit_true_atoml_not_empty:
-  ∀ atoml h' b s_in st_num.        
-    is_hit s_in st_num (simp_row (mk_substitute_row atoml h' b)) ⇒
-    atoml ≠ []
+
+
+(*******************************************)
+(*                property 2               *)
+(*******************************************)
+
+
+Theorem final_row_final_result:
+  ∀ atoms_list st res s_in q.
+    final_row (atoms_list,st,res) s_in = SOME q ⇒
+    (atoms_list = [True] ∧ st = s_in ∧ q = res)
 Proof
-  gvs[is_hit_def, all_true_def, mk_substitute_row_def, simp_row_def]
+  Cases >> rw[final_row_def] >>
+  Cases_on ‘t’ >> gvs[] >>
+  Cases_on ‘h’ >> gvs[final_row_def]
 QED
 
 
-
-                         
-Theorem hit_implies_match_after_subst:
-  ∀ atoml s_in st_num h' b mv.
-    ALOOKUP mv h' = SOME b ∧
-    is_hit s_in st_num (simp_row (mk_substitute_row atoml h' b)) ⇒
-    is_match_row s_in st_num atoml mv
-Proof
-  Induct_on ‘atoml’ >>
-  rpt strip_tac >>
-  imp_res_tac is_hit_true_atoml_not_empty >>               
-  gvs[is_hit_def, is_match_row_def] >>
-  gvs[is_atoml_true_def, mk_substitute_row_def, simp_row_def, all_true_def] >>
-  res_tac >>
-          
-  rpt (BasicProvers.FULL_CASE_TAC >> gvs[]) >>
-  gvs[sem_var_atom_def] >>
-
-          
-  Cases_on ‘atoml=[]’ >> gvs[] >>
-  imp_res_tac subst_simp_sound_for_atom      
-QED
 
 
         
         
-Theorem row_miss_preserved_by_subst_simp:
-  ∀ tbl s_in h' b mv.
-    ALOOKUP mv h' = SOME b ∧
-    EVERY ($¬ ∘ (λ(p,a). p)) (MAP (λ(atoml,st_num,res). (is_match_row s_in st_num atoml mv,res)) tbl)
-    ⇒
-    ¬ EXISTS (λx. (λ(p,a). p) ((λ(atoml,st_num,res). (is_hit s_in st_num atoml,st_num,res))
-                               ((λ(atoml,st_num,res). (simp_row atoml,st_num,res))
-                                ((λ(atoml,st_num,res). (mk_substitute_row atoml h' b,st_num,res)) x)))) tbl
-Proof
-Induct >> gvs[] >>                  
-rpt strip_tac >>
-PairCases_on ‘h’ >> gvs[] >>
-imp_res_tac hit_implies_match_after_subst >>
-res_tac
-QED
 
-
-
-Theorem pre_lines_are_fail_normalize:
-  ∀ l h idx st_num.
-    idx > 0 ∧
-    idx < LENGTH (h::l) ∧
-    pre_lines_are_fail (h::l) idx st_num ⇒
-    pre_lines_are_fail l (idx-1) st_num
-Proof
-  rpt strip_tac >>
-  gvs[pre_lines_are_fail_def] >>
-  imp_res_tac every_seg_property_1 >>
-  Cases_on ‘idx’ >> gvs[SUC_ADD_ONE] >>
-  res_tac >>
-  imp_res_tac every_seg_property_1 >>
-  ‘n < LENGTH l’ by gvs[] >>
-  gvs[]
-QED
-
-
-
-       
-Theorem index_find_not_prev:
-  ∀ l P r.         
-    INDEX_FIND 1 P l ≠ SOME (0,r)            
-Proof
-  Induct >> gvs[INDEX_FIND_def] >>
-  rpt strip_tac >>
-  rpt (BasicProvers.FULL_CASE_TAC >> gvs[]) >>
-  assume_tac P_hold_on_next >>
-  first_x_assum (strip_assume_tac o (Q.SPECL [‘(1:num)’, ‘l’, ‘P’, ‘(0,r)’])) >>
-  gvs[SUC_ADD_ONE]
-QED
-                          
-        
-
-Theorem index_find_not_prev_gen:
-  ∀ i l P r .
-    i > 1 ∧
-    0 < LENGTH l ⇒
-    INDEX_FIND i P l ≠ SOME (i-1,r)
-Proof
-  Induct >> gvs[INDEX_FIND_def] >>
-  rpt strip_tac >>
-  rpt (BasicProvers.FULL_CASE_TAC >> gvs[]) >>
-  assume_tac P_hold_on_next >> 
-  first_x_assum (strip_assume_tac o (Q.SPECL [‘(i:num)’, ‘l’, ‘P’, ‘(i,r)’])) >>
-  gvs[SUC_ADD_ONE] >>
-
-  Cases_on ‘i > 1’ >> gvs[] >>
-  Cases_on ‘i=1’ >> gvs[] >>
-  imp_res_tac index_find_not_prev      
-QED
-
-
-
-
-
-Theorem every_seg_property_3:         
-  ∀ n l h p.
-    0 < n ∧
-    EVERY p (SEG n 0 (h::l)) ⇒
-    EVERY p (SEG (n-1) 0 l)
-Proof
-  Induct >>
-  rpt strip_tac >>
-  gvs[SEG, SUC_ADD_ONE] >>
-  gvs[GSYM TAKE_SEG]
-QED
-        
-                        
-        
-Theorem every_simp_false_imp_sem_false:
-  ∀ atoml h' b mv.
-    atoml ≠ [] ∧
-    ALOOKUP mv h' = SOME b ∧
-    EVERY (λatom. atom = False) (simp_row (mk_substitute_row atoml h' b)) ⇒
-    ~ EVERY (λminipred. sem_var_atom minipred mv = SOME T) atoml
+Theorem property_final_imp_match_simp:
+  ∀ tbl s_in q mv.
+    final_tbl tbl s_in = SOME q ⇒
+    match_tbl tbl mv s_in = SOME q
 Proof
   Induct >-
-   gvs[mk_substitute_row_def, simp_row_def] >>
-  rpt strip_tac >>
+   gvs[final_tbl_def] >>
+  rw[] >>
   
-  Cases_on ‘atoml=[]’ >> gvs[] >| [
-    gvs[EVERY_MEM] >>
-    gvs[mk_substitute_row_def, simp_row_def] >>
-    rpt (BasicProvers.FULL_CASE_TAC >> gvs[]) >>
-    imp_res_tac subst_simp_sound_for_atom >> gvs[]
+  PairCases_on ‘h’ >>
+  rename1 ‘((atoms_list,st,res)::t)’ >>
+  
+  gvs[final_tbl_def] >>
+  rpt (BasicProvers.FULL_CASE_TAC >> gvs[]) >|[
+    
+    gvs[match_tbl_def] >>
+    res_tac >>
+    first_x_assum (strip_assume_tac o (Q.SPECL [‘mv’])) >>
+    
+    Cases_on ‘min_idx_till (check_all_rows_match s_in t mv) T’ >> gvs[] >>
+    PairCases_on ‘x’ >> gvs[] >>
+    
+    Cases_on ‘min_idx_till (check_all_rows_match s_in (([False],st,res)::t) mv) T’ >>
+    
+    (gvs[check_all_rows_match_def, is_match_row_def, is_atoml_true_def, sem_var_atom_def] >>
+     gvs[min_idx_till_def, INDEX_FIND_def] >>
+     imp_res_tac P_NONE_hold2 >> gvs[]) >>
+    
+    Cases_on ‘x’ >> gvs[] >>
+    Cases_on ‘r’ >> gvs[] >>    
+    imp_res_tac INDEX_FIND_some_eq_next >> gvs[]
     ,
-
-    rgs[Once mk_substitute_row_def, Once simp_row_def] >>
-    rpt (BasicProvers.FULL_CASE_TAC >> gvs[]) >|[
-        imp_res_tac subst_simp_sound_for_atom >> gvs[]
-        ,
-        gvs[EVERY_MAP] >>
-        imp_res_tac sem_var_atom_failure_from_simp_atom_false
-      ]
+    
+    gvs[final_row_def]
+    ,
+    
+    imp_res_tac final_row_final_result >> gvs[] >>
+    gvs[final_row_def, match_tbl_def] >>
+    gvs[check_all_rows_match_def, is_match_row_def, is_atoml_true_def, sem_var_atom_def] >>
+    gvs[min_idx_till_def, INDEX_FIND_def]
   ]
 QED
 
 
-    
 
-Theorem subst_simp_miss_implies_sem_miss:
-  ∀ atoml h' b mv st_num s_in. 
-    ALOOKUP mv h' = SOME b ∧
-    ¬is_hit s_in st_num (simp_row (mk_substitute_row atoml h' b)) ∧
-    all_false (simp_row (mk_substitute_row atoml h' b)) ⇒
-    ¬is_match_row s_in st_num atoml mv
+
+   
+        
+Theorem property_final_imp_sem_tbll_simp:
+  ∀ tbll mv q s_in.
+    final_tables (tbll,s_in) = SOME q
+    ⇒
+    sem_tables (tbll,s_in) mv = SOME q
 Proof
-  rpt strip_tac >>                   
-  gvs[all_false_def, is_match_row_def, is_hit_def] >>
-  gvs[is_atoml_true_def] >-
-   imp_res_tac every_simp_false_imp_sem_false >>
-  gvs[mk_substitute_row_def, simp_row_def] >>
-  rpt (BasicProvers.FULL_CASE_TAC >> gvs[])
-QED
-
-
-
-
-        
-Theorem index_find_agreement_under_subst_and_all_false_prefix:       
-∀ tbl (s_in:num) n st_num st_num' res q (res':'a action_expr) h' b mv.
-  ALOOKUP mv h' = SOME b ∧
-EVERY (λ(atoml,st_num',res'). st_num' = s_in ⇒ all_false atoml)
-               (SEG n 0
-                  (MAP
-                     ((λ(atoml,st_num,res). (simp_row atoml,st_num,res)) ∘
-                      (λ(atoml,st_num,res).
-                           (mk_substitute_row atoml h' b,st_num,res))) tbl)) ∧
-INDEX_FIND 0 (λ(p,a). p)
-               (MAP
-                  (λ(atoml,st_num,res).
-                       (is_match_row s_in st_num atoml mv,res)) tbl) =
-             SOME (q − 1,T,res') ∧
-INDEX_FIND 0 (λ(p,a). p)
-               (MAP
-                  ((λ(atoml,st_num,res).
-                        (is_hit s_in st_num atoml,st_num,res)) ∘
-                   (λ(atoml,st_num,res). (simp_row atoml,st_num,res)) ∘
-                   (λ(atoml,st_num,res).
-                        (mk_substitute_row atoml h' b,st_num,res))) tbl) =
-             SOME (n,T,st_num,res) ⇒
-res=res'
-Proof
-
-Induct >|[
-    gvs[INDEX_FIND_def]
+  Induct >>
+  rw[sem_tables_def] >|[
+    gvs[final_tables_def, simp_tables_def, final_tbll_def]
     ,
-    rpt strip_tac >>
-    PairCases_on ‘h’ >>
-    gvs[INDEX_FIND_def] >>
-    rpt (BasicProvers.FULL_CASE_TAC >> gvs[]) >|[
-                                    
-        imp_res_tac hit_implies_match_after_subst
-        ,
-        Cases_on ‘h1 = s_in’ >|[
-              Cases_on ‘q=0’ >> gvs[] >|[
-                Cases_on ‘n’ >>
-                gvs[SEG, SUC_ADD_ONE] >>
-                gvs[GSYM TAKE_SEG] >>
-                gvs[index_find_not_prev] >>
-                imp_res_tac subst_simp_miss_implies_sem_miss
-                ,
-                ‘q=1’ by gvs[] >>
-                gvs[] >>
-                Cases_on ‘n’ >>
-                gvs[SEG, SUC_ADD_ONE] >>
-                gvs[GSYM TAKE_SEG] >>
-                gvs[index_find_not_prev] >>
-                imp_res_tac subst_simp_miss_implies_sem_miss
-              ]                                       
-                                                
-            ,
-            gvs[is_hit_def, is_match_row_def]
-          ]
-                                        
+    Cases_on ‘tbll’ >> gvs[] >|[
+
+        gvs[final_tables_def, match_tbll_def, final_tbll_def] >>
+        rpt (BasicProvers.FULL_CASE_TAC >> gvs[]) >>
+
+        imp_res_tac property_final_imp_match_simp >>
+        first_x_assum (strip_assume_tac o (Q.SPECL [‘mv’])) >>
+        Cases_on ‘match_tbl h mv s_in’ >> gvs[]                    
         ,
         
-        
-        assume_tac (INST_TYPE [“:'a” |-> “:(bool # 'a action_expr)”,
-                               “:'b” |-> “:num”] P_hold_on_next)  >>
-        first_x_assum (strip_assume_tac o (Q.SPECL [‘0’,
-         ‘(MAP (λ(atoml,st_num,res). (is_match_row (s_in:num) st_num atoml mv,res)) tbl)’,
-         ‘(λ(p,a). p)’, ‘(q − 1,T,(res':α action_expr))’])) >>
+        gvs[final_tables_def, match_tbll_def, final_tbll_def] >>
+        Cases_on ‘final_tbl h s_in’ >> gvs[] >>
+        Cases_on ‘x’ >> gvs[] >>
+                
+        imp_res_tac property_final_imp_match_simp >>
+        first_x_assum (strip_assume_tac o (Q.SPECL [‘mv’])) >>
         gvs[] >>
-
-
-
-
-        
-        assume_tac (INST_TYPE [“:'a” |-> “:(bool # num # 'a action_expr)”] P_hold_on_next)  >>
-        first_x_assum (strip_assume_tac o (Q.SPECL [‘0’,
-         ‘(MAP ((λ(atoml,st_num,res). (is_hit s_in st_num atoml,st_num,res)) ∘
-                (λ(atoml,st_num,res). (simp_row atoml,st_num,res)) ∘
-                (λ(atoml,st_num,res). (mk_substitute_row atoml h' b,st_num,res))) tbl)’,
-         ‘(λ(p,a). p)’, ‘(n,T,st_num,res)’])) >>
-        gvs[] >>
-
-
-
-        imp_res_tac every_seg_property_3 >>
-        last_x_assum (strip_assume_tac o (Q.SPECL [‘s_in’, ‘n-1’, ‘st_num’, ‘res’,
-                                                   ‘q-1’ ,‘res'’, ‘h'’, ‘b’, ‘mv’])) >>
-        gvs[]    
+              
+        res_tac >>
+        gvs[sem_tables_def]
       ]
-]
+  ] 
 QED
 
 
 
 
-                           
-    
-
-    
-Theorem prop2_var_single_tbl_verbose:
-  ∀ tbl mv h' b res s_in.
-    ALOOKUP mv h' = SOME b ∧
-    final_tbl (simp_tbl (mk_substitute_tbl tbl h' b)) s_in = SOME res ⇒
-    match_tbl tbl mv s_in = SOME res
-Proof       
-  
-  Cases_on ‘tbl’ >| [
-    gvs[fv_tbl_def, mk_substitute_tbl_def, simp_tbl_def, final_tbl_def,
-        min_idx_till_def, is_hit_tbl_check_def, INDEX_FIND_def]
-    ,
-    rpt strip_tac >>
-    gvs[mk_substitute_tbl_def, simp_tbl_def, final_tbl_def] >>
-    gvs[match_tbl_def] >>
-    rpt (BasicProvers.FULL_CASE_TAC >> gvs[]) >>
-    
-    rename1 ‘(idx,bool,st_num,res)’ >>
-    PairCases_on ‘h’ >>
-    gvs[is_hit_tbl_check_def, check_all_rows_match_def] >>
-    gvs[min_idx_till_def] >|[
-        
-        
-        gvs[INDEX_FIND_def] >>
-        rpt (BasicProvers.FULL_CASE_TAC >> gvs[])  >|[
-          imp_res_tac hit_implies_match_after_subst
-          ,
-          imp_res_tac INDEX_FIND_NONE_EXISTS >>
-          imp_res_tac exists_index_some >>
-          gvs[EXISTS_MAP] >>
-          gvs[MAP_MAP_o] >>
-          imp_res_tac row_miss_preserved_by_subst_simp
-        ]
-        ,
-        
-        
-        gvs[INDEX_FIND_def] >>
-        rpt (BasicProvers.FULL_CASE_TAC >> gvs[]) >|[
-            imp_res_tac hit_implies_match_after_subst
-            ,
-            
-            gvs[pre_lines_are_fail_def] >>
-            Cases_on ‘idx’ >>
-            gvs[SEG, SUC_ADD_ONE] >>
-            gvs[GSYM TAKE_SEG] >| [
-                gvs[index_find_not_prev]
-                ,
-                Cases_on ‘h1 = s_in’ >|[
-                    imp_res_tac subst_simp_miss_implies_sem_miss >>
-                    gvs[]
-                    ,
-                    gvs[is_hit_def, is_match_row_def]
-                  ]
-              ]
-            ,
-
-
-            gvs[pre_lines_are_fail_def] >>
-            Cases_on ‘idx’ >>
-            gvs[SEG, SUC_ADD_ONE] >>
-            gvs[GSYM TAKE_SEG] >>
-            gvs[index_find_not_prev] >>
-            PairCases_on ‘r’ >> gvs[] >>
-            
-            Cases_on ‘h1=s_in’ >|[
-                
-                
-                assume_tac (INST_TYPE [“:'a” |-> “:(bool # 'a action_expr)”,
-                                       “:'b” |-> “:num”] P_hold_on_next)  >>
-                first_x_assum (strip_assume_tac o (Q.SPECL [‘0’,
-                               ‘(MAP (λ(atoml,st_num,res). (is_match_row (h1:num) st_num atoml mv,res)) t)’,
-                               ‘(λ(p,a). p)’, ‘(q,r0,r1)’])) >>
-                gvs[] >>
-                
-                assume_tac (INST_TYPE [“:'a” |-> “:(bool # num # 'a action_expr)”] P_hold_on_next)  >>
-                first_x_assum (strip_assume_tac o (Q.SPECL [‘0’,
-                               ‘(MAP (λ(atoml,st_num,res). (is_hit h1 st_num atoml,st_num,res))
-                                (MAP (λ(atoml,st_num,res). (simp_row atoml,st_num,res))
-                                (MAP (λ(atoml,st_num,res). (mk_substitute_row atoml h' b,st_num,res)) t)))’,
-                               ‘(λ(p,a). p)’, ‘(n + 1,bool,st_num,res)’])) >>
-
-
-                gvs[] >>
-                
-                
-                ‘(λ(p,a). p) (bool,st_num,res)’ by imp_res_tac INDEX_FIND_EQ_SOME_0 >>
-                ‘(λ(p,a). p) (r0,r1)’ by imp_res_tac INDEX_FIND_EQ_SOME_0 >>
-                
-                gvs[] >>
-                
-                
-                gvs[MAP_MAP_o] >>
-                imp_res_tac index_find_agreement_under_subst_and_all_false_prefix >>
-                gvs[]
-                   
-                ,
-                
-                assume_tac (INST_TYPE [“:'a” |-> “:(bool # 'a action_expr)”,
-                                       “:'b” |-> “:num”] P_hold_on_next)  >>
-                first_x_assum (strip_assume_tac o (Q.SPECL [‘0’,
-                               ‘(MAP (λ(atoml,st_num,res). (is_match_row (s_in:num) st_num atoml mv,res)) t)’,
-                               ‘(λ(p,a). p)’, ‘(q,r0,r1)’])) >>
-                gvs[] >>
-                
-                assume_tac (INST_TYPE [“:'a” |-> “:(bool # num # 'a action_expr)”] P_hold_on_next)  >>
-                first_x_assum (strip_assume_tac o (Q.SPECL [‘0’,
-                           ‘(MAP (λ(atoml,st_num,res). (is_hit s_in st_num atoml,st_num,res))
-                            (MAP (λ(atoml,st_num,res). (simp_row atoml,st_num,res))
-                            (MAP (λ(atoml,st_num,res). (mk_substitute_row atoml h' b,st_num,res)) t)))’,
-                           ‘(λ(p,a). p)’, ‘(n + 1,bool,st_num,res)’])) >>
-
-
-                gvs[] >>
-          
-          
-                ‘(λ(p,a). p) (bool,st_num,res)’ by imp_res_tac INDEX_FIND_EQ_SOME_0 >>
-                ‘(λ(p,a). p) (r0,r1)’ by imp_res_tac INDEX_FIND_EQ_SOME_0 >>
-                
-                gvs[] >>
-                
-                
-                gvs[MAP_MAP_o] >>
-                imp_res_tac index_find_agreement_under_subst_and_all_false_prefix >>
-                gvs[]
-              ] 
-          ]
-      ]
-  ]         
-QED
-
-
-
-
-        
 
 Theorem prop2_var_tables_verbose:
-  ∀ tbls h b mv s_in res.
+  ∀ tbll mv s_in h b q.
     ALOOKUP mv h = SOME b ∧
-    final_tbll (simp_tbll (mk_substitute_tbll tbls h b)) s_in = SOME res ⇒
-    sem_tables (tbls,s_in) mv = SOME res 
+    final_tables (simp_tables (MAP (λtbl. mk_substitute_tbl tbl h b) tbll) (SOME s_in),s_in)
+    = SOME q ⇒
+    sem_tables (tbll,s_in) mv = SOME q
 Proof
-
-  Induct_on ‘tbls’ >> rpt strip_tac >-
-   gvs[mk_substitute_tbll_def, simp_tbll_def, final_tbll_def] >> 
-  rename1 ‘(tbl::tbll)’ >>
-
-
-  Cases_on ‘tbll’ >> gvs[] >|[
-    
-    gvs[sem_tables_def, match_tbll_def] >>
-    gvs[mk_substitute_tbll_def, simp_tbll_def, final_tbll_def] >>
-    gvs[] >>
-    rpt (BasicProvers.FULL_CASE_TAC >> gvs[]) >>
-    
-    imp_res_tac prop2_var_single_tbl_verbose >> gvs[]              
-    ,
-    rename1 ‘(tbl::nexttbl::tbll)’ >>
-    rgs[Once mk_substitute_tbll_def, Once simp_tbll_def] >>
-    rgs[Once final_tbll_def] >>     
-
-    Cases_on ‘final_tbl (simp_tbl (mk_substitute_tbl tbl h' b)) s_in’ >>
-    gvs[] >>
-    Cases_on ‘x’ >>
-    gvs[] >>
-    
-    rgs[Once mk_substitute_tbll_def, Once simp_tbll_def] >>
-    rgs[Once final_tbll_def] >>  
-    res_tac >>
-
-    gvs[sem_tables_def, match_tbll_def] >>
-    gvs[mk_substitute_tbll_def, simp_tbll_def, final_tbll_def] >>
-    gvs[] >>
-    rpt (BasicProvers.FULL_CASE_TAC >> gvs[]) >>
-    
-    imp_res_tac prop2_var_single_tbl_verbose >> gvs[]     
-  ]
+  rw[] >>
+  imp_res_tac property_final_imp_sem_tbll_simp >>
+  first_x_assum (strip_assume_tac o (Q.SPECL [‘mv’])) >>
+  
+  imp_res_tac prop1_tables_verbose >>
+  first_x_assum (strip_assume_tac o (Q.SPECL [‘tbll’,‘s_in’])) >>
+  metis_tac[]
 QED
 
+        
 
-
+         
 Theorem prop2_var_tables:
   prop2 table_structure
 Proof
@@ -1397,160 +2383,14 @@ Proof
   Cases_on ‘p’ >>
   rename1 ‘(tbls, s_in)’ >>
 
-  gvs[final_tables_def, fv_tables_def, mk_substitute_tables_def, simp_tables_def] >>
-  imp_res_tac prop1_var_tables_verbose >> gvs[] >>
-  imp_res_tac prop2_var_tables_verbose >> gvs[]
-QED
-
-
-                   
-Theorem hit_implies_match_after_all:
-  ∀ atoml s_in st_num h' b mv.
-    is_hit s_in st_num atoml ⇒
-    is_match_row s_in st_num atoml mv
-Proof
-  Induct_on ‘atoml’ >>
-  rpt strip_tac >>
-  gvs[is_hit_def, is_match_row_def] >>
-  gvs[is_atoml_true_def,all_true_def] >>
-  res_tac >>
-  Cases_on ‘atoml=[]’ >>
-  gvs[sem_var_atom_def]
+  gvs[mk_substitute_tables_def, simp_tables_def, simp_tables_wrapper_def] >>
+  gvs[mk_substitute_tbll_def] >>
+  metis_tac[prop2_var_tables_verbose]
 QED
 
 
 
-Theorem subst_simp_miss_implies_sem_miss_full:
-  ∀ atoml h' b mv s_in st_num .
-    ¬is_hit s_in st_num (simp_row (mk_substitute_row atoml h' b)) ∧
-    all_false (simp_row (mk_substitute_row atoml h' b)) ⇒
-    ¬is_match_row s_in st_num  (simp_row (mk_substitute_row atoml h' b)) mv
-Proof
-  Induct >>
-  rpt strip_tac >>                   
-  gvs[all_false_def, is_match_row_def, is_hit_def] >>
-  gvs[is_atoml_true_def, all_true_def] >>
-  gvs[mk_substitute_row_def, simp_row_def] >>
-  res_tac >>
-  rpt (BasicProvers.FULL_CASE_TAC >> gvs[]) >>
-  gvs[mk_substitute_row_def, simp_row_def, sem_var_atom_def]
-QED
-
-
-
-        
-
-Theorem match_follows_hit_at_minimal_index:
-  ∀ tbl s_in idx  bool  st_num res mv h' b.
-    pre_lines_are_fail (simp_tbl (mk_substitute_tbl tbl h' b)) idx s_in ∧
-    min_idx_till (is_hit_tbl_check (simp_tbl (mk_substitute_tbl tbl h' b)) s_in) T =
-    SOME (idx,bool,st_num,res)  ⇒
-    min_idx_till (check_all_rows_match s_in (simp_tbl (mk_substitute_tbl tbl h' b)) mv) T =
-    SOME (idx,bool,res)
-Proof
-  gvs[min_idx_till_def] >>
-  Induct >>
-  rpt strip_tac >-
-   gvs[mk_substitute_tbl_def, check_all_rows_match_def, simp_tbl_def,
-       is_hit_tbl_check_def, INDEX_FIND_def] >>
-  
-  
-  PairCases_on ‘h’ >>
-  gvs[simp_tbl_def, mk_substitute_tbl_def, is_hit_tbl_check_def] >>
-  gvs[INDEX_FIND_def]>>
-  rpt (BasicProvers.FULL_CASE_TAC >> gvs[]) >|[
-    
-    gvs[check_all_rows_match_def, INDEX_FIND_def] >>
-    rpt (BasicProvers.FULL_CASE_TAC >> gvs[])>>
-    imp_res_tac hit_implies_match_after_all >>
-    gvs[]
-    ,
-
-    gvs[check_all_rows_match_def, INDEX_FIND_def]>>
-    rpt (BasicProvers.FULL_CASE_TAC >> gvs[]) >|[
-
-        gvs[pre_lines_are_fail_def] >>
-        Cases_on ‘idx’ >>
-        gvs[SEG, SUC_ADD_ONE] >>
-        gvs[GSYM TAKE_SEG] >>
-        gvs[index_find_not_prev] >>
-                                 
-        Cases_on ‘h1 = s_in’ >> gvs[] >>
-        imp_res_tac subst_simp_miss_implies_sem_miss_full >> gvs[is_hit_def, is_match_row_def]
-                                                                    
-        ,
-        gvs[MAP_MAP_o] >>
-        gvs[pre_lines_are_fail_def] >>
-        Cases_on ‘idx’ >>
-        gvs[SEG, SUC_ADD_ONE] >>
-        gvs[GSYM TAKE_SEG] >>
-        gvs[index_find_not_prev] >>
-        
-        
-        
-        assume_tac (INST_TYPE [“:'a” |-> “:(bool # num # 'a action_expr)”] P_hold_on_next)  >>
-        first_x_assum (strip_assume_tac o (Q.SPECL [‘0’,
-            ‘(MAP ((λ(atoml,st_num,res). (is_hit s_in st_num atoml,st_num,res)) ∘
-              (λ(atoml,st_num,res). (simp_row atoml,st_num,res)) ∘
-              (λ(atoml,st_num,res). (mk_substitute_row atoml h' b,st_num,res))) tbl)’,
-            ‘(λ(p,a). p)’, ‘(n + 1,bool,st_num,res)’])) >>
-          gvs[] >>
-          
-        
-        res_tac >>
-        first_x_assum (strip_assume_tac o (Q.SPECL [‘mv’])) >>
-        drule P_implies_next >>
-        gvs[]
-  ] 
-]
-QED
-
-
-        
-
-Theorem final_tbl_yields_match_tbl:      
-  ∀ tbl s_in mv res h' b.
-    final_tbl (simp_tbl (mk_substitute_tbl tbl h' b)) s_in = SOME res ⇒
-    match_tbl (simp_tbl (mk_substitute_tbl tbl h' b)) mv s_in = SOME res
-Proof
-  rpt strip_tac >>
-  gvs[final_tbl_def, match_tbl_def] >>
-  rpt (BasicProvers.FULL_CASE_TAC >> gvs[]) >>
-  imp_res_tac match_follows_hit_at_minimal_index >> gvs[]
-QED
-
-
-Theorem final_tbll_yields_match_tbll:                            
-  ∀ tbll s_in h b mv q .
-    final_tbll (simp_tbll (mk_substitute_tbll tbll h b)) s_in = SOME q ⇒
-    match_tbll (simp_tbll (mk_substitute_tbll tbll h b))  mv s_in = SOME q
-Proof
-
-  Induct >-
-   (gvs[mk_substitute_tbll_def, simp_tbll_def, final_tbll_def]) >>
-  
-  
-  rpt strip_tac >>
-  Cases_on ‘tbll’ >|[
-    simp[match_tbll_def] >>
-    gvs[mk_substitute_tbll_def, simp_tbll_def, final_tbll_def] >>
-    rpt (BasicProvers.FULL_CASE_TAC >> gvs[]) >>
-    imp_res_tac final_tbl_yields_match_tbl >> gvs[match_tbll_def]
-    ,
-    
-    gvs[mk_substitute_tbll_def, simp_tbll_def, final_tbll_def] >>
-    rpt (BasicProvers.FULL_CASE_TAC >> gvs[]) >>
-    res_tac >>
-    
-    gvs[match_tbll_def] >>
-    rpt (BasicProvers.FULL_CASE_TAC >> gvs[]) >>
-    imp_res_tac final_tbl_yields_match_tbl >> gvs[match_tbll_def]
-  ]
-QED
-
-
-
-
+         
 Theorem prop3_var_tables:
   prop3 table_structure
 Proof
@@ -1559,97 +2399,221 @@ Proof
   rpt strip_tac >>
   Cases_on ‘p’ >>
   rename1 ‘(tbls, s_in)’ >>
-  gvs[final_tables_def, simp_tables_def, mk_substitute_tables_def, sem_tables_def] >>
-  imp_res_tac final_tbll_yields_match_tbll >> gvs[]
+
+  gvs[mk_substitute_tables_def, simp_tables_def, simp_tables_wrapper_def] >>
+  gvs[mk_substitute_tbll_def] >>
+  metis_tac[property_final_imp_sem_tbll_simp]
 QED
 
-
-
-
-
-
-Theorem fv_mem_tbll_varslist_thm:
-  ∀ tbll tbl varslist.
-    (∀x. MEM x (fv_tbll (tbl::tbll)) ⇒ MEM x varslist) ⇒
-    (∀x. MEM x (fv_tbll  tbll) ⇒  MEM x varslist)
-Proof
-  gvs[fv_tbll_def]
-QED
-
-
-
-Theorem free_vars_simp_subst_in_original:
-  ∀ atom h' b x.
-    MEM x (fv_atom (simp_atom (mk_substitute_atom atom h' b))) ⇒
-    MEM x (fv_atom atom)
-Proof
-  Induct >>
-  gvs[fv_atom_def, simp_atom_def, mk_substitute_atom_def] >>
-  rpt strip_tac >>
-  rpt (BasicProvers.FULL_CASE_TAC >> gvs[]) >>
-  gvs[fv_atom_def, simp_atom_def, mk_substitute_atom_def] 
-QED
-      
 
         
-Theorem free_vars_simp_subst_row_in_original:
-  ∀ row h' b x.
-    MEM x (fv_row (simp_row (mk_substitute_row row h' b))) ⇒
-    MEM x (fv_row row)
+Theorem fv_atom_sub_single:
+  ∀ h x b x'.
+    MEM x' (fv_atom (mk_substitute_atom h x b)) ⇒
+    MEM x' (fv_atom h)
 Proof
   Induct >>
-  gvs[fv_row_def, simp_row_def, mk_substitute_row_def] >>
-  rpt strip_tac >>
-  gvs[MEM_FLAT] >>
+  rw[mk_substitute_atom_def, fv_atom_def]
+QED
+       
+
+Theorem fv_atoml_row_single:
+  ∀ atoml x' x b.
+    MEM x' (fv_row (mk_substitute_row atoml x b)) ⇒
+    MEM x' (fv_row atoml) 
+Proof
+  
+  Induct >>
+  rw[mk_substitute_row_def] >>
+  gvs[fv_row_def] >>
+  imp_res_tac fv_atom_sub_single >> gvs[] >>
+  first_x_assum (strip_assume_tac o (Q.SPECL [‘x'’, ‘x’, ‘b’])) >>
+  gvs[mk_substitute_row_def]
+QED
+
+        
+Theorem fv_tbl_sub_single:
+  ∀ tbl x' h' b.
+    MEM x' (fv_tbl (mk_substitute_tbl tbl h' b)) ⇒
+    MEM x' (fv_tbl tbl)
+Proof
+  Induct >>
+  rw[mk_substitute_tbl_def] >>
+  PairCases_on ‘h’ >> gvs[] >>
+  gvs[fv_tbl_def] >>
+  imp_res_tac fv_atoml_row_single >> gvs[] >>
+  gvs[mk_substitute_tbl_def] >>
+  res_tac >> gvs[]
+QED        
+
+Triviality mem_head_fv_tbll_triv:
+  ∀ varslist h tbl x' tbls.
+    (∀x. MEM x (fv_tbll (h::tbls)) ⇒ MEM x varslist) ∧
+    MEM x' (fv_tbl h) ⇒
+    MEM x' varslist
+Proof
+  rw[fv_tbll_def]
+QED
+
+        
+
+Theorem fv_tbls_in_sub_varslist_thm:
+  ∀ tbls varslist h b.
+    (∀x. MEM x (fv_tbll tbls) ⇒ MEM x varslist) ⇒
+    (∀x'. MEM x' (fv_tbll (MAP (λtbl. mk_substitute_tbl tbl h b) tbls)) ⇒ MEM x' varslist)
+Proof
+
+  Induct >>
+  rw[] >>
+  
+  imp_res_tac fv_mem_tbll_varslist_thm >>
   res_tac >>
-  first_x_assum (strip_assume_tac o (Q.SPECL [‘h'’, ‘b’])) >>
-  gvs[] >>
-  rpt (BasicProvers.FULL_CASE_TAC >> gvs[fv_atom_def]) >>
-  gvs[MEM_MAP] >> gvs[fv_atom_def] >>
-  imp_res_tac free_vars_simp_subst_in_original >> gvs[] >>
-  DISJ2_TAC >> gvs[] >>
-  metis_tac[]
+  
+  Cases_on ‘MEM x' (fv_tbl (mk_substitute_tbl h h' b)) ’ >>
+  
+  imp_res_tac fv_tbl_sub_single >>
+  imp_res_tac mem_head_fv_tbll_triv >>
+  
+  gvs[fv_tbll_def] >>
+  res_tac 
+QED  
+
+
+     
+Triviality simp_atom_fv_atom_triv:
+  ∀ atom s.
+    simp_atom atom = Var s ⇒ MEM s (fv_atom atom)
+Proof
+  Induct >> gvs[simp_atom_def, fv_atom_def]
 QED
 
 
+Theorem mem_flat_fv_row:
+  ∀ row row' x .
+    simp_row row = row' ∧
+    MEM x (FLAT (MAP (λatom. fv_atom atom) row')) ⇒
+    MEM x (FLAT (MAP (λatom. fv_atom atom) row))
+Proof
+  
+  Induct >>
+  gvs[simp_row_def] >> rw[]  >>
+  
+  (Cases_on ‘h’ >> gvs[simp_atom_def, fv_atom_def, is_not_true_var_atom_def] >>
+   rpt (BasicProvers.FULL_CASE_TAC >> gvs[])) >>
+  
+  fs[fv_atom_def]
+QED
+                     
 
-        
-Theorem free_vars_simp_subst_tbl_in_original:
-  ∀ tbl x h' b.
-    MEM x (fv_tbl (simp_tbl (mk_substitute_tbl tbl h' b))) ⇒
-    MEM x (fv_tbl tbl)
+     
+
+Theorem mem_fv_tbl_simp_mem:
+  ∀ tbl tbl' x.
+    MEM x ( fv_tbl tbl') ∧
+    simp_table tbl NONE = tbl' ⇒
+    MEM x ( fv_tbl tbl)
 Proof
   Induct >>
-  rpt strip_tac >>
-  gvs[fv_tbl_def, mk_substitute_tbl_def, simp_tbl_def] >|[
-    PairCases_on ‘h’ >> gvs[] >>
-    imp_res_tac free_vars_simp_subst_row_in_original >>
+  rw[simp_table_def] >>
+  gvs[fv_tbl_def] >>
+  PairCases_on ‘h’ >> 
+  
+  gvs[simp_table_def] >>
+  rpt (BasicProvers.FULL_CASE_TAC >> gvs[]) >>
+  gvs[fv_tbl_def, fv_row_def, fv_atom_def] >>
+  res_tac >> gvs[simp_row_cannot_result1] >>
+                                                 
+  imp_res_tac mem_flat_fv_row >>
+  gvs[fv_atom_def]
+QED     
+        
+
+
+
+Theorem fv_simp_tables_some_in_varlist:
+  ∀ t x s_in varslist.
+    (∀x'. MEM x' (fv_tbl t) ⇒ MEM x' varslist) ∧
+    MEM x (fv_tbl (simp_table t (SOME s_in))) ⇒
+    MEM x varslist
+Proof
+  
+  Induct >>
+  rw[simp_table_def] >>
+  PairCases_on ‘h’ >> gvs[] >>
+  rename1 ‘fv_tbl ((atoml, st, res)::t)’ >>
+  gvs[fv_tbl_def] >>
+  
+  ‘∀x'. MEM x' (fv_row atoml) ⇒ MEM x' varslist’ by gvs[] >>
+  
+  gvs[simp_table_def] >>
+  Cases_on ‘s_in ≠ st’ >> gvs[] >-
+   (
+   res_tac >> gvs[]
+   ) >>
+  
+  Cases_on ‘simp_row atoml’ >> gvs[] >-
+   gvs[fv_row_def] >>
+  res_tac >> gvs[] >>
+  
+  Cases_on ‘t'’ >> gvs[] >|[
+    Cases_on ‘h’ >> gvs[] >>
+    imp_res_tac mem_flat_fv_row >>
+    gvs[simp_row_cannot_result1] >>
+    res_tac >> gvs[] >>
+    gvs[fv_row_def]
+    ,
+    gvs[fv_row_def] >>
+    imp_res_tac mem_flat_fv_row >>
     gvs[]
     ,
     res_tac >> gvs[]
-  ]
-QED                                                         
-      
+  ]        
+QED
 
-Theorem free_vars_simp_subst_tbll_in_original:
-  ∀ tbls h b x varslist.
+
+
+Theorem mem_fv_tbl_simp_imp:
+  ∀ t n x.  MEM x (fv_tbl (simp_table t (SOME n))) ⇒
+            MEM x (fv_tbl (simp_table t NONE))
+Proof
+  Induct >>
+  rw[simp_table_def] >>
+  PairCases_on ‘h’ >>
+  rename1 ‘((atoml,st,res)::t)’ >>
+  gvs[simp_table_def] >>
+  
+  rpt (BasicProvers.FULL_CASE_TAC >> gvs[]) >>
+  gvs[fv_tbl_def, fv_row_def, fv_atom_def] >>
+  gvs[simp_row_cannot_result1] >>
+  res_tac >> gvs[]
+QED
+
+
+
+   
+Theorem mem_var_list_simp_tables_fv_tbll:
+  ∀ tbls s_in  h b x varslist.
     (∀x'. MEM x' (fv_tbll tbls) ⇒ MEM x' varslist) ∧
-    MEM x (fv_tbll (simp_tbll (mk_substitute_tbll tbls h b))) ⇒
+    (MEM x (fv_tbll (simp_tables tbls (SOME s_in))) ∨
+      MEM x (fv_tbll (simp_tables tbls NONE))   )⇒
     MEM x varslist
 Proof
-  Induct >-
-   (gvs[fv_tbll_def, mk_substitute_tbll_def, simp_tbll_def]) >>
+  gvs[simp_tables_eq] >>
+  Induct >>
+  rw[simp_tables2_def] >>
+  gvs[fv_tbll_def] >>
+
   
-  rpt strip_tac >>    
-  gvs[mk_substitute_tbll_def, simp_tbll_def] >>
-  imp_res_tac fv_mem_tbll_varslist_thm >>
-  res_tac >>
-  gvs[fv_tbll_def] >|[
-    imp_res_tac free_vars_simp_subst_tbl_in_original >>
-    gvs[]
+  imp_res_tac fv_simp_tables_some_in_varlist >> gvs[] >>
+  imp_res_tac mem_fv_tbl_simp_mem >> gvs[] >|[
+
+    Cases_on ‘next_state (simp_table h (SOME s_in))’ >> gvs[] >>
+    res_tac >> gvs[]
     ,
-    metis_tac[]      
-  ]                            
+        
+    Cases_on ‘next_state (simp_table h NONE)’ >> gvs[] >>
+    res_tac >> gvs[]
+  ]
 QED
 
         
@@ -1662,14 +2626,27 @@ Proof
   rpt strip_tac >>
   Cases_on ‘prop_parent’ >>
   rename1 ‘(tbls, s_in)’ >>
-  gvs[fv_tables_def, simp_tables_def, mk_substitute_tables_def] >>
-  imp_res_tac free_vars_simp_subst_tbll_in_original
+          
+  gvs[fv_tables_def, simp_tables_def, mk_substitute_tables_def, mk_substitute_tbll_def,
+      simp_tables_wrapper_def] >>
+
+  imp_res_tac fv_tbls_in_sub_varslist_thm >>
+  imp_res_tac mem_var_list_simp_tables_fv_tbll >>
+  res_tac >> gvs[] >>
+
+  metis_tac[]
+                        
 QED
 
 
 
 
-                 
+
+
+        
+        
+
+        
 val _ = export_theory ();
 
     
