hol/policy_to_table/bdd_gen_optimizationScript.sml
@@ -39,341 +39,225 @@ val _ = new_theory "bdd_gen_optimization";
 
 
 
-(* Helper lemma: operate_opt1 preserves correctness *)
-Theorem operate_opt1_preserves_correctness:
-  ∀BDD nl all_nodes vars vars_consumed rec.
-    valid_BDD rec BDD vars vars_consumed∧
-    correct_sem rec BDD (vars ⧺ vars_consumed)   ⇒
-    (valid_BDD rec (operate_opt1 BDD nl all_nodes) vars vars_consumed ∧
-     correct_sem rec (operate_opt1 BDD nl all_nodes) (vars ⧺ vars_consumed) 
-     )
-Proof
 
-  Induct_on ‘nl’ >> rpt gen_tac >- (
-    (* Base case: empty list *)
-    fs [operate_opt1_def]
-  ) >>
-  
-  (* Inductive case *)
-  rpt gen_tac >> strip_tac >>
-  fs [operate_opt1_def] >>
-  
-  (* Apply inductive hypothesis *)
-  first_x_assum irule >>
-          
-  (* Use merge_BDD_preserves_valid_and_correctness *)
-  imp_res_tac merge_BDD_preserves_valid_and_correctness >>
-  metis_tac[]  
-QED
-
-
-
-        
-(* Now the main theorem follows easily *)
-Theorem bdd_optminzation1_preserves_correctness:
-  ∀BDD vars vars_consumed rec.   
-    valid_BDD rec BDD vars vars_consumed ∧
-    correct_sem rec BDD (vars ⧺ vars_consumed)  ⇒
-    ( valid_BDD rec (bdd_optminzation1 BDD) vars vars_consumed ∧
-      correct_sem rec (bdd_optminzation1 BDD) (vars ⧺ vars_consumed) 
-    )
-Proof
-  rpt strip_tac >>
-  fs [bdd_optminzation1_def] >>
-  
-  PairCases_on ‘BDD’ >>
-  rename1 ‘(root, edges, labels)’ >>
-
-  rw[]>>
-  (* Apply operate_opt1_preserves_correctness *)
-  imp_res_tac operate_opt1_preserves_correctness >>
-  metis_tac[] 
-QED
-
-
-
-
-(* some elimination work*)
-
-Theorem operate_opt2_preserves_correctness:
-  ∀BDD nl all_nodes vars vars_consumed rec.
-    valid_BDD rec BDD vars vars_consumed ∧
-    correct_sem rec BDD (vars ⧺ vars_consumed)   ⇒
-    (valid_BDD rec (operate_opt2 BDD nl all_nodes) vars vars_consumed ∧
-     correct_sem rec (operate_opt2 BDD nl all_nodes) (vars ⧺ vars_consumed) 
-     )
-Proof
-
-  Induct_on ‘nl’ >> rpt gen_tac >- (
-    (* Base case: empty list *)
-    fs [operate_opt2_def]
-  ) >>
-  
-  (* Inductive case *)
-  rpt gen_tac >> strip_tac >>
-  fs [operate_opt2_def] >>
-  
-  (* Apply inductive hypothesis *)
-  first_x_assum irule >>
-                
-  gvs[] >>
-  imp_res_tac eliminate_BDD_preserves_valid_and_correctness >>
-  metis_tac[]  
-QED
-
-
-
-        
-(* Now the main theorem follows easily *)
-Theorem bdd_optminzation2_preserves_correctness:
-  ∀BDD vars vars_consumed rec.   
-    valid_BDD rec BDD vars vars_consumed ∧
-    correct_sem rec BDD (vars ⧺ vars_consumed) ⇒
-    ( valid_BDD rec (bdd_optminzation2 BDD) vars vars_consumed  ∧
-      correct_sem rec (bdd_optminzation2 BDD) (vars ⧺ vars_consumed)
-    )
-Proof
-  rpt strip_tac >>
-  fs [bdd_optminzation2_def] >>
-  
-  PairCases_on ‘BDD’ >>
-  rename1 ‘(root, edges, labels)’ >>
-
-
-  rw[]>>
-  (* Apply operate_opt1_preserves_correctness *)
-  imp_res_tac operate_opt2_preserves_correctness >>
-  metis_tac[] 
-QED
-
-
-
-
- (**** GLUE OPT TOGETHER *****)       
- 
-(* Combining the two optimizations *)
-Theorem bdd_one_round_preserves_correctness:
-  ∀BDD vars vars_consumed rec.
-    valid_BDD rec BDD vars vars_consumed ∧
-    correct_sem rec BDD (vars ⧺ vars_consumed) ⇒
-    (
-    valid_BDD rec (bdd_one_round BDD) vars vars_consumed ∧
-    correct_sem rec (bdd_one_round BDD) (vars ⧺ vars_consumed)
-    )            
-Proof
-  rw[bdd_one_round_def] >>
-  imp_res_tac bdd_optminzation2_preserves_correctness >>
-  imp_res_tac bdd_optminzation1_preserves_correctness
-QED
-
-
-
-
-        
-
-        
-(* This theorem is just for optimisations *)
-Theorem bdd_optimize_preserves_correctness:
-  ∀BDD vars vars_consumed rec.
-    valid_BDD rec BDD vars vars_consumed ∧
-    correct_sem rec BDD (vars ⧺ vars_consumed) ⇒
-    (
-    valid_BDD rec (bdd_full_optimize BDD) vars vars_consumed ∧
-    correct_sem rec (bdd_full_optimize BDD) (vars ⧺ vars_consumed)
-    )
-Proof
-  (* Use strong induction on the measure that ensures termination *)
-  completeInduct_on ‘BDD_label_length BDD’ >>
-  rpt gen_tac >> strip_tac >>
-  rpt gen_tac >> strip_tac >>
-      
-  (* Unfold the definition *)
-  once_rewrite_tac[bdd_full_optimize_def] >>
-  Cases_on ‘bdd_one_round BDD = BDD’ >> fs[] >>
-           
-  (* Recursive case: optimization makes progress *)
-  imp_res_tac bdd_one_round_preserves_correctness >>
-
-  (* Apply induction hypothesis *)
-  subgoal ‘BDD_label_length (bdd_one_round BDD) < BDD_label_length BDD’ >- (
-    metis_tac[bdd_one_round_reduce]
-  ) >>
+Theorem merge_safe_preserves_valid_and_correctness:
+  ∀ BDD b_BDD' rec vars_consumed vars n n' c.
     
-  (* Apply induction hypothesis *)
-  first_x_assum (strip_assume_tac o (Q.SPECL [‘BDD_label_length (bdd_one_round BDD)’])) >>
-  gvs[] >>
-        
-  first_x_assum (strip_assume_tac o (Q.SPECL [‘(bdd_one_round BDD)’])) >>
-  gvs[] >>
-
-  first_x_assum (strip_assume_tac o (Q.SPECL [‘vars’, ‘rec’])) >>
-  gvs[] 
-       
-QED
-
-
-
-
-
-
-Theorem fv_in_BDD_reverse_triv2:
-  ∀ BDD vars vars_consumed h rec.
-    fv_in_BDD rec BDD (REVERSE vars ++ h ++ vars_consumed) =
-    fv_in_BDD rec BDD (vars ++ h ++ vars_consumed)
+    valid_BDD rec BDD vars vars_consumed ∧
+    correct_sem rec BDD (REVERSE vars ⧺ vars_consumed) ∧
+    range_c c BDD ∧
+    
+    b_BDD' = merge_safe BDD n n' ⇒
+    
+    (valid_BDD rec (SND b_BDD') vars vars_consumed ∧
+     correct_sem rec (SND b_BDD') (REVERSE vars ⧺ vars_consumed) ∧
+     range_c c (SND b_BDD')
+     )
 Proof
-  rpt strip_tac >>
-  PairCases_on ‘BDD’ >>
-  rename1 ‘(r,edges,labels)’ >>
-  
-  fs[fv_in_labels_def, fv_in_BDD_def, merge_def, fv_in_vars_def] >>
-  rpt strip_tac >>
-  res_tac >>
-  fs[fv_in_vars_def]
-QED
-
-
-
-(* RANGE IS PRESERVED *)
-
-   
-Theorem merge_BDD_preserves_range:
-  ∀ BDD c n nl.
-    range_c c BDD ⇒
-    (range_c c (merge_BDD BDD n nl) ∧
-     range_c c (eliminate_BDD BDD nl) )
-Proof
-  Induct_on ‘nl’ >-
-   fs [merge_BDD_def, eliminate_BDD_def] >>
-  
-  rpt strip_tac >>
-      
-  fs [merge_BDD_def, eliminate_BDD_def] >>
-  rpt (BasicProvers.FULL_CASE_TAC >> rgs[]) >|[
-      
-    Cases_on ‘mergable BDD n h’ >> gvs[] >>
-    imp_res_tac merge_range_preservation >>
-    metis_tac[]
+  rw[merge_safe_def] >>
+  Cases_on ‘mergable BDD n n'’ >> gvs[] >|[
+    gvs[valid_BDD_def] >>
+    ‘BDD_WF (merge BDD n n')’ by imp_res_tac merge_wf_preservation >>
+    ‘BDD_ordered (merge BDD n n') vars_consumed’ by imp_res_tac merge_order_preservation >>
+    ‘fv_in_BDD rec (merge BDD n n') (REVERSE vars ⧺ vars_consumed)’ by
+      (imp_res_tac merge_fv_final_preservation >>
+       first_x_assum (strip_assume_tac o (Q.SPECL [‘n'’, ‘n’]))) >>
+    ‘consumed_dom_bdd vars_consumed (merge BDD n n')’ by
+      (imp_res_tac merge_consumed_dom_final_preservation >>
+       first_x_assum (strip_assume_tac o (Q.SPECL [‘n'’, ‘n’]))) >>
+    
+    gvs[]
     ,
-    imp_res_tac merge_range_preservation >>
-    metis_tac[]
+    
+    gvs[valid_BDD_def] >>
+    assume_tac merge_correct >>
+    first_x_assum (strip_assume_tac o (Q.SPECL [‘BDD’, ‘REVERSE vars’, ‘vars_consumed’, ‘n’, ‘n'’, ‘rec’])) >>
+    gvs[]
+    ,
+    gvs[merge_range_preservation]
   ]
 QED
-        
 
-Theorem operate_opt1_preserves_range:
-  ∀BDD c nl all_nodes.   
-    range_c c BDD  ⇒
-    range_c c (operate_opt1 BDD nl all_nodes) 
-Proof
-
-  Induct_on ‘nl’ >> rpt gen_tac >- 
-    fs [operate_opt1_def] >>
-  
-  rpt gen_tac >> strip_tac >>
-  fs [operate_opt1_def] >>
-  
-  first_x_assum irule >>    
-  gvs[] >>
-  imp_res_tac merge_BDD_preserves_range >>
-  metis_tac[]  
-QED
-
-
-
-
-Theorem operate_opt2_preserves_range:
-  ∀BDD c nl all_nodes.   
-    range_c c BDD  ⇒
-    range_c c (operate_opt2 BDD nl all_nodes) 
-Proof
-
-  Induct_on ‘nl’ >> rpt gen_tac >- 
-    fs [operate_opt2_def] >>
-  
-  rpt gen_tac >> strip_tac >>
-  fs [operate_opt2_def] >>
-  
-  first_x_assum irule >>    
-  gvs[] >>
-  imp_res_tac merge_BDD_preserves_range >>
-  metis_tac[]  
-QED
 
         
-   
-Theorem bdd_optminzation1_preserves_range:
-  ∀BDD c.   
-    range_c c BDD  ⇒
-    range_c c (bdd_optminzation1 BDD) 
-Proof
-  rpt strip_tac >>
-  fs [bdd_optminzation1_def] >>
-  
-  PairCases_on ‘BDD’ >>
-  rename1 ‘(root, edges, labels)’ >>
-
-
-  rw[]>>
-  metis_tac[operate_opt1_preserves_range]
-QED
-
-   
-Theorem bdd_optminzation2_preserves_range:
-  ∀BDD c.   
-    range_c c BDD  ⇒
-    range_c c (bdd_optminzation2 BDD) 
-Proof
-  rpt strip_tac >>
-  fs [bdd_optminzation2_def] >>
-  
-  PairCases_on ‘BDD’ >>
-  rename1 ‘(root, edges, labels)’ >>
-
-
-  rw[]>>
-  metis_tac[operate_opt2_preserves_range]
-QED
-
-
-Theorem bdd_one_round_preserves_range:
-  ∀ BDD c.
-    range_c c BDD ⇒
-    range_c c (bdd_one_round BDD)
-Proof
-  rw[bdd_one_round_def] >>
-  imp_res_tac bdd_optminzation2_preserves_range >>
-  imp_res_tac bdd_optminzation1_preserves_range
-QED
-
-        
-Theorem full_optimizations_preserves_range:
-  ∀ BDD c.
-    range_c c BDD ⇒
-    range_c c (bdd_full_optimize BDD)
-Proof
-
- completeInduct_on ‘BDD_label_length BDD’ >>
-  rpt gen_tac >> strip_tac >>
-  rpt gen_tac >> strip_tac >>
-      
-  (* Unfold the definition *)
-  once_rewrite_tac[bdd_full_optimize_def] >>
-  Cases_on ‘bdd_one_round BDD = BDD’ >> fs[] >>
-           
-  (* Recursive case: optimization makes progress *)
-  imp_res_tac bdd_one_round_preserves_range >>
-
-  (* Apply induction hypothesis *)
-  subgoal ‘BDD_label_length (bdd_one_round BDD) < BDD_label_length BDD’ >- (
-    metis_tac[bdd_one_round_reduce]
-  ) >>
-
- gvs[]
-QED
-      
+Theorem eliminate_safe_preserves_valid_and_correctness:
+  ∀ BDD b_BDD' rec vars_consumed vars n c.
     
+    valid_BDD rec BDD vars vars_consumed ∧
+    correct_sem rec BDD (REVERSE vars ⧺ vars_consumed) ∧
+    range_c c BDD ∧
+    
+    b_BDD' = eliminate_safe BDD n ⇒
+    
+    (valid_BDD rec (SND b_BDD') vars vars_consumed ∧
+     correct_sem rec (SND b_BDD') (REVERSE vars ⧺ vars_consumed)∧
+     range_c c (SND b_BDD'))
+Proof
+  rw[eliminate_safe_def] >>
+  Cases_on ‘eliminable BDD n’ >> gvs[] >|[
+    gvs[valid_BDD_def] >>
+    ‘BDD_WF (merge BDD x n)’ by imp_res_tac eliminate_wf_preservation >>
+    ‘BDD_ordered (merge BDD x n) vars_consumed’ by imp_res_tac eliminate_order_preservation >>
+    ‘fv_in_BDD rec (merge BDD x n) (REVERSE vars ⧺ vars_consumed)’ by
+      (imp_res_tac merge_fv_final_preservation >>
+       first_x_assum (strip_assume_tac o (Q.SPECL [‘n’, ‘x’]))) >>
+    imp_res_tac merge_consumed_dom_final_preservation >>
+    first_x_assum (strip_assume_tac o (Q.SPECL [‘n’, ‘x’]) ) >>
+    gvs[]
+    ,
+    gvs[valid_BDD_def] >>
+    assume_tac eliminate_correct >>
+    first_x_assum (strip_assume_tac o (Q.SPECL [‘BDD’, ‘REVERSE vars’, ‘vars_consumed’, ‘x’, ‘n’, ‘rec’])) >>
+    gvs[]
+    ,
+    gvs[merge_range_preservation]
+  ]
+QED
+                                         
 
+
+
+Theorem optimize_node_preserves_valid_and_correctness:
+  ∀ BDD BDD' rec vars_consumed vars edges_proj labels_proj nl n c.
+    
+    valid_BDD rec BDD vars vars_consumed ∧
+    correct_sem rec BDD (REVERSE vars ⧺ vars_consumed) ∧
+    range_c c BDD ∧
+            
+    BDD' = optimize_node edges_proj labels_proj BDD n nl ⇒
+    
+    (valid_BDD rec BDD' vars vars_consumed ∧
+     correct_sem rec BDD' (REVERSE vars ⧺ vars_consumed) ∧
+     range_c c BDD') 
+Proof
+  
+  Induct_on ‘nl’ >> rpt gen_tac >> strip_tac >|[
+    gvs[optimize_node_def] >>
+    metis_tac[eliminate_safe_preserves_valid_and_correctness]
+    ,
+    rgs[optimize_node_def] >>
+    Cases_on ‘eliminable_projection edges_proj n’ >> rgs[] >|[
+        Cases_on ‘mergable_projection edges_proj labels_proj h n’ >> rgs[] >>
+        Cases_on ‘merge_safe BDD h n ’ >> rgs[] >>
+        Cases_on ‘q’ >> gvs[] >>
         
+        imp_res_tac merge_safe_preserves_valid_and_correctness >>
+        gvs[] >>
+        first_x_assum (strip_assume_tac o (Q.SPECL [‘n’, ‘h’, ‘vars_consumed’, ‘vars’, ‘rec’])) >>
+        first_x_assum (strip_assume_tac o (Q.SPECL [‘n’, ‘h’, ‘vars_consumed’, ‘vars’, ‘rec’])) >>
+        first_x_assum (strip_assume_tac o (Q.SPECL [‘n’, ‘h’, ‘c’])) >>
+        gvs[] >>
+
+        res_tac >>
+        metis_tac[]
+        ,
+        metis_tac[eliminate_safe_preserves_valid_and_correctness]  
+      ]                                                                                             
+  ]
+QED
+
+
+
+      
+
+Theorem optimize_layer_preserves_valid_and_correctness:
+  ∀ nl BDD BDD' rec vars_consumed vars edges_proj labels_proj c.
+       
+    valid_BDD rec BDD vars vars_consumed ∧
+    correct_sem rec BDD (REVERSE vars ⧺ vars_consumed) ∧
+    range_c c BDD ∧
+    
+    BDD' = optimize_layer edges_proj labels_proj BDD nl ⇒
+         
+    (valid_BDD rec BDD' vars vars_consumed ∧
+     correct_sem rec BDD' (REVERSE vars ⧺ vars_consumed) ∧
+     range_c c BDD')
+Proof
+  Induct >>
+  rw[optimize_layer_def] >> gvs[] >>
+  ‘∃ BDD_opt . optimize_node edges_proj labels_proj BDD h nl = BDD_opt’ by gvs[] >> rgs[] >>
+  metis_tac[optimize_node_preserves_valid_and_correctness]
+QED
+
+
+      
+
+
+Theorem optimize_internals_preserves_valid_and_correctness:
+  ∀ internals BDD BDD' rec vars_consumed vars c.
+    valid_BDD rec BDD vars vars_consumed ∧
+    correct_sem rec BDD (REVERSE vars ⧺ vars_consumed) ∧
+    range_c c BDD ∧
+    
+    BDD' = optimize_internals BDD internals ⇒
+    (correct_sem rec BDD' (REVERSE vars ⧺ vars_consumed) ∧
+     valid_BDD rec BDD' vars vars_consumed ∧
+     range_c c BDD')
+Proof
+  Induct >> rpt gen_tac >> strip_tac >>
+  rgs[optimize_internals_def] >>
+
+  PairCases_on ‘h’ >>
+  Cases_on ‘h1’ >>
+
+  rgs[optimize_internals_def] >>
+
+  ‘∃ edges_proj . project_edges_to BDD x = edges_proj’ by gvs[] >> rgs[] >>
+  ‘∃ labels_proj . project_labels_to BDD x = labels_proj’ by gvs[] >> rgs[] >>
+  ‘∃ BDD1 . optimize_layer edges_proj labels_proj BDD x = BDD1’ by gvs[] >> rgs[] >>
+  
+  metis_tac[optimize_layer_preserves_valid_and_correctness]
+QED
+
+
+                              
+Theorem optimize_bdd_preserves_valid_and_correctness:
+
+ ∀ BDD BDD' vars_consumed vars rec c.
+       
+   valid_BDD rec BDD vars vars_consumed ∧
+   correct_sem rec BDD (REVERSE vars ⧺ vars_consumed) ∧
+   range_c c BDD ∧
+
+               
+   optimize_bdd BDD vars_consumed = BDD'
+   ⇒
+   (correct_sem rec BDD' (REVERSE vars ⧺ vars_consumed) ∧
+    valid_BDD rec BDD' vars vars_consumed ∧
+    range_c c BDD' )
+Proof
+  
+  rpt gen_tac >> strip_tac >>
+  rgs[optimize_bdd_def] >>
+  
+  ‘∃ l . bdd_distribute BDD vars_consumed = l ’ by gvs[] >> rgs[] >>
+  PairCases_on ‘l’ >> rgs[] >>
+  rename1 ‘(internals,ntl,tl)’ >>
+  ‘∃ labels_proj_tl . project_labels_to BDD tl = labels_proj_tl’ by gvs[] >> rgs[] >>
+  ‘∃ labels_proj_ntl . project_labels_to BDD ntl = labels_proj_ntl’ by gvs[] >> rgs[] >>
+  ‘∃ BDD1 . optimize_layer [] labels_proj_tl BDD tl = BDD1’  by gvs[] >> rgs[] >>
+  ‘∃ BDD2 . optimize_layer [] labels_proj_ntl BDD1 ntl = BDD2’  by gvs[] >> rgs[] >>
+  
+  
+  ‘correct_sem rec BDD1 (REVERSE vars ⧺ vars_consumed) ∧
+   valid_BDD rec BDD1 vars vars_consumed ∧
+   range_c c BDD1’ by metis_tac[optimize_layer_preserves_valid_and_correctness] >>
+  
+  
+  ‘correct_sem rec BDD2 (REVERSE vars ⧺ vars_consumed)∧
+   valid_BDD rec BDD2 vars vars_consumed ∧
+   range_c c BDD2’ by metis_tac[optimize_layer_preserves_valid_and_correctness] >>
+  
+  metis_tac[optimize_internals_preserves_valid_and_correctness]
+QED
+
+
+
+
+
+
+
+      
 Theorem correct_sem_valid_translation_opt:
   ∀ vars vars_consumed BDD BDD' rec c.
     prop1 rec ∧ prop2 rec ∧ prop3 rec ∧ prop4 rec ∧
@@ -393,59 +277,65 @@ Proof
   
  Induct >>
  rpt gen_tac >> strip_tac >>
- gvs[mk_BDDPred_opt_def] >>
+ gvs[mk_BDDPred_opt_def] >|[
+                         
+    (* base case : one final optimization *)
+    assume_tac optimize_bdd_preserves_valid_and_correctness >>
+    gvs[] >>
+    first_x_assum (strip_assume_tac o (Q.SPECL [‘BDD’, ‘vars_consumed’, ‘[]’,  ‘rec’, ‘c’])) >>
+    gvs[]
+          
+    ,
 
- gvs[AllCaseEqs()] >>
+    gvs[AllCaseEqs()] >>
 
-
- rpt strip_tac >>
+    PairCases_on ‘BDD’ >>
+    rename1 ‘(r,edges,labels)’ >>
  
- PairCases_on ‘BDD’ >>
- rename1 ‘(r,edges,labels)’ >>
+    PairCases_on ‘BDD'’ >>
+    rename1 ‘(r',edges',labels')’ >>
  
- PairCases_on ‘BDD'’ >>
- rename1 ‘(r',edges',labels')’ >>
+    PairCases_on ‘BDD''’ >>
+    rename1‘((r'',edges'',labels''),c')’ >>
  
- PairCases_on ‘BDD''’ >>
- rename1‘((r'',edges'',labels''),c')’ >>
- 
- gvs[valid_BDD_def] >>
-
- ‘range_c c' (r'',edges'',labels'')’ by imp_res_tac WFness_range_c_inter >>
- 
- ‘BDD_WF (r'',edges'',labels'')’ by imp_res_tac WFness_translation_inter >> gvs[]>>
- 
- ‘ALL_DISTINCT (h::vars_consumed)’ by gvs[ALL_DISTINCT_APPEND] >>        
- ‘BDD_ordered (r'',edges'',labels'') (h::vars_consumed)’ by imp_res_tac order_translation_inter >>
- 
- ‘consumed_dom_bdd (h::vars_consumed) (r'',edges'',labels'')’ by imp_res_tac consumed_dom_bdd_inter >>
- 
- 
- assume_tac correct_sem_translation_inter >>
- first_x_assum (strip_assume_tac o (Q.SPECL [‘(r,edges,labels)’, ‘(r'',edges'',labels'')’, ‘rec’, ‘c’, ‘c'’, ‘REVERSE vars’, ‘h’, ‘vars_consumed’])) >>
- gvs[]>>
-
- ‘fv_in_BDD rec (r'',edges'',labels'') (REVERSE vars ⧺ [h] ⧺ vars_consumed)’ by metis_tac[fv_in_BDD_body_preserved] >>
-
- (* now we show that opt is also correct *)
- 
- assume_tac bdd_optimize_preserves_correctness >>
- first_x_assum (strip_assume_tac o (Q.SPECL [‘(r'',edges'',labels'')’, ‘REVERSE vars’, ‘[h] ⧺ vars_consumed’, ‘rec’])) >>
- gvs[valid_BDD_def] >>
+    gvs[valid_BDD_def] >>
 
 
- ‘fv_in_BDD rec (r'',edges'',labels'') (vars ⧺ [h] ⧺ vars_consumed) ’ by metis_tac[fv_in_BDD_reverse_triv2] >>
-  gvs[] >>
-        
- first_x_assum (strip_assume_tac o (Q.SPECL [‘[h] ⧺ vars_consumed’, ‘(bdd_full_optimize (r'',edges'',labels''))’,
-                                            ‘(r',edges',labels')’, ‘rec’, ‘c'’])) >>
-
- gvs[] >>
-
- ‘range_c c' (bdd_full_optimize (r'',edges'',labels''))’ by metis_tac[full_optimizations_preserves_range] >>
- ‘fv_in_BDD rec (bdd_full_optimize (r'',edges'',labels'')) (REVERSE vars ⧺ [h] ⧺ vars_consumed)’ by metis_tac[fv_in_BDD_reverse_triv2] >>
+    (* first show that the body of make preserves all of the desired properties *)
+                       
+    ‘range_c c' (r'',edges'',labels'')’ by imp_res_tac WFness_range_c_inter >>
  
- metis_tac[]
+    ‘BDD_WF (r'',edges'',labels'')’ by imp_res_tac WFness_translation_inter >> gvs[]>>
+ 
+    ‘ALL_DISTINCT (h::vars_consumed)’ by gvs[ALL_DISTINCT_APPEND] >>        
+    ‘BDD_ordered (r'',edges'',labels'') (h::vars_consumed)’ by
+      imp_res_tac order_translation_inter >>
+
+    ‘consumed_dom_bdd (h::vars_consumed) (r'',edges'',labels'')’ by
+      imp_res_tac consumed_dom_bdd_inter >>
+    
+    
+    assume_tac correct_sem_translation_inter >>
+    first_x_assum (strip_assume_tac o (Q.SPECL [‘(r,edges,labels)’, ‘(r'',edges'',labels'')’,
+                                                ‘rec’, ‘c’, ‘c'’, ‘REVERSE vars’, ‘h’, ‘vars_consumed’])) >>
+    gvs[]>>
+    
+    ‘fv_in_BDD rec (r'',edges'',labels'') (REVERSE vars ⧺ [h] ⧺ vars_consumed)’ by
+      metis_tac[fv_in_BDD_body_preserved] >>
+     
+    (* now we show that opt is also correct *)
+    
+    assume_tac optimize_bdd_preserves_valid_and_correctness >> gvs[] >>
+    first_x_assum (strip_assume_tac o (Q.SPECL [‘(r'',edges'',labels'')’, ‘[h] ⧺ vars_consumed’, ‘vars’,  ‘rec’, ‘c'’])) >>
+    gvs[valid_BDD_def] >>
+
+       
+    first_x_assum (strip_assume_tac o (Q.SPECL [‘[h] ⧺ vars_consumed’,
+                                                ‘optimize_bdd (r'',edges'',labels'') (h::vars_consumed)’,
+                                                ‘(r',edges',labels')’, ‘rec’, ‘c'’])) >>
+
+    gvs[] 
+  ]
 QED 
 
 
