hol/policy_to_table/tables_spec_oldScript.sml
@@ -1,0 +1,1675 @@
+open HolKernel boolLib liteLib simpLib Parse bossLib;
+open arithmeticTheory stringTheory containerTheory pred_setTheory
+     listTheory finite_mapTheory;
+
+open p4Lib;
+open blastLib bitstringLib;
+open p4Theory;
+open p4_auxTheory;
+open p4_coreTheory;
+
+open bitstringTheory;
+open wordsTheory;
+open optionTheory;
+open sumTheory;
+open stringTheory;
+open ottTheory;
+open pairTheory;
+open rich_listTheory;
+open arithmeticTheory;
+open alistTheory;
+open numeralTheory;
+open alistTheory;
+open set_relationTheory;
+open pred_setTheory;
+open pred_setLib;
+
+open bdd_genTheory;     
+open pred_specTheory;     
+open policy_specTheory;     
+     
+
+
+val _ = new_theory "tables_spec_old";
+
+    
+
+(* atomic variable based predicates predicates*)
+val _ = Hol_datatype `
+     atom_var = True
+                | False
+                | NotTrue
+                | NotFalse
+                | Var of string
+                | Not of string
+               `;
+
+val _ = Hol_datatype `action_expr = action of 'a | state of num`;
+
+
+Type var_line = “:(atom_var list # num # 'a action_expr)”;
+Type var_table = “: ('a var_line) list”
+Type var_table_list = “: ('a var_table) list”
+   
+
+
+
+(***************************************************)
+(* some work for the variable based atoms          *)
+(***************************************************)
+
+
+
+Definition sem_var_atom_def:
+  (sem_var_atom ((Var x): atom_var) mv = (ALOOKUP mv x)) /\
+  (sem_var_atom True _ = SOME T) /\
+  (sem_var_atom False _ = SOME F) /\
+  (sem_var_atom NotTrue _ = SOME F) /\
+  (sem_var_atom NotFalse _ = SOME T) /\
+  (sem_var_atom (Not x) mv = 
+   case (ALOOKUP mv x) of
+   | SOME b => SOME (~b)
+   | _ => NONE
+  )
+End
+
+
+Definition mk_substitute_atom_def:
+  (mk_substitute_atom (True:atom_var) x b = True) ∧
+  (mk_substitute_atom False x b = False) ∧
+  (mk_substitute_atom NotTrue x b = NotTrue) ∧
+  (mk_substitute_atom NotFalse x b = NotFalse) ∧
+  (mk_substitute_atom (Var x') x b = 
+   if (x=x') then (if b then True else False) else (Var x')) ∧
+  (mk_substitute_atom (Not x') x b = 
+   if (x=x') then (if b then NotTrue else NotFalse) else (Not x'))
+End
+
+   
+Definition simp_atom_def:
+  (simp_atom ((Var x):atom_var) = Var x) /\
+  (simp_atom True = True) /\
+  (simp_atom False = False) /\
+  (simp_atom NotTrue = False) /\
+  (simp_atom NotFalse = True) /\
+  (simp_atom (Not x) = Not x)
+End
+
+
+Definition final_atom_def:
+  final_atom (p:atom_var) = 
+  case p of
+  | True => SOME T
+  | False => SOME F
+  | NotTrue => SOME F
+  | NotFalse => SOME T
+  | _ => NONE
+End
+
+
+Definition fv_atom_def:
+  (fv_atom ((Var x):atom_var) = [x]) ∧
+  (fv_atom True = []) ∧
+  (fv_atom False = []) ∧
+  (fv_atom NotTrue = []) ∧
+  (fv_atom NotFalse = []) ∧
+  (fv_atom (Not x) = [x])
+End
+
+                        
+                
+(***************************************************)
+(* specialized definitions for a predicate record. *)
+(*   here 'a would be policy and 'b would be       *) 
+(*          action wrt record data type            *)
+(***************************************************)
+
+           
+
+(* Check if all predicates in list evaluate to true *)
+Definition is_atoml_true_def:
+  is_atoml_true atoml mv = 
+  EVERY (\minipred. sem_var_atom minipred mv = SOME T) atoml
+End
+
+        
+(* Check if row matches current state and guard conditions *)
+Definition is_match_row_def:
+  is_match_row st_in st_num atoml mv = 
+    ((st_in = st_num) ∧ is_atoml_true atoml mv ∧ atoml ≠ [])
+End
+
+
+Definition check_all_rows_match_def:
+  check_all_rows_match st_in tbl mv =
+  MAP (\(atoml,st_num,res). (is_match_row st_in st_num atoml mv, res)) tbl
+End
+
+
+
+(* Find first matching line in a single table *)
+Definition match_tbl_def:
+  match_tbl (tbl: 'a var_table) mv st_in =
+  let lines_res = (check_all_rows_match st_in tbl mv) in
+    case min_idx_till lines_res T of
+    | SOME (idx, line) => SOME (SND line)
+    | NONE => NONE
+End
+
+
+        
+        
+        
+(* Process table list with state propagation *) 
+Definition match_tbll_def:
+  match_tbll ([]: 'a var_table_list) mv st_in = NONE ∧
+  match_tbll [tbl] mv st_in =
+  ( case match_tbl tbl mv st_in of
+    | SOME (action a) => SOME (action a)
+    | _ => NONE       
+  )∧
+  match_tbll (tbl::tbls) mv st_in =
+  ( case match_tbl tbl mv st_in of
+    | SOME (state n) => match_tbll tbls mv n
+    | _ => NONE
+  )
+End
+
+ 
+(* Top-level table semantics, return the starting state as well*)       
+Definition sem_tables_def:
+  sem_tables ((tbll: 'a var_table_list),st_in) mv =
+   match_tbll tbll mv st_in
+End
+
+
+(*
+EVAL “match_tbl [([False], 0 , action "s")] [] 0”;
+EVAL “match_tbl [([True], 0 , action "s")] [] 0”;
+EVAL “match_tbl [([Var "a"], 0 , action "s1");([True], 0 , action "s2")] [("a",T)] 0”;
+EVAL “match_tbl [([Var "a"; True], 0 , action "s1"); ([True], 0 , action "s2")] [("a",T)] 0”;
+
+                    
+EVAL “match_tbl [([False;True],0,state 2); ([False],0,state 3);([True],0,state 3)] [] 0”;
+EVAL “match_tbl [([True],3,state 4); ([False],3,state 5); ([True],2,state 2)] [] 3”;
+EVAL “match_tbl [([True],2,action ("fwd",[(1:num)])); ([True],4,action ("fwd",[2])); ([True],5,action ("drop",[]))] [] 4”;
+
+
+EVAL “sem_tables ([[([False],0,state 2); ([False],0,state 3);([True],0,state 3)];
+                  [([True],3,state 4); ([False],3,state 5); ([True],2,state 2)];
+                  [([True],2,action ("fwd",[1])); ([True],4,action ("fwd",[2])); ([True],5,action ("drop",[]))]],0) []”                  
+*)
+
+      
+(* table substitute *)
+                          
+Definition mk_substitute_row_def:
+  mk_substitute_row atoml x b =
+    MAP (\atom. mk_substitute_atom atom x b) atoml
+End
+   
+Definition mk_substitute_tbl_def:
+  mk_substitute_tbl (tbl: 'a var_table) x b =
+  ((MAP (\(atoml,st_num,res). (mk_substitute_row atoml x b, st_num, res)) tbl) :'a var_table)
+End
+
+   
+Definition mk_substitute_tbll_def:
+  mk_substitute_tbll (tbll: 'a var_table_list) x b =
+  MAP (\(tbl). mk_substitute_tbl (tbl: 'a var_table) x b) tbll 
+End
+
+
+Definition mk_substitute_tables_def:
+  mk_substitute_tables ((tbll: 'a var_table_list), st_in) x b =
+   (mk_substitute_tbll tbll x b, st_in:num)
+End
+        
+(* table simplifications *)
+
+Definition simp_row_old_def:
+  simp_row_old atoml =
+  let simplified_row = MAP (\atom. simp_atom atom) atoml in
+    case MEM False simplified_row of
+    | T => MAP (\a. False) atoml
+    | F => simplified_row
+End
+
+
+Definition simp_tbl_def:
+  simp_tbl (tbl: 'a var_table) =
+  MAP (\(atoml,st_num,res). simp_row_old atoml,st_num,res) tbl
+End
+
+
+Definition simp_tbll_def:
+  simp_tbll (tbll: 'a var_table_list) =
+  MAP (\tbl. simp_tbl tbl) tbll
+End
+
+
+Definition simp_tables_old_def:
+  simp_tables_old ((tbll: 'a var_table_list), st_in) =
+   (simp_tbll tbll, st_in:num)
+End
+
+
+(*
+EVAL “simp_tbl [([False], 0 , action "s")]”;
+EVAL “simp_tbl [([True; False], 0 , action "s")]”;
+EVAL “simp_tbl [([Var "a"], 0 , action "s1");([True;False], 0 , action "s2")]”;
+EVAL “simp_tbl [([Var "a"; False], 0 , action "s1"); ([True], 0 , action "s2")]”;
+
+EVAL “simp_tbll   ([[([False; Var "a"],0,state 2); ([False],0,state 3);([True],0,state 3)];
+                  [([True],3,state 4); ([False],3,state 5); ([True],2,state 2)];
+                  [([Var "a"; False], 0 , action "s1"); ([True], 0 , action "s2")]]) ”                  
+*)
+
+
+        
+(* table final *)
+
+Definition all_true_def:
+  all_true atoml =
+  EVERY (\atom. atom = True) atoml
+End
+
+
+Definition all_false_def:
+  all_false atoml =
+  EVERY (\atom. atom = False) atoml
+End
+        
+       
+Definition is_hit_def:
+  is_hit st_in st_num atoml = 
+    ((st_in = st_num) ∧ all_true atoml ∧ atoml ≠ [])
+End
+
+
+Definition is_hit_tbl_check_def:
+  is_hit_tbl_check (tbl: 'a var_table) st_in =
+  MAP (\(atoml, st_num, res). is_hit st_in st_num atoml, st_num, res) tbl
+End
+
+
+
+Definition pre_lines_are_fail_def:
+  pre_lines_are_fail (tbl: 'a var_table) idx st_in =
+  EVERY (\(atoml, st_num, res).  if st_num = st_in then all_false atoml else T) (SEG idx 0 tbl)
+End
+
+        
+Definition final_tbl_old_def:
+  final_tbl_old  (tbl: 'a var_table) st_in =
+  let lines_res = is_hit_tbl_check tbl st_in in
+    case min_idx_till lines_res T of
+    | SOME (idx, b, st_num, res) =>
+        ( case pre_lines_are_fail tbl idx st_in of
+          | T => SOME res
+          | F => NONE
+        )
+    | _ => NONE
+End
+
+(*
+EVAL “final_tbl_old  [([False], 0 , action "s")] 0” (*must fail *)
+EVAL “final_tbl_old  [([True], 0 , action "s")] 0”
+EVAL “final_tbl_old  [([False], 0 , action "s1");([True], 0 , action "s2")] 0”
+EVAL “final_tbl_old  [([Var "a"], 0 , action "s1");([True], 1 , action "s2")] 1”
+EVAL “final_tbl_old  [([Var "a"], 0 , action "s1");([True], 0 , action "s2")] 0” (* must fail *)  
+*)
+        
+        
+Definition final_tbll_old_def:
+  final_tbll_old ([]: 'a var_table_list) st_in = NONE ∧
+  final_tbll_old [tbl] st_in =
+  ( case final_tbl_old  tbl st_in of
+    | SOME (action a) => SOME (action a)
+    | _ => NONE       
+  )∧
+  final_tbll_old (tbl::tbls) st_in =
+  ( case final_tbl_old  tbl st_in of
+    | SOME (state n) => final_tbll_old tbls n
+    | _ => NONE
+  )
+End
+
+
+
+Definition final_tables_old_def:
+  final_tables_old (tbll, st_in) =
+  final_tbll_old tbll st_in
+End
+
+        
+(*
+     
+EVAL “final_tbll_old [[([False],0,state 2); ([False],0,state 3); ([True],0,state 3)];
+                  [([True],3,state 4); ([False],3,state 5); ([True],2,state 2)];
+                  [([True],2,action ("fwd",[1])); ([True],4,action ("fwd",[2]));
+               ([True],5,action ("drop",[]))]] 0 ”
+
+EVAL “final_tbll_old [[([False],0,state 2); ([False],0,state 3); ([False],0,state 3)];
+                  [([True],3,state 4); ([False],3,state 5); ([True],2,state 2)];
+                  [([True],2,action ("fwd",[1])); ([True],4,action ("fwd",[2]));
+               ([True],5,action ("drop",[]))]] 0 ”
+*)
+
+(*  free variables tables *)
+
+        
+Definition fv_row_def:
+  fv_row atoml =
+  let fv_in_row = MAP (\atom. fv_atom atom) atoml in
+    nub(FLAT fv_in_row)
+End
+
+
+Definition fv_tbl_def:
+  fv_tbl (tbl: 'a var_table) =
+  (let fv_in_tbl = MAP(\(atom,st_num,res). fv_row atom) tbl in
+      nub (FLAT fv_in_tbl))
+End
+        
+        
+
+    
+Definition fv_tbll_def:
+  fv_tbll (tbll: 'a var_table_list) =
+  let fv_in_tbll = MAP (\tbl. fv_tbl tbl) tbll in
+    nub(FLAT fv_in_tbll)
+End
+
+
+        
+Definition fv_tables_def:
+  fv_tables (tbll, st_in) =
+  fv_tbll tbll
+End
+
+
+
+        
+                                                                 
+Definition table_structure_old_def:
+  table_structure_old =
+  <|
+    sem := sem_tables;
+    sub := mk_substitute_tables;
+    simp := simp_tables_old;
+    final := final_tables_old;
+    fv := fv_tables;
+  |>
+End            
+
+
+
+
+
+
+
+
+        
+
+               
+
+               
+Theorem fv_mem_tbll_thm:
+  ∀ tbll tbl mv.
+    (∀x. MEM x (fv_tbll (tbl::tbll)) ⇒ ∃b. ALOOKUP mv x = SOME b) ⇒
+    (∀x. MEM x (fv_tbll  tbll) ⇒ ∃b. ALOOKUP mv x = SOME b)
+Proof
+  gvs[fv_tbll_def]
+QED
+
+        
+Theorem fv_mem_tbll_hd_thm:
+  ∀ tbll tbl mv.
+    (∀x. MEM x (fv_tbll (tbl::tbll)) ⇒ ∃b. ALOOKUP mv x = SOME b) ⇒
+    (∀x. MEM x (fv_tbl  tbl) ⇒ ∃b. ALOOKUP mv x = SOME b)
+Proof
+  gvs[fv_tbll_def, fv_tbl_def]
+QED
+        
+
+Theorem fv_mem_tbl_thm:
+  ∀ tbl h mv.
+    (∀x. MEM x (fv_tbl (h::tbl)) ⇒ ∃b. ALOOKUP mv x = SOME b) ⇒
+    (∀x. MEM x (fv_tbl  tbl) ⇒ ∃b. ALOOKUP mv x = SOME b)
+Proof
+  gvs[fv_tbl_def]
+QED
+
+
+Theorem fv_mem_tbl_h_thm:
+  ∀ tbl h mv.
+    (∀x. MEM x (fv_tbl (h::tbl)) ⇒ ∃b. ALOOKUP mv x = SOME b) ⇒
+    (∀x. MEM x (fv_tbl  [h]) ⇒ ∃b. ALOOKUP mv x = SOME b)
+Proof
+  gvs[fv_tbl_def]
+QED        
+
+
+
+Theorem fv_mem_row_thm:
+  ∀ atoml h mv.
+    (∀x. MEM x (fv_row (h::atoml)) ⇒ ∃b. ALOOKUP mv x = SOME b) ⇒
+    (∀x. MEM x (fv_row atoml) ⇒ ∃b. ALOOKUP mv x = SOME b)
+Proof
+  gvs[fv_row_def]
+QED 
+
+
+
+Theorem fv_mem_row_h_thm:
+  ∀ atoml h mv.
+    (∀x. MEM x (fv_row (h::atoml)) ⇒ ∃b. ALOOKUP mv x = SOME b) ⇒
+    (∀x. MEM x (fv_row [h]) ⇒ ∃b. ALOOKUP mv x = SOME b)
+Proof
+  gvs[fv_row_def]
+QED
+
+(*
+Theorem fv_mem_atom_not_thm:        
+  ∀ atom mv.
+    (∀x. MEM x (fv_row [Not atom]) ⇒ ∃b. ALOOKUP mv x = SOME b) ⇒
+    (∀x. MEM x (fv_row [atom]) ⇒ ∃b. ALOOKUP mv x = SOME b)
+Proof     
+  gvs[fv_row_def, fv_atom_def]
+QED
+*)
+
+          
+Theorem mk_substitute_tbl_normalize1:
+  ∀h rows x b.
+       mk_substitute_tbl (h::rows) x b =
+       mk_substitute_tbl [h] x b ⧺ mk_substitute_tbl rows x b
+Proof
+  gvs[mk_substitute_tbl_def]
+QED
+
+
+Theorem mk_substitute_tbl_normalize2:
+  ∀atoml st_num res rows x b.
+       mk_substitute_tbl ((atoml,st_num,res)::rows) x b =
+       (mk_substitute_row atoml x b,st_num,res)::mk_substitute_tbl rows x b
+Proof
+  gvs[mk_substitute_tbl_def]
+QED
+
+
+Theorem simp_tbl_normalize1:
+  ∀atoml st_num res rows x b.
+       simp_tbl ((atoml,st_num,res)::rows) =
+       (simp_row_old atoml,st_num,res)::simp_tbl rows
+Proof
+  gvs[simp_tbl_def]
+QED
+
+
+        
+Theorem sub_then_simp_answer_indeed_in_fv:
+  ∀ atom h' b s.                      
+    (simp_atom (mk_substitute_atom atom h' b) = Var s) ⇒
+    MEM s (fv_atom atom)
+Proof
+  Cases >>
+  rpt strip_tac >>
+  gvs[fv_atom_def, mk_substitute_atom_def, simp_atom_def] >>
+  rpt (BasicProvers.FULL_CASE_TAC >> gvs[]) >>
+  gvs[fv_atom_def, mk_substitute_atom_def, simp_atom_def] 
+QED
+
+
+Triviality mem_fv_sub_simp_tbl_triv1:
+  ∀ atom h' b x.        
+    MEM x (fv_atom (simp_atom (mk_substitute_atom atom h' b))) ⇒
+    MEM x (fv_atom atom)
+Proof
+  Cases >>
+  rpt strip_tac >>
+  gvs[fv_atom_def, mk_substitute_atom_def, simp_atom_def] >>
+  rpt (BasicProvers.FULL_CASE_TAC >> gvs[]) >>
+  gvs[fv_atom_def, mk_substitute_atom_def, simp_atom_def] 
+QED
+             
+      
+
+Theorem mem_imp_sem_tbl:
+  ∀ atom mv.
+    (∀x. MEM x (fv_atom atom) ⇒ ∃b. ALOOKUP mv x = SOME b) ⇒
+    sem_var_atom atom mv ≠ NONE ∧ ∃ b' . sem_var_atom atom mv = SOME b'
+Proof
+  Cases >>
+  rw[fv_atom_def] >> gvs[AllCaseEqs()] >>
+  gvs[sem_var_atom_def, simp_atom_def] >>
+  rpt (BasicProvers.FULL_CASE_TAC >> gvs[]) 
+QED
+
+
+Triviality non_empty_line_simp_not_empty:
+  ∀ atoml h' b.
+    atoml ≠ [] ⇔  simp_row_old (mk_substitute_row atoml h' b) ≠ []
+Proof
+  Induct >> gvs[mk_substitute_row_def, simp_row_old_def] >>
+  rpt strip_tac >>
+  rpt (BasicProvers.FULL_CASE_TAC >> gvs[])
+QED
+
+
+
+Theorem lookup_implies_sem_var_atoms_same:
+  ∀ atom h' b bool mv.
+    ALOOKUP mv h' = SOME b  ⇒
+    (sem_var_atom atom mv = SOME bool ⇔ sem_var_atom (simp_atom (mk_substitute_atom atom h' b)) mv = SOME bool)
+Proof
+  Cases >>
+  rpt strip_tac >>
+  rpt (gvs[mk_substitute_atom_def, simp_atom_def, sem_var_atom_def] >>
+       BasicProvers.FULL_CASE_TAC >>
+       res_tac >>               
+       gvs[])
+QED
+
+
+
+Theorem sem_var_atom_failure_from_simp_atom_false:        
+  ∀ atoml h' b mv.
+    atoml ≠ [] ∧
+    ALOOKUP mv h' = SOME b ∧
+    MEM False (MAP (λatom. simp_atom atom) (MAP (λatom. mk_substitute_atom atom h' b) atoml)) ⇒
+    ~ EVERY (λminipred. sem_var_atom minipred mv = SOME T) atoml
+Proof
+  Induct >>
+  rpt strip_tac >> gvs[] >>
+  imp_res_tac lookup_implies_sem_var_atoms_same >> gvs[sem_var_atom_def] >>
+  res_tac >>
+  Cases_on ‘atoml = []’ >> gvs[] >>
+  imp_res_tac NOT_EVERY
+QED
+
+        
+
+Theorem subst_simp_sound_for_atom:
+  ∀atom h' b mv.
+    ALOOKUP mv h' = SOME b ⇒
+    (simp_atom (mk_substitute_atom atom h' b) = True ⇒
+     sem_var_atom atom mv = SOME T) ∧
+    (simp_atom (mk_substitute_atom atom h' b) = False ⇒
+     sem_var_atom atom mv = SOME F)
+Proof                                   
+  Cases >>
+  gvs[simp_atom_def, mk_substitute_atom_def, sem_var_atom_def] >>
+  rpt strip_tac >>
+  rpt (BasicProvers.FULL_CASE_TAC >> gvs[simp_atom_def, mk_substitute_atom_def, sem_var_atom_def])
+QED
+
+
+       
+
+Theorem lookup_implies_sem_var_atoml_same2:
+  ∀ atoml h' b mv.
+    ALOOKUP mv h' = SOME b ∧
+    atoml ≠ [] ∧
+    EVERY ((λminipred. sem_var_atom minipred mv = SOME T)) (simp_row_old (mk_substitute_row atoml h' b)) ⇒
+    EVERY (λminipred. sem_var_atom minipred mv = SOME T) atoml
+Proof
+  Induct >>
+  rpt strip_tac >> 
+  gvs[mk_substitute_row_def, simp_row_old_def] >>
+
+  rpt (BasicProvers.FULL_CASE_TAC >> gvs[]) >>
+  gvs[sem_var_atom_def] >>
+                             
+  imp_res_tac lookup_implies_sem_var_atoms_same >> gvs[] >> res_tac >>
+  gvs[] >>
+  Cases_on ‘atoml = []’ >> gvs[]
+QED
+
+
+
+
+
+          
+Theorem simp_sub_mem_normalization:
+  ∀ atoml h h' b atom.        
+    atom ≠ simp_atom (mk_substitute_atom h h' b) ∧
+    MEM atom (simp_row_old (mk_substitute_row (h::atoml) h' b)) ⇒
+    MEM atom (simp_row_old (mk_substitute_row atoml h' b))
+Proof
+  rpt strip_tac >>
+  gvs[mk_substitute_row_def, simp_row_old_def] >>
+  rpt (BasicProvers.FULL_CASE_TAC >> gvs[]) >>
+  gvs[MEM_MAP] >> metis_tac[]
+QED
+
+
+         
+        
+
+Theorem is_match_row_substitute_preserve1:
+  ∀ atoml mv h' b s_in st_num.        
+    ALOOKUP mv h' = SOME b ∧
+    is_match_row s_in st_num atoml mv ⇒
+    is_match_row s_in st_num (simp_row_old (mk_substitute_row atoml h' b)) mv
+Proof
+  Induct >>
+  gvs[is_match_row_def] >>
+  rpt strip_tac >>
+  gvs[is_atoml_true_def] >>
+  
+  Cases_on ‘atoml = []’ >> gvs[] >|[
+    simp[mk_substitute_row_def, simp_row_old_def] >>
+    rpt (BasicProvers.FULL_CASE_TAC >> gvs[sem_var_atom_def]) >>
+    imp_res_tac subst_simp_sound_for_atom >> gvs[] >>
+    imp_res_tac lookup_implies_sem_var_atoms_same >> gvs[]
+    ,
+    res_tac >>
+    rgs[] >>
+    gvs[Once EVERY_NOT_EXISTS] >>
+    gvs[EVERY_MEM] >>
+    gvs[EVERY_MAP] >>
+    rpt strip_tac >>
+    
+    Cases_on ‘minipred = simp_atom(mk_substitute_atom h h' b)’ >> gvs[] >>
+    res_tac >|[
+        imp_res_tac lookup_implies_sem_var_atoms_same >> gvs[]
+        ,
+        imp_res_tac simp_sub_mem_normalization >>
+        res_tac
+      ]   
+    ,
+    
+    gvs[mk_substitute_row_def, simp_row_old_def] >>
+    rpt (BasicProvers.FULL_CASE_TAC >> gvs[])
+    ,
+                                
+    res_tac >>
+    rgs[] >>
+    gvs[mk_substitute_row_def, simp_row_old_def] >>
+    rpt (BasicProvers.FULL_CASE_TAC >> gvs[])
+  ]
+QED
+
+
+
+Theorem is_match_row_substitute_preserve2:
+  ∀ atoml mv h' b s_in st_num.        
+    ALOOKUP mv h' = SOME b ∧
+    is_match_row s_in st_num (simp_row_old (mk_substitute_row atoml h' b)) mv ⇒
+    is_match_row s_in st_num atoml mv
+Proof
+  Induct >>
+  gvs[is_match_row_def] >>
+  rpt strip_tac >>
+  gvs[is_atoml_true_def] >>
+  (
+  imp_res_tac lookup_implies_sem_var_atoml_same2 >> 
+  gvs[mk_substitute_row_def, simp_row_old_def] 
+  )
+QED
+
+
+
+Theorem is_match_row_substitute_preserve:
+  ∀ atoml mv h' b (s_in:num) st_num.        
+    ALOOKUP mv h' = SOME b ⇒
+    (is_match_row s_in st_num (simp_row_old (mk_substitute_row atoml h' b)) mv =
+    is_match_row s_in st_num atoml mv)
+Proof
+  rpt strip_tac >>
+  EQ_TAC >>
+  metis_tac[is_match_row_substitute_preserve1, is_match_row_substitute_preserve2]
+QED
+
+
+
+Theorem exists_is_match_row_after_subst_simp:        
+  ∀ tbl s_in h' b mv.
+    ALOOKUP mv h' = SOME b ∧
+    EXISTS (λ(p,a). p) (MAP (λ(atoml,st_num,res). (is_match_row s_in st_num atoml mv,res)) tbl) ⇒
+    EXISTS (λ(p,a). p) (MAP (λ(atoml,st_num,res). (is_match_row s_in st_num atoml mv,res))
+                            (simp_tbl (mk_substitute_tbl tbl h' b)))
+Proof
+  Induct >-
+   gvs[mk_substitute_tbl_def, simp_tbl_def] >>
+  rpt strip_tac >>
+  simp[mk_substitute_tbl_def, simp_tbl_def] >>
+  gvs[] >|[
+  
+    PairCases_on ‘h’ >>
+    rename1 ‘(atoml, st_num, res)’ >>
+    gvs[MAP_MAP_o] >>
+    gvs[EXISTS_MAP] >>
+    imp_res_tac is_match_row_substitute_preserve1 >> gvs[]
+    ,
+    res_tac >>
+    gvs[mk_substitute_tbl_def, simp_tbl_def]
+  ]    
+QED
+
+
+Theorem exists_is_match_row_before_subst_simp:        
+  ∀ tbl s_in h' b mv.
+    ALOOKUP mv h' = SOME b ∧
+    EXISTS (λ(p,a). p) (MAP (λ(atoml,st_num,res). (is_match_row s_in st_num atoml mv,res))
+                            (simp_tbl (mk_substitute_tbl tbl h' b))) ⇒
+    EXISTS (λ(p,a). p) (MAP (λ(atoml,st_num,res). (is_match_row s_in st_num atoml mv,res)) tbl)
+Proof
+  Induct >-
+   gvs[mk_substitute_tbl_def, simp_tbl_def] >>
+  rpt strip_tac >>
+  gvs[mk_substitute_tbl_def, simp_tbl_def] >>
+  gvs[] >|[
+  
+    PairCases_on ‘h’ >>
+    rename1 ‘(atoml, st_num, res)’ >>
+    gvs[MAP_MAP_o] >>
+    gvs[EXISTS_MAP] >>
+    imp_res_tac is_match_row_substitute_preserve2 >> gvs[]
+    ,
+    res_tac >>
+    gvs[mk_substitute_tbl_def, simp_tbl_def]
+  ]    
+QED
+
+
+
+
+Theorem is_match_row_lists_subst_simp_eq:        
+∀tbl h' b mv s_in.
+       ALOOKUP mv h' = SOME b ⇒
+       MAP (λ(atoml,st_num,res). (is_match_row s_in st_num atoml mv,res))
+         (simp_tbl (mk_substitute_tbl tbl h' b)) =
+       MAP (λ(atoml,st_num,res). (is_match_row s_in st_num atoml mv,res)) tbl 
+Proof
+  Induct >>
+  rpt strip_tac >>
+  gvs[mk_substitute_tbl_def,simp_tbl_def] >>
+  PairCases_on ‘h’ >>
+  rename1 ‘(atoml, st_num, res)’ >>
+  gvs[MAP_MAP_o] >>
+  gvs[EXISTS_MAP] >>
+  res_tac >>
+                  
+  imp_res_tac is_match_row_substitute_preserve >>
+  gvs[]
+QED
+
+
+
+
+Theorem subst_simp_sem_tables_INDEX_FIND_congruence:
+  ∀ tbl mv s_in h' b i.
+    ALOOKUP mv h' = SOME b  ⇒
+    INDEX_FIND i (λ(p,a). p)
+               (MAP (λ(atoml,st_num,res). (is_match_row s_in st_num atoml mv,res)) (simp_tbl (mk_substitute_tbl tbl h' b))) =
+    INDEX_FIND i (λ(p,a). p)
+               (MAP (λ(atoml,st_num,res). (is_match_row s_in st_num atoml mv,res)) tbl)
+
+Proof
+  rpt strip_tac >>
+  imp_res_tac is_match_row_lists_subst_simp_eq >>
+  gvs[]
+QED
+
+
+
+Theorem subst_check_rows_sem_tables_INDEX_FIND_congruence:
+  ∀ tbl mv s_in h' b.
+    ALOOKUP mv h' = SOME b  ⇒
+    (check_all_rows_match s_in(simp_tbl (mk_substitute_tbl tbl h' b)) mv) =
+    (check_all_rows_match s_in tbl mv)
+Proof
+  gvs[check_all_rows_match_def] >>
+  rpt strip_tac >>
+  imp_res_tac is_match_row_lists_subst_simp_eq >>
+  gvs[]
+QED
+                      
+
+Theorem min_idx_till_subst_simp_invariant1:
+  ∀ tbl mv s_in h' b atoml st_num res .
+      ALOOKUP mv h' = SOME b  ⇒
+      min_idx_till (check_all_rows_match s_in (simp_tbl (mk_substitute_tbl ((atoml,st_num,res)::tbl) h' b)) mv) T =
+      min_idx_till (check_all_rows_match s_in ((atoml,st_num,res)::tbl) mv) T
+Proof
+  rpt strip_tac >> 
+  gvs[min_idx_till_def] >>
+  imp_res_tac subst_check_rows_sem_tables_INDEX_FIND_congruence >>
+  gvs[]  
+QED
+
+
+Theorem min_idx_till_subst_simp_invariant2:
+  ∀ tbl mv s_in h' b  .
+      ALOOKUP mv h' = SOME b  ⇒
+      min_idx_till (check_all_rows_match s_in (simp_tbl (mk_substitute_tbl (tbl) h' b)) mv) T =
+      min_idx_till (check_all_rows_match s_in (tbl) mv) T
+Proof   
+  rpt strip_tac >> 
+  gvs[min_idx_till_def] >>
+  imp_res_tac subst_check_rows_sem_tables_INDEX_FIND_congruence >>
+  gvs[]  
+QED
+
+
+Theorem sem_tables_subst_simp_invariant:
+  ∀ tbl mv s_in h' b row .
+    ALOOKUP mv h' = SOME b   ⇒
+    sem_tables ([simp_tbl (mk_substitute_tbl (row::tbl) h' b)],s_in) mv =
+    sem_tables ([row::tbl],s_in) mv
+Proof
+  rpt strip_tac >>
+  PairCases_on ‘row’ >> rename1 ‘(atoml,st_num,res)’ >>
+  gvs[] >>
+        
+  simp[sem_tables_def, match_tbll_def] >>
+  gvs[match_tbl_def] >>
+  rpt (BasicProvers.FULL_CASE_TAC >> gvs[]) >>
+  
+  imp_res_tac min_idx_till_subst_simp_invariant1 >> gvs[] 
+QED
+  
+
+     
+Theorem prop1_var_single_tbl_verbose:
+  ∀ tbl mv h' b s_in.
+    ALOOKUP mv h' = SOME b ⇒
+    sem_tables (simp_tbll (mk_substitute_tbll [tbl] h' b),s_in) mv =
+    sem_tables ([tbl],s_in) mv
+Proof
+  Cases >-
+   (gvs[fv_tbll_def, mk_substitute_tbll_def, simp_tbll_def] >> 
+   gvs[fv_tbl_def, mk_substitute_tbl_def, simp_tbl_def]) >> 
+
+  rpt strip_tac >>
+  gvs[mk_substitute_tbll_def, simp_tbll_def] >> 
+  imp_res_tac sem_tables_subst_simp_invariant >>
+  gvs[]  
+QED
+            
+
+
+            
+Theorem prop1_var_tables_old_verbose:
+  ∀ tbls h b mv s_in.
+    ALOOKUP mv h = SOME b 
+    ⇒
+    sem_tables (simp_tbll (mk_substitute_tbll tbls h b),s_in) mv =
+    sem_tables (tbls,s_in) mv
+Proof
+
+  Induct_on ‘tbls’ >> rpt strip_tac >-
+   gvs[fv_tbll_def, mk_substitute_tbll_def, simp_tbll_def] >> 
+  rename1 ‘(tbl::tbll)’ >>
+
+  imp_res_tac prop1_var_single_tbl_verbose >>
+  first_x_assum (strip_assume_tac o (Q.SPECL [‘tbl’, ‘s_in’])) >>
+                
+  Cases_on ‘tbll’ >> gvs[] >> 
+  rename1 ‘(tbl::nexttbl::tbll)’ >>
+
+  gvs[sem_tables_def, match_tbll_def] >>
+  Cases_on ‘match_tbl tbl mv s_in’ >> gvs[] >>
+  rpt (BasicProvers.FULL_CASE_TAC >> gvs[]) >>
+
+  gvs[mk_substitute_tbll_def, simp_tbll_def] >>
+  gvs[match_tbll_def] >>     
+  Cases_on ‘match_tbl (simp_tbl (mk_substitute_tbl tbl h' b)) mv s_in’ >> gvs[] >>
+  rpt (BasicProvers.FULL_CASE_TAC >> gvs[]) >>
+
+  gvs[match_tbl_def] >>
+  rpt (BasicProvers.FULL_CASE_TAC >> gvs[]) >>
+  imp_res_tac min_idx_till_subst_simp_invariant2 >> gvs[]
+QED
+
+                          
+               
+Theorem prop1_var_tables_old:
+  prop1 table_structure_old
+Proof
+  rgs[prop1_def, table_structure_old_def, fv_in_p_def] >>
+
+  rpt strip_tac >>
+  Cases_on ‘p’ >>
+  rename1 ‘(tbls, s_in)’ >>
+
+  gvs[fv_tables_def, mk_substitute_tables_def, simp_tables_old_def] >>
+  imp_res_tac prop1_var_tables_old_verbose >> gvs[]    
+QED
+
+
+Theorem is_hit_true_atoml_not_empty:
+  ∀ atoml h' b s_in st_num.        
+    is_hit s_in st_num (simp_row_old (mk_substitute_row atoml h' b)) ⇒
+    atoml ≠ []
+Proof
+  gvs[is_hit_def, all_true_def, mk_substitute_row_def, simp_row_old_def]
+QED
+
+
+
+                         
+Theorem hit_implies_match_after_subst:
+  ∀ atoml s_in st_num h' b mv.
+    ALOOKUP mv h' = SOME b ∧
+    is_hit s_in st_num (simp_row_old (mk_substitute_row atoml h' b)) ⇒
+    is_match_row s_in st_num atoml mv
+Proof
+  Induct_on ‘atoml’ >>
+  rpt strip_tac >>
+  imp_res_tac is_hit_true_atoml_not_empty >>               
+  gvs[is_hit_def, is_match_row_def] >>
+  gvs[is_atoml_true_def, mk_substitute_row_def, simp_row_old_def, all_true_def] >>
+  res_tac >>
+          
+  rpt (BasicProvers.FULL_CASE_TAC >> gvs[]) >>
+  gvs[sem_var_atom_def] >>
+
+          
+  Cases_on ‘atoml=[]’ >> gvs[] >>
+  imp_res_tac subst_simp_sound_for_atom      
+QED
+
+
+        
+        
+Theorem row_miss_preserved_by_subst_simp:
+  ∀ tbl s_in h' b mv.
+    ALOOKUP mv h' = SOME b ∧
+    EVERY ($¬ ∘ (λ(p,a). p)) (MAP (λ(atoml,st_num,res). (is_match_row s_in st_num atoml mv,res)) tbl)
+    ⇒
+    ¬ EXISTS (λx. (λ(p,a). p) ((λ(atoml,st_num,res). (is_hit s_in st_num atoml,st_num,res))
+                               ((λ(atoml,st_num,res). (simp_row_old atoml,st_num,res))
+                                ((λ(atoml,st_num,res). (mk_substitute_row atoml h' b,st_num,res)) x)))) tbl
+Proof
+Induct >> gvs[] >>                  
+rpt strip_tac >>
+PairCases_on ‘h’ >> gvs[] >>
+imp_res_tac hit_implies_match_after_subst >>
+res_tac
+QED
+
+
+
+Theorem pre_lines_are_fail_normalize:
+  ∀ l h idx st_num.
+    idx > 0 ∧
+    idx < LENGTH (h::l) ∧
+    pre_lines_are_fail (h::l) idx st_num ⇒
+    pre_lines_are_fail l (idx-1) st_num
+Proof
+  rpt strip_tac >>
+  gvs[pre_lines_are_fail_def] >>
+  imp_res_tac every_seg_property_1 >>
+  Cases_on ‘idx’ >> gvs[SUC_ADD_ONE] >>
+  res_tac >>
+  imp_res_tac every_seg_property_1 >>
+  ‘n < LENGTH l’ by gvs[] >>
+  gvs[]
+QED
+
+
+
+       
+Theorem index_find_not_prev:
+  ∀ l P r.         
+    INDEX_FIND 1 P l ≠ SOME (0,r)            
+Proof
+  Induct >> gvs[INDEX_FIND_def] >>
+  rpt strip_tac >>
+  rpt (BasicProvers.FULL_CASE_TAC >> gvs[]) >>
+  assume_tac P_hold_on_next >>
+  first_x_assum (strip_assume_tac o (Q.SPECL [‘(1:num)’, ‘l’, ‘P’, ‘(0,r)’])) >>
+  gvs[SUC_ADD_ONE]
+QED
+                          
+        
+
+Theorem index_find_not_prev_gen:
+  ∀ i l P r .
+    i > 1 ∧
+    0 < LENGTH l ⇒
+    INDEX_FIND i P l ≠ SOME (i-1,r)
+Proof
+  Induct >> gvs[INDEX_FIND_def] >>
+  rpt strip_tac >>
+  rpt (BasicProvers.FULL_CASE_TAC >> gvs[]) >>
+  assume_tac P_hold_on_next >> 
+  first_x_assum (strip_assume_tac o (Q.SPECL [‘(i:num)’, ‘l’, ‘P’, ‘(i,r)’])) >>
+  gvs[SUC_ADD_ONE] >>
+
+  Cases_on ‘i > 1’ >> gvs[] >>
+  Cases_on ‘i=1’ >> gvs[] >>
+  imp_res_tac index_find_not_prev      
+QED
+
+
+
+
+
+Theorem every_seg_property_3:         
+  ∀ n l h p.
+    0 < n ∧
+    EVERY p (SEG n 0 (h::l)) ⇒
+    EVERY p (SEG (n-1) 0 l)
+Proof
+  Induct >>
+  rpt strip_tac >>
+  gvs[SEG, SUC_ADD_ONE] >>
+  gvs[GSYM TAKE_SEG]
+QED
+        
+                        
+        
+Theorem every_simp_false_imp_sem_false:
+  ∀ atoml h' b mv.
+    atoml ≠ [] ∧
+    ALOOKUP mv h' = SOME b ∧
+    EVERY (λatom. atom = False) (simp_row_old (mk_substitute_row atoml h' b)) ⇒
+    ~ EVERY (λminipred. sem_var_atom minipred mv = SOME T) atoml
+Proof
+  Induct >-
+   gvs[mk_substitute_row_def, simp_row_old_def] >>
+  rpt strip_tac >>
+  
+  Cases_on ‘atoml=[]’ >> gvs[] >| [
+    gvs[EVERY_MEM] >>
+    gvs[mk_substitute_row_def, simp_row_old_def] >>
+    rpt (BasicProvers.FULL_CASE_TAC >> gvs[]) >>
+    imp_res_tac subst_simp_sound_for_atom >> gvs[]
+    ,
+
+    rgs[Once mk_substitute_row_def, Once simp_row_old_def] >>
+    rpt (BasicProvers.FULL_CASE_TAC >> gvs[]) >|[
+        imp_res_tac subst_simp_sound_for_atom >> gvs[]
+        ,
+        gvs[EVERY_MAP] >>
+        imp_res_tac sem_var_atom_failure_from_simp_atom_false
+      ]
+  ]
+QED
+
+
+    
+
+Theorem subst_simp_miss_implies_sem_miss:
+  ∀ atoml h' b mv st_num s_in. 
+    ALOOKUP mv h' = SOME b ∧
+    ¬is_hit s_in st_num (simp_row_old (mk_substitute_row atoml h' b)) ∧
+    all_false (simp_row_old (mk_substitute_row atoml h' b)) ⇒
+    ¬is_match_row s_in st_num atoml mv
+Proof
+  rpt strip_tac >>                   
+  gvs[all_false_def, is_match_row_def, is_hit_def] >>
+  gvs[is_atoml_true_def] >-
+   imp_res_tac every_simp_false_imp_sem_false >>
+  gvs[mk_substitute_row_def, simp_row_old_def] >>
+  rpt (BasicProvers.FULL_CASE_TAC >> gvs[])
+QED
+
+
+
+
+        
+Theorem index_find_agreement_under_subst_and_all_false_prefix:       
+∀ tbl (s_in:num) n st_num st_num' res q (res':'a action_expr) h' b mv.
+  ALOOKUP mv h' = SOME b ∧
+EVERY (λ(atoml,st_num',res'). st_num' = s_in ⇒ all_false atoml)
+               (SEG n 0
+                  (MAP
+                     ((λ(atoml,st_num,res). (simp_row_old atoml,st_num,res)) ∘
+                      (λ(atoml,st_num,res).
+                           (mk_substitute_row atoml h' b,st_num,res))) tbl)) ∧
+INDEX_FIND 0 (λ(p,a). p)
+               (MAP
+                  (λ(atoml,st_num,res).
+                       (is_match_row s_in st_num atoml mv,res)) tbl) =
+             SOME (q − 1,T,res') ∧
+INDEX_FIND 0 (λ(p,a). p)
+               (MAP
+                  ((λ(atoml,st_num,res).
+                        (is_hit s_in st_num atoml,st_num,res)) ∘
+                   (λ(atoml,st_num,res). (simp_row_old atoml,st_num,res)) ∘
+                   (λ(atoml,st_num,res).
+                        (mk_substitute_row atoml h' b,st_num,res))) tbl) =
+             SOME (n,T,st_num,res) ⇒
+res=res'
+Proof
+
+Induct >|[
+    gvs[INDEX_FIND_def]
+    ,
+    rpt strip_tac >>
+    PairCases_on ‘h’ >>
+    gvs[INDEX_FIND_def] >>
+    rpt (BasicProvers.FULL_CASE_TAC >> gvs[]) >|[
+                                    
+        imp_res_tac hit_implies_match_after_subst
+        ,
+        Cases_on ‘h1 = s_in’ >|[
+              Cases_on ‘q=0’ >> gvs[] >|[
+                Cases_on ‘n’ >>
+                gvs[SEG, SUC_ADD_ONE] >>
+                gvs[GSYM TAKE_SEG] >>
+                gvs[index_find_not_prev] >>
+                imp_res_tac subst_simp_miss_implies_sem_miss
+                ,
+                ‘q=1’ by gvs[] >>
+                gvs[] >>
+                Cases_on ‘n’ >>
+                gvs[SEG, SUC_ADD_ONE] >>
+                gvs[GSYM TAKE_SEG] >>
+                gvs[index_find_not_prev] >>
+                imp_res_tac subst_simp_miss_implies_sem_miss
+              ]                                       
+                                                
+            ,
+            gvs[is_hit_def, is_match_row_def]
+          ]
+                                        
+        ,
+        
+        
+        assume_tac (INST_TYPE [“:'a” |-> “:(bool # 'a action_expr)”,
+                               “:'b” |-> “:num”] P_hold_on_next)  >>
+        first_x_assum (strip_assume_tac o (Q.SPECL [‘0’,
+         ‘(MAP (λ(atoml,st_num,res). (is_match_row (s_in:num) st_num atoml mv,res)) tbl)’,
+         ‘(λ(p,a). p)’, ‘(q − 1,T,(res':α action_expr))’])) >>
+        gvs[] >>
+
+
+
+
+        
+        assume_tac (INST_TYPE [“:'a” |-> “:(bool # num # 'a action_expr)”] P_hold_on_next)  >>
+        first_x_assum (strip_assume_tac o (Q.SPECL [‘0’,
+         ‘(MAP ((λ(atoml,st_num,res). (is_hit s_in st_num atoml,st_num,res)) ∘
+                (λ(atoml,st_num,res). (simp_row_old atoml,st_num,res)) ∘
+                (λ(atoml,st_num,res). (mk_substitute_row atoml h' b,st_num,res))) tbl)’,
+         ‘(λ(p,a). p)’, ‘(n,T,st_num,res)’])) >>
+        gvs[] >>
+
+
+
+        imp_res_tac every_seg_property_3 >>
+        last_x_assum (strip_assume_tac o (Q.SPECL [‘s_in’, ‘n-1’, ‘st_num’, ‘res’,
+                                                   ‘q-1’ ,‘res'’, ‘h'’, ‘b’, ‘mv’])) >>
+        gvs[]    
+      ]
+]
+QED
+
+
+
+
+                           
+    
+
+    
+Theorem prop2_var_single_tbl_verbose:
+  ∀ tbl mv h' b res s_in.
+    ALOOKUP mv h' = SOME b ∧
+    final_tbl_old  (simp_tbl (mk_substitute_tbl tbl h' b)) s_in = SOME res ⇒
+    match_tbl tbl mv s_in = SOME res
+Proof       
+  
+  Cases_on ‘tbl’ >| [
+    gvs[fv_tbl_def, mk_substitute_tbl_def, simp_tbl_def, final_tbl_old_def,
+        min_idx_till_def, is_hit_tbl_check_def, INDEX_FIND_def]
+    ,
+    rpt strip_tac >>
+    gvs[mk_substitute_tbl_def, simp_tbl_def, final_tbl_old_def] >>
+    gvs[match_tbl_def] >>
+    rpt (BasicProvers.FULL_CASE_TAC >> gvs[]) >>
+    
+    rename1 ‘(idx,bool,st_num,res)’ >>
+    PairCases_on ‘h’ >>
+    gvs[is_hit_tbl_check_def, check_all_rows_match_def] >>
+    gvs[min_idx_till_def] >|[
+        
+        
+        gvs[INDEX_FIND_def] >>
+        rpt (BasicProvers.FULL_CASE_TAC >> gvs[])  >|[
+          imp_res_tac hit_implies_match_after_subst
+          ,
+          imp_res_tac INDEX_FIND_NONE_EXISTS >>
+          imp_res_tac exists_index_some >>
+          gvs[EXISTS_MAP] >>
+          gvs[MAP_MAP_o] >>
+          imp_res_tac row_miss_preserved_by_subst_simp
+        ]
+        ,
+        
+        
+        gvs[INDEX_FIND_def] >>
+        rpt (BasicProvers.FULL_CASE_TAC >> gvs[]) >|[
+            imp_res_tac hit_implies_match_after_subst
+            ,
+            
+            gvs[pre_lines_are_fail_def] >>
+            Cases_on ‘idx’ >>
+            gvs[SEG, SUC_ADD_ONE] >>
+            gvs[GSYM TAKE_SEG] >| [
+                gvs[index_find_not_prev]
+                ,
+                Cases_on ‘h1 = s_in’ >|[
+                    imp_res_tac subst_simp_miss_implies_sem_miss >>
+                    gvs[]
+                    ,
+                    gvs[is_hit_def, is_match_row_def]
+                  ]
+              ]
+            ,
+
+
+            gvs[pre_lines_are_fail_def] >>
+            Cases_on ‘idx’ >>
+            gvs[SEG, SUC_ADD_ONE] >>
+            gvs[GSYM TAKE_SEG] >>
+            gvs[index_find_not_prev] >>
+            PairCases_on ‘r’ >> gvs[] >>
+            
+            Cases_on ‘h1=s_in’ >|[
+                
+                
+                assume_tac (INST_TYPE [“:'a” |-> “:(bool # 'a action_expr)”,
+                                       “:'b” |-> “:num”] P_hold_on_next)  >>
+                first_x_assum (strip_assume_tac o (Q.SPECL [‘0’,
+                               ‘(MAP (λ(atoml,st_num,res). (is_match_row (h1:num) st_num atoml mv,res)) t)’,
+                               ‘(λ(p,a). p)’, ‘(q,r0,r1)’])) >>
+                gvs[] >>
+                
+                assume_tac (INST_TYPE [“:'a” |-> “:(bool # num # 'a action_expr)”] P_hold_on_next)  >>
+                first_x_assum (strip_assume_tac o (Q.SPECL [‘0’,
+                               ‘(MAP (λ(atoml,st_num,res). (is_hit h1 st_num atoml,st_num,res))
+                                (MAP (λ(atoml,st_num,res). (simp_row_old atoml,st_num,res))
+                                (MAP (λ(atoml,st_num,res). (mk_substitute_row atoml h' b,st_num,res)) t)))’,
+                               ‘(λ(p,a). p)’, ‘(n + 1,bool,st_num,res)’])) >>
+
+
+                gvs[] >>
+                
+                
+                ‘(λ(p,a). p) (bool,st_num,res)’ by imp_res_tac INDEX_FIND_EQ_SOME_0 >>
+                ‘(λ(p,a). p) (r0,r1)’ by imp_res_tac INDEX_FIND_EQ_SOME_0 >>
+                
+                gvs[] >>
+                
+                
+                gvs[MAP_MAP_o] >>
+                imp_res_tac index_find_agreement_under_subst_and_all_false_prefix >>
+                gvs[]
+                   
+                ,
+                
+                assume_tac (INST_TYPE [“:'a” |-> “:(bool # 'a action_expr)”,
+                                       “:'b” |-> “:num”] P_hold_on_next)  >>
+                first_x_assum (strip_assume_tac o (Q.SPECL [‘0’,
+                               ‘(MAP (λ(atoml,st_num,res). (is_match_row (s_in:num) st_num atoml mv,res)) t)’,
+                               ‘(λ(p,a). p)’, ‘(q,r0,r1)’])) >>
+                gvs[] >>
+                
+                assume_tac (INST_TYPE [“:'a” |-> “:(bool # num # 'a action_expr)”] P_hold_on_next)  >>
+                first_x_assum (strip_assume_tac o (Q.SPECL [‘0’,
+                           ‘(MAP (λ(atoml,st_num,res). (is_hit s_in st_num atoml,st_num,res))
+                            (MAP (λ(atoml,st_num,res). (simp_row_old atoml,st_num,res))
+                            (MAP (λ(atoml,st_num,res). (mk_substitute_row atoml h' b,st_num,res)) t)))’,
+                           ‘(λ(p,a). p)’, ‘(n + 1,bool,st_num,res)’])) >>
+
+
+                gvs[] >>
+          
+          
+                ‘(λ(p,a). p) (bool,st_num,res)’ by imp_res_tac INDEX_FIND_EQ_SOME_0 >>
+                ‘(λ(p,a). p) (r0,r1)’ by imp_res_tac INDEX_FIND_EQ_SOME_0 >>
+                
+                gvs[] >>
+                
+                
+                gvs[MAP_MAP_o] >>
+                imp_res_tac index_find_agreement_under_subst_and_all_false_prefix >>
+                gvs[]
+              ] 
+          ]
+      ]
+  ]         
+QED
+
+
+
+
+        
+
+Theorem prop2_var_tables_old_verbose:
+  ∀ tbls h b mv s_in res.
+    ALOOKUP mv h = SOME b ∧
+    final_tbll_old (simp_tbll (mk_substitute_tbll tbls h b)) s_in = SOME res ⇒
+    sem_tables (tbls,s_in) mv = SOME res 
+Proof
+
+  Induct_on ‘tbls’ >> rpt strip_tac >-
+   gvs[mk_substitute_tbll_def, simp_tbll_def, final_tbll_old_def] >> 
+  rename1 ‘(tbl::tbll)’ >>
+
+
+  Cases_on ‘tbll’ >> gvs[] >|[
+    
+    gvs[sem_tables_def, match_tbll_def] >>
+    gvs[mk_substitute_tbll_def, simp_tbll_def, final_tbll_old_def] >>
+    gvs[] >>
+    rpt (BasicProvers.FULL_CASE_TAC >> gvs[]) >>
+    
+    imp_res_tac prop2_var_single_tbl_verbose >> gvs[]              
+    ,
+    rename1 ‘(tbl::nexttbl::tbll)’ >>
+    rgs[Once mk_substitute_tbll_def, Once simp_tbll_def] >>
+    rgs[Once final_tbll_old_def] >>     
+
+    Cases_on ‘final_tbl_old  (simp_tbl (mk_substitute_tbl tbl h' b)) s_in’ >>
+    gvs[] >>
+    Cases_on ‘x’ >>
+    gvs[] >>
+    
+    rgs[Once mk_substitute_tbll_def, Once simp_tbll_def] >>
+    rgs[Once final_tbll_old_def] >>  
+    res_tac >>
+
+    gvs[sem_tables_def, match_tbll_def] >>
+    gvs[mk_substitute_tbll_def, simp_tbll_def, final_tbll_old_def] >>
+    gvs[] >>
+    rpt (BasicProvers.FULL_CASE_TAC >> gvs[]) >>
+    
+    imp_res_tac prop2_var_single_tbl_verbose >> gvs[]     
+  ]
+QED
+
+
+
+Theorem prop2_var_tables_old:
+  prop2 table_structure_old
+Proof
+  rgs[prop2_def, table_structure_old_def, fv_in_p_def] >>
+
+  rpt strip_tac >>
+  Cases_on ‘p’ >>
+  rename1 ‘(tbls, s_in)’ >>
+
+  gvs[final_tables_old_def, fv_tables_def, mk_substitute_tables_def, simp_tables_old_def] >>
+  imp_res_tac prop1_var_tables_old_verbose >> gvs[] >>
+  imp_res_tac prop2_var_tables_old_verbose >> gvs[]
+QED
+
+
+                   
+Theorem hit_implies_match_after_all:
+  ∀ atoml s_in st_num h' b mv.
+    is_hit s_in st_num atoml ⇒
+    is_match_row s_in st_num atoml mv
+Proof
+  Induct_on ‘atoml’ >>
+  rpt strip_tac >>
+  gvs[is_hit_def, is_match_row_def] >>
+  gvs[is_atoml_true_def,all_true_def] >>
+  res_tac >>
+  Cases_on ‘atoml=[]’ >>
+  gvs[sem_var_atom_def]
+QED
+
+
+
+Theorem subst_simp_miss_implies_sem_miss_full:
+  ∀ atoml h' b mv s_in st_num .
+    ¬is_hit s_in st_num (simp_row_old (mk_substitute_row atoml h' b)) ∧
+    all_false (simp_row_old (mk_substitute_row atoml h' b)) ⇒
+    ¬is_match_row s_in st_num  (simp_row_old (mk_substitute_row atoml h' b)) mv
+Proof
+  Induct >>
+  rpt strip_tac >>                   
+  gvs[all_false_def, is_match_row_def, is_hit_def] >>
+  gvs[is_atoml_true_def, all_true_def] >>
+  gvs[mk_substitute_row_def, simp_row_old_def] >>
+  res_tac >>
+  rpt (BasicProvers.FULL_CASE_TAC >> gvs[]) >>
+  gvs[mk_substitute_row_def, simp_row_old_def, sem_var_atom_def]
+QED
+
+
+
+        
+
+Theorem match_follows_hit_at_minimal_index:
+  ∀ tbl s_in idx  bool  st_num res mv h' b.
+    pre_lines_are_fail (simp_tbl (mk_substitute_tbl tbl h' b)) idx s_in ∧
+    min_idx_till (is_hit_tbl_check (simp_tbl (mk_substitute_tbl tbl h' b)) s_in) T =
+    SOME (idx,bool,st_num,res)  ⇒
+    min_idx_till (check_all_rows_match s_in (simp_tbl (mk_substitute_tbl tbl h' b)) mv) T =
+    SOME (idx,bool,res)
+Proof
+  gvs[min_idx_till_def] >>
+  Induct >>
+  rpt strip_tac >-
+   gvs[mk_substitute_tbl_def, check_all_rows_match_def, simp_tbl_def,
+       is_hit_tbl_check_def, INDEX_FIND_def] >>
+  
+  
+  PairCases_on ‘h’ >>
+  gvs[simp_tbl_def, mk_substitute_tbl_def, is_hit_tbl_check_def] >>
+  gvs[INDEX_FIND_def]>>
+  rpt (BasicProvers.FULL_CASE_TAC >> gvs[]) >|[
+    
+    gvs[check_all_rows_match_def, INDEX_FIND_def] >>
+    rpt (BasicProvers.FULL_CASE_TAC >> gvs[])>>
+    imp_res_tac hit_implies_match_after_all >>
+    gvs[]
+    ,
+
+    gvs[check_all_rows_match_def, INDEX_FIND_def]>>
+    rpt (BasicProvers.FULL_CASE_TAC >> gvs[]) >|[
+
+        gvs[pre_lines_are_fail_def] >>
+        Cases_on ‘idx’ >>
+        gvs[SEG, SUC_ADD_ONE] >>
+        gvs[GSYM TAKE_SEG] >>
+        gvs[index_find_not_prev] >>
+                                 
+        Cases_on ‘h1 = s_in’ >> gvs[] >>
+        imp_res_tac subst_simp_miss_implies_sem_miss_full >> gvs[is_hit_def, is_match_row_def]
+                                                                    
+        ,
+        gvs[MAP_MAP_o] >>
+        gvs[pre_lines_are_fail_def] >>
+        Cases_on ‘idx’ >>
+        gvs[SEG, SUC_ADD_ONE] >>
+        gvs[GSYM TAKE_SEG] >>
+        gvs[index_find_not_prev] >>
+        
+        
+        
+        assume_tac (INST_TYPE [“:'a” |-> “:(bool # num # 'a action_expr)”] P_hold_on_next)  >>
+        first_x_assum (strip_assume_tac o (Q.SPECL [‘0’,
+            ‘(MAP ((λ(atoml,st_num,res). (is_hit s_in st_num atoml,st_num,res)) ∘
+              (λ(atoml,st_num,res). (simp_row_old atoml,st_num,res)) ∘
+              (λ(atoml,st_num,res). (mk_substitute_row atoml h' b,st_num,res))) tbl)’,
+            ‘(λ(p,a). p)’, ‘(n + 1,bool,st_num,res)’])) >>
+          gvs[] >>
+          
+        
+        res_tac >>
+        first_x_assum (strip_assume_tac o (Q.SPECL [‘mv’])) >>
+        drule P_implies_next >>
+        gvs[]
+  ] 
+]
+QED
+
+
+        
+
+Theorem final_tbl_old_yields_match_tbl:      
+  ∀ tbl s_in mv res h' b.
+    final_tbl_old  (simp_tbl (mk_substitute_tbl tbl h' b)) s_in = SOME res ⇒
+    match_tbl (simp_tbl (mk_substitute_tbl tbl h' b)) mv s_in = SOME res
+Proof
+  rpt strip_tac >>
+  gvs[final_tbl_old_def, match_tbl_def] >>
+  rpt (BasicProvers.FULL_CASE_TAC >> gvs[]) >>
+  imp_res_tac match_follows_hit_at_minimal_index >> gvs[]
+QED
+
+
+Theorem final_tbll_old_yields_match_tbll:                            
+  ∀ tbll s_in h b mv q .
+    final_tbll_old (simp_tbll (mk_substitute_tbll tbll h b)) s_in = SOME q ⇒
+    match_tbll (simp_tbll (mk_substitute_tbll tbll h b))  mv s_in = SOME q
+Proof
+
+  Induct >-
+   (gvs[mk_substitute_tbll_def, simp_tbll_def, final_tbll_old_def]) >>
+  
+  
+  rpt strip_tac >>
+  Cases_on ‘tbll’ >|[
+    simp[match_tbll_def] >>
+    gvs[mk_substitute_tbll_def, simp_tbll_def, final_tbll_old_def] >>
+    rpt (BasicProvers.FULL_CASE_TAC >> gvs[]) >>
+    imp_res_tac final_tbl_old_yields_match_tbl >> gvs[match_tbll_def]
+    ,
+    
+    gvs[mk_substitute_tbll_def, simp_tbll_def, final_tbll_old_def] >>
+    rpt (BasicProvers.FULL_CASE_TAC >> gvs[]) >>
+    res_tac >>
+    
+    gvs[match_tbll_def] >>
+    rpt (BasicProvers.FULL_CASE_TAC >> gvs[]) >>
+    imp_res_tac final_tbl_old_yields_match_tbl >> gvs[match_tbll_def]
+  ]
+QED
+
+
+
+
+Theorem prop3_var_tables_old:
+  prop3 table_structure_old
+Proof
+  rgs[prop3_def, table_structure_old_def, fv_in_p_def] >>
+
+  rpt strip_tac >>
+  Cases_on ‘p’ >>
+  rename1 ‘(tbls, s_in)’ >>
+  gvs[final_tables_old_def, simp_tables_old_def, mk_substitute_tables_def, sem_tables_def] >>
+  imp_res_tac final_tbll_old_yields_match_tbll >> gvs[]
+QED
+
+
+
+
+
+
+Theorem fv_mem_tbll_varslist_thm:
+  ∀ tbll tbl varslist.
+    (∀x. MEM x (fv_tbll (tbl::tbll)) ⇒ MEM x varslist) ⇒
+    (∀x. MEM x (fv_tbll  tbll) ⇒  MEM x varslist)
+Proof
+  gvs[fv_tbll_def]
+QED
+
+
+
+Theorem free_vars_simp_subst_in_original:
+  ∀ atom h' b x.
+    MEM x (fv_atom (simp_atom (mk_substitute_atom atom h' b))) ⇒
+    MEM x (fv_atom atom)
+Proof
+  Induct >>
+  gvs[fv_atom_def, simp_atom_def, mk_substitute_atom_def] >>
+  rpt strip_tac >>
+  rpt (BasicProvers.FULL_CASE_TAC >> gvs[]) >>
+  gvs[fv_atom_def, simp_atom_def, mk_substitute_atom_def] 
+QED
+      
+
+        
+Theorem free_vars_simp_subst_row_in_original:
+  ∀ row h' b x.
+    MEM x (fv_row (simp_row_old (mk_substitute_row row h' b))) ⇒
+    MEM x (fv_row row)
+Proof
+  Induct >>
+  gvs[fv_row_def, simp_row_old_def, mk_substitute_row_def] >>
+  rpt strip_tac >>
+  gvs[MEM_FLAT] >>
+  res_tac >>
+  first_x_assum (strip_assume_tac o (Q.SPECL [‘h'’, ‘b’])) >>
+  gvs[] >>
+  rpt (BasicProvers.FULL_CASE_TAC >> gvs[fv_atom_def]) >>
+  gvs[MEM_MAP] >> gvs[fv_atom_def] >>
+  imp_res_tac free_vars_simp_subst_in_original >> gvs[] >>
+  DISJ2_TAC >> gvs[] >>
+  metis_tac[]
+QED
+
+
+
+        
+Theorem free_vars_simp_subst_tbl_in_original:
+  ∀ tbl x h' b.
+    MEM x (fv_tbl (simp_tbl (mk_substitute_tbl tbl h' b))) ⇒
+    MEM x (fv_tbl tbl)
+Proof
+  Induct >>
+  rpt strip_tac >>
+  gvs[fv_tbl_def, mk_substitute_tbl_def, simp_tbl_def] >|[
+    PairCases_on ‘h’ >> gvs[] >>
+    imp_res_tac free_vars_simp_subst_row_in_original >>
+    gvs[]
+    ,
+    res_tac >> gvs[]
+  ]
+QED                                                         
+      
+
+Theorem free_vars_simp_subst_tbll_in_original:
+  ∀ tbls h b x varslist.
+    (∀x'. MEM x' (fv_tbll tbls) ⇒ MEM x' varslist) ∧
+    MEM x (fv_tbll (simp_tbll (mk_substitute_tbll tbls h b))) ⇒
+    MEM x varslist
+Proof
+  Induct >-
+   (gvs[fv_tbll_def, mk_substitute_tbll_def, simp_tbll_def]) >>
+  
+  rpt strip_tac >>    
+  gvs[mk_substitute_tbll_def, simp_tbll_def] >>
+  imp_res_tac fv_mem_tbll_varslist_thm >>
+  res_tac >>
+  gvs[fv_tbll_def] >|[
+    imp_res_tac free_vars_simp_subst_tbl_in_original >>
+    gvs[]
+    ,
+    metis_tac[]      
+  ]                            
+QED
+
+        
+
+Theorem prop4_var_tables_old:
+  prop4 table_structure_old
+Proof
+  rgs[prop4_def, table_structure_old_def, fv_in_p_def, fv_in_vars_def] >>
+
+  rpt strip_tac >>
+  Cases_on ‘prop_parent’ >>
+  rename1 ‘(tbls, s_in)’ >>
+  gvs[fv_tables_def, simp_tables_old_def, mk_substitute_tables_def] >>
+  imp_res_tac free_vars_simp_subst_tbll_in_original
+QED
+
+
+
+
+                 
+val _ = export_theory ();
+
+    
